@prefix : <http://stko-kwg.geog.ucsb.edu/lod/ontology/> .
@prefix sf: <http://www.opengis.net/ont/sf#> .
@prefix c4o: <http://purl.org/spar/c4o/> .
@prefix owl: <http://www.w3.org/2002/07/owl#> .
@prefix rdf: <http://www.w3.org/1999/02/22-rdf-syntax-ns#> .
@prefix xml: <http://www.w3.org/XML/1998/namespace> .
@prefix xsd: <http://www.w3.org/2001/XMLSchema#> .
@prefix core: <http://purl.org/vocab/frbr/core/> .
@prefix gnis: <http://gnis-ld.org/lod/gnis/ontology/> .
@prefix irdr: <http://www.knowwheregraph.org/ontologies/hazard/IRDR/> .
@prefix kwgr: <http://stko-kwg.geog.ucsb.edu/lod/resource/> .
@prefix qudt: <http://qudt.org/1.1/schema/qudt#> .
@prefix rdfs: <http://www.w3.org/2000/01/rdf-schema#> .
@prefix skos: <http://www.w3.org/2004/02/skos/core#> .
@prefix sosa: <http://www.w3.org/ns/sosa/> .
@prefix time: <http://www.w3.org/2006/time#> .
@prefix usgs: <http://gnis-ld.org/lod/usgs/ontology/> .
@prefix terms: <http://purl.org/dc/terms/> .
@prefix schema: <http://schema.org/> .
@prefix geocode: <http://ld.iospress.nl/rdf/geocode/> .
@prefix kwg-ont: <http://stko-kwg.geog.ucsb.edu/lod/ontology/> .
@prefix iospress: <http://ld.iospress.nl/rdf/ontology/> .
@prefix wgs84_pos: <http://www.w3.org/2003/01/geo/wgs84_pos#> .
@base <http://stko-kwg.geog.ucsb.edu/lod/ontology/> .

<http://stko-kwg.geog.ucsb.edu/lod/ontology/> rdf:type owl:Ontology ;
                                               terms:contributor """Krysztof Janowicz,
Pascal Hitzler,
Mark Schildhauer,
Wenwen Li,
Dean Rehnberger,
Shirly Stephen,
Rui Zhu,
Cogan Shimizu,
Lu Zhou,
Ling Cai,
Joseph Zalewski,
Meilin Shi,
Yuanyuan Tian,
Sizhe Wang,
Zhangyu Wang,
Gengchen Mai,
Colby Fisher,
Zilong Liu,
Antrea Christou,
Abhilekha Dalal,
Mohammad Saeid Mahdavinejad,
Seila Gonzales,
David Smith,
Bryce Mecum,
Anna Lopez-Carr,
Andrew Schroeder,
Thomas Thelen,
Kitty Currier,
Anthony D'Onofrio"""@en ;
                                               terms:created "2023-04-11"@en ;
                                               terms:creator "The KnowWhereGraph Project" ;
                                               terms:description "This ontology supports the KnowWhereGraph"@en ;
                                               rdfs:label "KWG Integrated Ontology"@en .

#################################################################
#    Annotation properties
#################################################################

###  http://purl.org/dc/terms/contributor
terms:contributor rdf:type owl:AnnotationProperty .


###  http://purl.org/dc/terms/created
terms:created rdf:type owl:AnnotationProperty .


###  http://purl.org/dc/terms/creator
terms:creator rdf:type owl:AnnotationProperty .


###  http://purl.org/dc/terms/description
terms:description rdf:type owl:AnnotationProperty .


###  http://schema.org/domainIncludes
schema:domainIncludes rdf:type owl:AnnotationProperty .


###  http://schema.org/rangeIncludes
schema:rangeIncludes rdf:type owl:AnnotationProperty .


###  http://www.w3.org/2004/02/skos/core#definition
skos:definition rdf:type owl:AnnotationProperty .


###  http://www.w3.org/2004/02/skos/core#editorialNote
skos:editorialNote rdf:type owl:AnnotationProperty .


###  http://www.w3.org/2004/02/skos/core#example
skos:example rdf:type owl:AnnotationProperty .


###  http://www.w3.org/2004/02/skos/core#note
skos:note rdf:type owl:AnnotationProperty .


###  http://www.w3.org/2004/02/skos/core#prefLabel
skos:prefLabel rdf:type owl:AnnotationProperty .


#################################################################
#    Datatypes
#################################################################

###  http://ld.iospress.nl/rdf/datatype/artifactId
<http://ld.iospress.nl/rdf/datatype/artifactId> rdf:type rdfs:Datatype .


###  http://w3id.org/lindt/custom_datatypes#ucum
<http://w3id.org/lindt/custom_datatypes#ucum> rdf:type rdfs:Datatype .


###  http://www.opengis.net/ont/geosparql#wktLiteral
<http://www.opengis.net/ont/geosparql#wktLiteral> rdf:type rdfs:Datatype ;
                                                  rdfs:isDefinedBy <http://www.opengis.net/ont/geosparql#> ;
                                                  skos:definition "A Well-known Text serialization of a Geometry object."@en ;
                                                  skos:prefLabel "Well-known Text Literal"@en .


###  http://www.w3.org/2001/XMLSchema#date
xsd:date rdf:type rdfs:Datatype .


###  http://www.w3.org/2001/XMLSchema#duration
xsd:duration rdf:type rdfs:Datatype .


###  http://www.w3.org/2001/XMLSchema#gYear
xsd:gYear rdf:type rdfs:Datatype .


###  http://www.w3.org/2003/01/geo/wgs84_pos#wktLiteral
wgs84_pos:wktLiteral rdf:type rdfs:Datatype .


#################################################################
#    Object Properties
#################################################################

###  http://gnis-ld.org/lod/gnis/ontology/country
gnis:country rdf:type owl:ObjectProperty ;
             rdfs:label "country"@en .


###  http://gnis-ld.org/lod/gnis/ontology/county
gnis:county rdf:type owl:ObjectProperty ;
            rdfs:label "county" .


###  http://gnis-ld.org/lod/gnis/ontology/elevation
gnis:elevation rdf:type owl:ObjectProperty ;
               rdfs:label "elevation"@en .


###  http://gnis-ld.org/lod/gnis/ontology/state
gnis:state rdf:type owl:ObjectProperty ;
           rdfs:label "state"@en .


###  http://qudt.org/2.1/schema/qudt#unit
<http://qudt.org/2.1/schema/qudt#unit> rdf:type owl:ObjectProperty .


###  http://stko-kwg.geog.ucsb.edu/lod/ontology/administrativeLevel
kwg-ont:administrativeLevel rdf:type owl:ObjectProperty ;
                            rdfs:label "administrative level" .


###  http://stko-kwg.geog.ucsb.edu/lod/ontology/affectedBy
kwg-ont:affectedBy rdf:type owl:ObjectProperty ;
                   owl:inverseOf kwg-ont:affectedByInverse ;
                   rdfs:label "affected by" .


###  http://stko-kwg.geog.ucsb.edu/lod/ontology/affectedByInverse
kwg-ont:affectedByInverse rdf:type owl:ObjectProperty ;
                          rdfs:label "inverse of affected by"^^xsd:string .


###  http://stko-kwg.geog.ucsb.edu/lod/ontology/censusGeographyTime
kwg-ont:censusGeographyTime rdf:type owl:ObjectProperty .


###  http://stko-kwg.geog.ucsb.edu/lod/ontology/endsAt
kwg-ont:endsAt rdf:type owl:ObjectProperty ;
               rdfs:label "hazard ends at" .


###  http://stko-kwg.geog.ucsb.edu/lod/ontology/episodeHasPart
kwg-ont:episodeHasPart rdf:type owl:ObjectProperty ;
                       rdfs:comment "This is the relation between episodes and storm events in the NOAA storm impact dataset." ;
                       rdfs:label "episode has part" .


###  http://stko-kwg.geog.ucsb.edu/lod/ontology/hasChiefJudge
kwg-ont:hasChiefJudge rdf:type owl:ObjectProperty ;
                      rdfs:label "has chief judge" .


###  http://stko-kwg.geog.ucsb.edu/lod/ontology/hasDeclaration
kwg-ont:hasDeclaration rdf:type owl:ObjectProperty ;
                       rdfs:comment "The relationship between a diasaster and declaration in the OpenFEMA dataset" ;
                       rdfs:label "has declaration" .


###  http://stko-kwg.geog.ucsb.edu/lod/ontology/hasFireCause
kwg-ont:hasFireCause rdf:type owl:ObjectProperty ;
                     rdfs:label "has fire cause" .


###  http://stko-kwg.geog.ucsb.edu/lod/ontology/hasFireMappingAssessmentLabel
kwg-ont:hasFireMappingAssessmentLabel rdf:type owl:ObjectProperty ;
                                      owl:inverseOf kwg-ont:hasFireMappingAssessmentLabelInverse ;
                                      rdfs:label "has fire mapping assessment label" .


###  http://stko-kwg.geog.ucsb.edu/lod/ontology/hasFireMappingAssessmentLabelInverse
kwg-ont:hasFireMappingAssessmentLabelInverse rdf:type owl:ObjectProperty ;
                                             rdfs:label "has fire mapping label inverse" .


###  http://stko-kwg.geog.ucsb.edu/lod/ontology/hasGeometry
kwg-ont:hasGeometry rdf:type owl:ObjectProperty ;
                    rdfs:label "kwg - has geometry" .


###  http://stko-kwg.geog.ucsb.edu/lod/ontology/hasGeometryCollection
kwg-ont:hasGeometryCollection rdf:type owl:ObjectProperty ;
                              rdfs:label "has geometry collection" .


###  http://stko-kwg.geog.ucsb.edu/lod/ontology/hasGeometryMember
kwg-ont:hasGeometryMember rdf:type owl:ObjectProperty ;
                          owl:inverseOf kwg-ont:hasGeometryMemberInverse ;
                          rdfs:label "has geometry member"^^xsd:string .


###  http://stko-kwg.geog.ucsb.edu/lod/ontology/hasGeometryMemberInverse
kwg-ont:hasGeometryMemberInverse rdf:type owl:ObjectProperty ;
                                 rdfs:label "inverse of has geometry member"^^xsd:string .


###  http://stko-kwg.geog.ucsb.edu/lod/ontology/hasJudgeInfo
kwg-ont:hasJudgeInfo rdf:type owl:ObjectProperty ;
                     rdfs:label "has judge info" .


###  http://stko-kwg.geog.ucsb.edu/lod/ontology/hasMappingProgram
kwg-ont:hasMappingProgram rdf:type owl:ObjectProperty ;
                          owl:inverseOf kwg-ont:hasMappingProgramInverse ;
                          rdfs:label "has mapping program" .


###  http://stko-kwg.geog.ucsb.edu/lod/ontology/hasMappingProgramInverse
kwg-ont:hasMappingProgramInverse rdf:type owl:ObjectProperty ;
                                 rdfs:label "has mapping program inverse" .


###  http://stko-kwg.geog.ucsb.edu/lod/ontology/hasPart
kwg-ont:hasPart rdf:type owl:ObjectProperty ;
                rdfs:label "has part" .


###  http://stko-kwg.geog.ucsb.edu/lod/ontology/hasProgram
kwg-ont:hasProgram rdf:type owl:ObjectProperty ;
                   rdfs:comment "The relationship between disaster and program in the OpenFEMA dataset" ;
                   rdfs:label "has program" .


###  http://stko-kwg.geog.ucsb.edu/lod/ontology/hasRoadType
kwg-ont:hasRoadType rdf:type owl:ObjectProperty ;
                    rdfs:label "has road type" .


###  http://stko-kwg.geog.ucsb.edu/lod/ontology/hasSegment
kwg-ont:hasSegment rdf:type owl:ObjectProperty ;
                   rdfs:label "has hazard segment" .


###  http://stko-kwg.geog.ucsb.edu/lod/ontology/hasStormTrack
kwg-ont:hasStormTrack rdf:type owl:ObjectProperty ;
                      rdfs:label "has storm track" .


###  http://stko-kwg.geog.ucsb.edu/lod/ontology/hasStormTracklet
kwg-ont:hasStormTracklet rdf:type owl:ObjectProperty ;
                         rdfs:comment "Relation between hurricane storm and smaller storm tracklets" ;
                         rdfs:label "has storm tracklet" .


###  http://stko-kwg.geog.ucsb.edu/lod/ontology/hasTemporalScope
kwg-ont:hasTemporalScope rdf:type owl:ObjectProperty ;
                         rdfs:comment "The temporal scoping property in KWG to represent the temporal extent of a hazard feature" ;
                         rdfs:label "has temporal scope" .


###  http://stko-kwg.geog.ucsb.edu/lod/ontology/hasTraumaDescription
kwg-ont:hasTraumaDescription rdf:type owl:ObjectProperty ;
                             rdfs:label "has trauma description" .


###  http://stko-kwg.geog.ucsb.edu/lod/ontology/helipadAvailability
kwg-ont:helipadAvailability rdf:type owl:ObjectProperty ;
                            rdfs:label "helipad availability" .


###  http://stko-kwg.geog.ucsb.edu/lod/ontology/hospitalStatus
kwg-ont:hospitalStatus rdf:type owl:ObjectProperty ;
                       rdfs:label "hospital status" .


###  http://stko-kwg.geog.ucsb.edu/lod/ontology/hospitalType
kwg-ont:hospitalType rdf:type owl:ObjectProperty ;
                     rdfs:label "hospital type" .


###  http://stko-kwg.geog.ucsb.edu/lod/ontology/inCircuit
kwg-ont:inCircuit rdf:type owl:ObjectProperty ;
                  rdfs:label "in circuit" .


###  http://stko-kwg.geog.ucsb.edu/lod/ontology/mean
kwg-ont:mean rdf:type owl:ObjectProperty ;
             rdfs:comment "Divisional mean (1901-2000 period) for the measured climate property" ;
             rdfs:label "mean" .


###  http://stko-kwg.geog.ucsb.edu/lod/ontology/nominatedBy
kwg-ont:nominatedBy rdf:type owl:ObjectProperty ;
                    rdfs:label "nominated by" .


###  http://stko-kwg.geog.ucsb.edu/lod/ontology/nominatedTime
kwg-ont:nominatedTime rdf:type owl:ObjectProperty ;
                      rdfs:label "nominated time" .


###  http://stko-kwg.geog.ucsb.edu/lod/ontology/pharmacyType
kwg-ont:pharmacyType rdf:type owl:ObjectProperty ;
                     rdfs:label "pharmacy type" .


###  http://stko-kwg.geog.ucsb.edu/lod/ontology/sfContains
kwg-ont:sfContains rdf:type owl:ObjectProperty ;
                   rdfs:subPropertyOf kwg-ont:spatialRelation ;
                   owl:inverseOf kwg-ont:sfWithin ;
                   terms:description "Exists if the subject SpatialObject spatially contains the object SpatialObject. DE-9IM: T*****FF*" ;
                   rdfs:comment "KWG's spatial contains relation" ;
                   rdfs:label "contains (simple feature)" .


###  http://stko-kwg.geog.ucsb.edu/lod/ontology/sfCrosses
kwg-ont:sfCrosses rdf:type owl:ObjectProperty ;
                  rdfs:subPropertyOf kwg-ont:spatialRelation ;
                  terms:description "Exists if the subject SpatialObject spatially crosses the object SpatialObject. DE-9IM: T*T******" ;
                  rdfs:comment "KWG's spatial comment relation" ;
                  rdfs:label "crosses (simple feature)" .


###  http://stko-kwg.geog.ucsb.edu/lod/ontology/sfEquals
kwg-ont:sfEquals rdf:type owl:ObjectProperty ;
                 rdfs:subPropertyOf kwg-ont:spatialRelation ;
                 terms:description "Exists if the subject SpatialObject spatially equals the object SpatialObject. DE-9IM: TFFFTFFFT" ;
                 rdfs:comment "KWG's spatial equal relation" ;
                 rdfs:label "equals (simple feature)" .


###  http://stko-kwg.geog.ucsb.edu/lod/ontology/sfOverlaps
kwg-ont:sfOverlaps rdf:type owl:ObjectProperty ;
                   rdfs:subPropertyOf kwg-ont:spatialRelation ;
                   terms:description "Exists if the subject SpatialObject spatially overlaps the object SpatialObject. DE-9IM: T*T***T**" ;
                   rdfs:comment "KWG's spatial overlap relation" ;
                   rdfs:label "overlaps (simple feature)" .


###  http://stko-kwg.geog.ucsb.edu/lod/ontology/sfTouches
kwg-ont:sfTouches rdf:type owl:ObjectProperty ;
                  rdfs:subPropertyOf kwg-ont:spatialRelation ;
                  terms:description """Exists if the subject SpatialObject spatially touches the object SpatialObject.
DE-9IM: FT******* ^ F**T***** ^ F***T****""" ;
                  rdfs:comment "KWG's spatial touches relation" ;
                  rdfs:label "touches (simple feature)" .


###  http://stko-kwg.geog.ucsb.edu/lod/ontology/sfWithin
kwg-ont:sfWithin rdf:type owl:ObjectProperty ;
                 rdfs:subPropertyOf kwg-ont:spatialRelation ;
                 terms:description "Exists if the subject SpatialObject is spatially within the object SpatialObject. DE-9IM: T*F**F***" ;
                 rdfs:comment "KWG's spatial within relation" ;
                 rdfs:label "within (simple feature)" .


###  http://stko-kwg.geog.ucsb.edu/lod/ontology/spatialRelation
kwg-ont:spatialRelation rdf:type owl:ObjectProperty ,
                                 owl:SymmetricProperty ;
                        rdfs:comment "KWG's general spatial relation" ;
                        rdfs:label "spatial relation" .


###  http://stko-kwg.geog.ucsb.edu/lod/ontology/startsFrom
kwg-ont:startsFrom rdf:type owl:ObjectProperty ;
                   rdfs:label "hazard starts from" ,
                              "road segment starts from" .


###  http://stko-kwg.geog.ucsb.edu/lod/ontology/target
kwg-ont:target rdf:type owl:ObjectProperty ;
               rdfs:comment "This property denotes the relation between an observation and a S2 Cell. This is analogous to a the property sosa:hasFearureOfInterest." ;
               rdfs:label "target" .


###  http://stko-kwg.geog.ucsb.edu/lod/ontology/timeScale
kwg-ont:timeScale rdf:type owl:ObjectProperty ;
                  rdfs:comment "Property that measures the duration over which NOAA's climate division observation measurements are made" ;
                  rdfs:label "time scale" .


###  http://stko-kwg.geog.ucsb.edu/lod/ontology/traumaCareLevel
kwg-ont:traumaCareLevel rdf:type owl:ObjectProperty ;
                        rdfs:label "trauma care level" .


###  http://stko-kwg.geog.ucsb.edu/lod/ontology/traumaDescriptionSourceDate
kwg-ont:traumaDescriptionSourceDate rdf:type owl:ObjectProperty ;
                                    rdfs:label "trauma description source date" .


###  http://stko-kwg.geog.ucsb.edu/lod/ontology/typeOfLSAD
kwg-ont:typeOfLSAD rdf:type owl:ObjectProperty ;
                   rdfs:comment "The legal/statistical area description (LSAD) codes describe the particular typology for each geographic entity." ;
                   rdfs:label "type of legal/statistical area description (LSAD) area" .


###  http://stko-kwg.geog.ucsb.edu/lod/ontology/value
kwg-ont:value rdf:type owl:ObjectProperty ;
              rdfs:comment "Divisional value (1-month period)of the measured climate property" ;
              rdfs:label "value" .


###  http://www.opengis.net/ont/geosparql#hasDefaultGeometry
<http://www.opengis.net/ont/geosparql#hasDefaultGeometry> rdf:type owl:ObjectProperty .


###  http://www.opengis.net/ont/geosparql#hasGeometry
<http://www.opengis.net/ont/geosparql#hasGeometry> rdf:type owl:ObjectProperty .


###  http://www.opengis.net/ont/geosparql#spatialRelation
<http://www.opengis.net/ont/geosparql#spatialRelation> rdf:type owl:ObjectProperty .


###  http://www.w3.org/2006/time#hasBeginning
time:hasBeginning rdf:type owl:ObjectProperty ;
                  rdfs:subPropertyOf time:hasTime .


###  http://www.w3.org/2006/time#hasDuration
time:hasDuration rdf:type owl:ObjectProperty ;
                 rdfs:subPropertyOf time:hasTemporalDuration ;
                 rdfs:label "has duration"@en .


###  http://www.w3.org/2006/time#hasDurationDescription
time:hasDurationDescription rdf:type owl:ObjectProperty ;
                            rdfs:subPropertyOf time:hasTemporalDuration ;
                            rdfs:label "has duration description"@en .


###  http://www.w3.org/2006/time#hasEnd
time:hasEnd rdf:type owl:ObjectProperty ;
            rdfs:subPropertyOf time:hasTime .


###  http://www.w3.org/2006/time#hasTemporalDuration
time:hasTemporalDuration rdf:type owl:ObjectProperty ;
                         rdfs:label "has temporal duration"@en .


###  http://www.w3.org/2006/time#hasTime
time:hasTime rdf:type owl:ObjectProperty ;
             rdfs:label "has time"@en .


###  http://www.w3.org/ns/sosa/hasFeatureOfInterest
sosa:hasFeatureOfInterest rdf:type owl:ObjectProperty ;
                          owl:inverseOf sosa:isFeatureOfInterestOf ;
                          rdfs:label "hasFeatureOfInterest"^^xsd:string .


###  http://www.w3.org/ns/sosa/hasMember
sosa:hasMember rdf:type owl:ObjectProperty ;
               rdfs:label "hasMember"^^xsd:string .


###  http://www.w3.org/ns/sosa/hasObservation
sosa:hasObservation rdf:type owl:ObjectProperty .


###  http://www.w3.org/ns/sosa/hasResult
sosa:hasResult rdf:type owl:ObjectProperty .


###  http://www.w3.org/ns/sosa/hosts
sosa:hosts rdf:type owl:ObjectProperty .


###  http://www.w3.org/ns/sosa/isFeatureOfInterestOf
sosa:isFeatureOfInterestOf rdf:type owl:ObjectProperty .


###  http://www.w3.org/ns/sosa/madeBySensor
sosa:madeBySensor rdf:type owl:ObjectProperty .


###  http://www.w3.org/ns/sosa/observedProperty
sosa:observedProperty rdf:type owl:ObjectProperty ;
                      rdfs:label "observedProperty"^^xsd:string .


###  http://www.w3.org/ns/sosa/phenomenonTime
sosa:phenomenonTime rdf:type owl:ObjectProperty .


#################################################################
#    Data properties
#################################################################

###  http://gnis-ld.org/lod/gnis/ontology/alternativeName
gnis:alternativeName rdf:type owl:DatatypeProperty .


###  http://gnis-ld.org/lod/gnis/ontology/citation
gnis:citation rdf:type owl:DatatypeProperty ;
              rdfs:label "citation" .


###  http://gnis-ld.org/lod/gnis/ontology/countyCode
gnis:countyCode rdf:type owl:DatatypeProperty ;
                rdfs:label "county code" .


###  http://gnis-ld.org/lod/gnis/ontology/countyId
gnis:countyId rdf:type owl:DatatypeProperty ;
              rdfs:label "county id" .


###  http://gnis-ld.org/lod/gnis/ontology/countyName
gnis:countyName rdf:type owl:DatatypeProperty ;
                rdfs:label "county name" .


###  http://gnis-ld.org/lod/gnis/ontology/dateFeatureCreated
gnis:dateFeatureCreated rdf:type owl:DatatypeProperty ;
                        rdfs:label "date feature created" .


###  http://gnis-ld.org/lod/gnis/ontology/dateFeatureEdited
gnis:dateFeatureEdited rdf:type owl:DatatypeProperty ;
                       rdfs:label "date feature edited" .


###  http://gnis-ld.org/lod/gnis/ontology/dateNameCreated
gnis:dateNameCreated rdf:type owl:DatatypeProperty ;
                     rdfs:label "date name created" .


###  http://gnis-ld.org/lod/gnis/ontology/description
gnis:description rdf:type owl:DatatypeProperty ;
                 rdfs:label "description" .


###  http://gnis-ld.org/lod/gnis/ontology/featureId
gnis:featureId rdf:type owl:DatatypeProperty ;
               rdfs:label "feature id" .


###  http://gnis-ld.org/lod/gnis/ontology/history
gnis:history rdf:type owl:DatatypeProperty ;
             rdfs:label "history" .


###  http://gnis-ld.org/lod/gnis/ontology/mapName
gnis:mapName rdf:type owl:DatatypeProperty ;
             rdfs:label "map name" .


###  http://gnis-ld.org/lod/gnis/ontology/officialName
gnis:officialName rdf:type owl:DatatypeProperty ;
                  rdfs:label "official name" .


###  http://gnis-ld.org/lod/gnis/ontology/stateCode
gnis:stateCode rdf:type owl:DatatypeProperty ;
               rdfs:label "state code" .


###  http://gnis-ld.org/lod/gnis/ontology/stateId
gnis:stateId rdf:type owl:DatatypeProperty ;
             rdfs:label "state id" .


###  http://gnis-ld.org/lod/gnis/ontology/stateName
gnis:stateName rdf:type owl:DatatypeProperty ;
               rdfs:label "state name" .


###  http://ld.iospress.nl/rdf/geocode/country
geocode:country rdf:type owl:DatatypeProperty ;
                rdfs:label "country" .


###  http://qudt.org/2.1/schema/qudt#numericValue
<http://qudt.org/2.1/schema/qudt#numericValue> rdf:type owl:DatatypeProperty .


###  http://qudt.org/2.1/schema/qudt#value
<http://qudt.org/2.1/schema/qudt#value> rdf:type owl:DatatypeProperty .


###  http://stko-kwg.geog.ucsb.edu/lod/ontology/address
kwg-ont:address rdf:type owl:DatatypeProperty ;
                rdfs:label "address" .


###  http://stko-kwg.geog.ucsb.edu/lod/ontology/amountApproved_HA
kwg-ont:amountApproved_HA rdf:type owl:DatatypeProperty ;
                          rdfs:comment "The total amount approved for Housing Assistance from the Individual and Households Program in dollars" ;
                          rdfs:label "amount approved for housing assistance" .


###  http://stko-kwg.geog.ucsb.edu/lod/ontology/amountApproved_IHP
kwg-ont:amountApproved_IHP rdf:type owl:DatatypeProperty ;
                           rdfs:comment "The total amount approved for the Individual and Households Program in dollars" ;
                           rdfs:label "amount approved for individuals and households" .


###  http://stko-kwg.geog.ucsb.edu/lod/ontology/amountApproved_ONA
kwg-ont:amountApproved_ONA rdf:type owl:DatatypeProperty ;
                           rdfs:comment "The total amount approved for Other Needs Assistance from the Individual and Households Program in dollars" ;
                           rdfs:label "amount approved for other needs assistance" .


###  http://stko-kwg.geog.ucsb.edu/lod/ontology/anomaly
kwg-ont:anomaly rdf:type owl:DatatypeProperty ;
                rdfs:comment "Divisional anomaly (1-month period) for the measured climate property" ;
                rdfs:label "anomaly" .


###  http://stko-kwg.geog.ucsb.edu/lod/ontology/cbsaCode
kwg-ont:cbsaCode rdf:type owl:DatatypeProperty ;
                 rdfs:comment "A core-based statistical area is a U.S. geographic area defined by the Office of Management and Budget that consists of one or more counties anchored by an urban center of at least 10,000 people plus adjacent counties that are socioeconomically tied to the urban center by commuting" ;
                 rdfs:label "cbsa code" .


###  http://stko-kwg.geog.ucsb.edu/lod/ontology/cbsaName
kwg-ont:cbsaName rdf:type owl:DatatypeProperty ;
                 rdfs:comment "A core-based statistical area is a U.S. geographic area defined by the Office of Management and Budget that consists of one or more counties anchored by an urban center of at least 10,000 people plus adjacent counties that are socioeconomically tied to the urban center by commuting" ;
                 rdfs:label "cbsa name" .


###  http://stko-kwg.geog.ucsb.edu/lod/ontology/climateDivisionFIPS
kwg-ont:climateDivisionFIPS rdf:type owl:DatatypeProperty ;
                            rdfs:comment "FIPS code for the climate division boundary" ;
                            rdfs:label "climate division FIPS" .


###  http://stko-kwg.geog.ucsb.edu/lod/ontology/climateDivisionNCDC_GEO
kwg-ont:climateDivisionNCDC_GEO rdf:type owl:DatatypeProperty ;
                                rdfs:comment "National Climatic Data Center identifier" ;
                                rdfs:label "climate division NCDC GEO" .


###  http://stko-kwg.geog.ucsb.edu/lod/ontology/climateDivisionName
kwg-ont:climateDivisionName rdf:type owl:DatatypeProperty ;
                            rdfs:comment "Name of climate division boundary" ;
                            rdfs:label "climate division name" .


###  http://stko-kwg.geog.ucsb.edu/lod/ontology/climateDivisionNumber
kwg-ont:climateDivisionNumber rdf:type owl:DatatypeProperty ;
                              rdfs:comment "NOAA climate division number" ;
                              rdfs:label "climate division number" .


###  http://stko-kwg.geog.ucsb.edu/lod/ontology/compositePercentageInformation
kwg-ont:compositePercentageInformation rdf:type owl:DatatypeProperty ;
                                       rdfs:label "composite drought zone percentage information" .


###  http://stko-kwg.geog.ucsb.edu/lod/ontology/correspondingMapID
kwg-ont:correspondingMapID rdf:type owl:DatatypeProperty ;
                           rdfs:label "corresponding map ID" .


###  http://stko-kwg.geog.ucsb.edu/lod/ontology/dailyAQIValue
kwg-ont:dailyAQIValue rdf:type owl:DatatypeProperty ;
                      rdfs:comment "Air Quality Index values for the specified year and location recorded by EPA" ;
                      rdfs:label "daily AQI value" .


###  http://stko-kwg.geog.ucsb.edu/lod/ontology/designatedArea
kwg-ont:designatedArea rdf:type owl:DatatypeProperty ;
                       rdfs:comment "The name or phrase describing the U.S. county that was included in the declaration" ;
                       rdfs:label "designated area" .


###  http://stko-kwg.geog.ucsb.edu/lod/ontology/detailsURL
kwg-ont:detailsURL rdf:type owl:DatatypeProperty .


###  http://stko-kwg.geog.ucsb.edu/lod/ontology/fipsCountyCode
kwg-ont:fipsCountyCode rdf:type owl:DatatypeProperty ;
                       rdfs:label "county FIPS code" .


###  http://stko-kwg.geog.ucsb.edu/lod/ontology/fipsStateCode
kwg-ont:fipsStateCode rdf:type owl:DatatypeProperty ;
                      rdfs:label "state FIPS code" .


###  http://stko-kwg.geog.ucsb.edu/lod/ontology/hasAzimuth
kwg-ont:hasAzimuth rdf:type owl:DatatypeProperty ;
                   rdfs:label "has azimuth" .


###  http://stko-kwg.geog.ucsb.edu/lod/ontology/hasCode
kwg-ont:hasCode rdf:type owl:DatatypeProperty ;
                rdfs:comment "metropolitan and micropolitan statistical area code" ;
                rdfs:label "census area code" ,
                           "has drought intensity code" .


###  http://stko-kwg.geog.ucsb.edu/lod/ontology/hasDeclarationDate
kwg-ont:hasDeclarationDate rdf:type owl:DatatypeProperty ;
                           rdfs:comment "The date a declaration was approved" ;
                           rdfs:label "has declaration date" .


###  http://stko-kwg.geog.ucsb.edu/lod/ontology/hasDeclarationID
kwg-ont:hasDeclarationID rdf:type owl:DatatypeProperty ;
                         rdfs:comment "Unique identifier of each declaration" ;
                         rdfs:label "has declaration ID" .


###  http://stko-kwg.geog.ucsb.edu/lod/ontology/hasDeclarationRequestNo
kwg-ont:hasDeclarationRequestNo rdf:type owl:DatatypeProperty ;
                                rdfs:comment "The identifier of the declaration when it was submitted for approval/request" ;
                                rdfs:label "has declaration request no" .


###  http://stko-kwg.geog.ucsb.edu/lod/ontology/hasDeclarationTitle
kwg-ont:hasDeclarationTitle rdf:type owl:DatatypeProperty ;
                            rdfs:comment "Title of the declaration" ;
                            rdfs:label "has declaration title" .


###  http://stko-kwg.geog.ucsb.edu/lod/ontology/hasDisasterName
kwg-ont:hasDisasterName rdf:type owl:DatatypeProperty ;
                        rdfs:comment "Name of the Disaster that the declaration was submitted or approved for" ;
                        rdfs:label "has disaster name" .


###  http://stko-kwg.geog.ucsb.edu/lod/ontology/hasDisasterNumber
kwg-ont:hasDisasterNumber rdf:type owl:DatatypeProperty ;
                          rdfs:comment "The identifier of each disaster - this is unique to the FEMA declaration dataset. Storm related disaster are related to NOAA Storm dataset. See property kwg-ont:noaaDisasterID" ;
                          rdfs:label "has disaster number" .


###  http://stko-kwg.geog.ucsb.edu/lod/ontology/hasFIPS
kwg-ont:hasFIPS rdf:type owl:DatatypeProperty ;
                rdfs:label "has FIPS" .


###  http://stko-kwg.geog.ucsb.edu/lod/ontology/hasFireName
kwg-ont:hasFireName rdf:type owl:DatatypeProperty ;
                    rdfs:label "has mtbs fire name" .


###  http://stko-kwg.geog.ucsb.edu/lod/ontology/hasGEOID
kwg-ont:hasGEOID rdf:type owl:DatatypeProperty ;
                 rdfs:comment "Refers to the GEOID20 property of zip code data obtained from the census bureau." ;
                 rdfs:label "has GEOID" .


###  http://stko-kwg.geog.ucsb.edu/lod/ontology/hasIncidentName
kwg-ont:hasIncidentName rdf:type owl:DatatypeProperty ;
                        rdfs:label "has incident name" .


###  http://stko-kwg.geog.ucsb.edu/lod/ontology/hasLength
kwg-ont:hasLength rdf:type owl:DatatypeProperty ;
                  rdfs:label "road length" .


###  http://stko-kwg.geog.ucsb.edu/lod/ontology/hasMapUnitAreaSymbol
kwg-ont:hasMapUnitAreaSymbol rdf:type owl:DatatypeProperty ;
                             rdfs:label "has map unit area symbol"^^xsd:string .


###  http://stko-kwg.geog.ucsb.edu/lod/ontology/hasNarrative
kwg-ont:hasNarrative rdf:type owl:DatatypeProperty ;
                     rdfs:label "has hazard narrative" .


###  http://stko-kwg.geog.ucsb.edu/lod/ontology/hasProgramCloseOutDate
kwg-ont:hasProgramCloseOutDate rdf:type owl:DatatypeProperty ;
                               rdfs:comment "The date when the relief program was closed" ;
                               rdfs:label "has program close out date" .


###  http://stko-kwg.geog.ucsb.edu/lod/ontology/hasProgramDescription
kwg-ont:hasProgramDescription rdf:type owl:DatatypeProperty ;
                              rdfs:comment "The description of the relief program" ;
                              rdfs:label "has program description" .


###  http://stko-kwg.geog.ucsb.edu/lod/ontology/hasProgramDesignatedDate
kwg-ont:hasProgramDesignatedDate rdf:type owl:DatatypeProperty ;
                                 rdfs:comment "The date when the relief program began" ;
                                 rdfs:label "has program designated date" .


###  http://stko-kwg.geog.ucsb.edu/lod/ontology/hasProgramID
kwg-ont:hasProgramID rdf:type owl:DatatypeProperty ;
                     rdfs:comment "Unique Identifier of the Program" ;
                     rdfs:label "has program ID" .


###  http://stko-kwg.geog.ucsb.edu/lod/ontology/hasRange
kwg-ont:hasRange rdf:type owl:DatatypeProperty ;
                 rdfs:label "has range" .


###  http://stko-kwg.geog.ucsb.edu/lod/ontology/hasRoadName
kwg-ont:hasRoadName rdf:type owl:DatatypeProperty ;
                    rdfs:label "has road name" .


###  http://stko-kwg.geog.ucsb.edu/lod/ontology/hasRoadSign
kwg-ont:hasRoadSign rdf:type owl:DatatypeProperty ;
                    rdfs:label "has road sign" .


###  http://stko-kwg.geog.ucsb.edu/lod/ontology/hasSoilMapUnitKey
kwg-ont:hasSoilMapUnitKey rdf:type owl:DatatypeProperty ;
                          rdfs:label "has soil map unit key"^^xsd:string .


###  http://stko-kwg.geog.ucsb.edu/lod/ontology/hasSoilMapUnitSymbol
kwg-ont:hasSoilMapUnitSymbol rdf:type owl:DatatypeProperty ;
                             rdfs:label "has soil map unit symbol"^^xsd:string .


###  http://stko-kwg.geog.ucsb.edu/lod/ontology/hasTraumaDefinition
kwg-ont:hasTraumaDefinition rdf:type owl:DatatypeProperty ;
                            rdfs:label "has trauma definition" .


###  http://stko-kwg.geog.ucsb.edu/lod/ontology/hasZipCode
kwg-ont:hasZipCode rdf:type owl:DatatypeProperty ;
                   rdfs:label "has zip code" .


###  http://stko-kwg.geog.ucsb.edu/lod/ontology/hospitalAddress
kwg-ont:hospitalAddress rdf:type owl:DatatypeProperty .


###  http://stko-kwg.geog.ucsb.edu/lod/ontology/hospitalName
kwg-ont:hospitalName rdf:type owl:DatatypeProperty ;
                     rdfs:label "hospital name" .


###  http://stko-kwg.geog.ucsb.edu/lod/ontology/isHMProgramDeclared
kwg-ont:isHMProgramDeclared rdf:type owl:DatatypeProperty ;
                            rdfs:comment "Denotes whether the Hazard Mitigation program was declared" ;
                            rdfs:label "is hazard mitigation program declared" .


###  http://stko-kwg.geog.ucsb.edu/lod/ontology/isIAProgramDeclared
kwg-ont:isIAProgramDeclared rdf:type owl:DatatypeProperty ;
                            rdfs:comment "Denotes whether the Individual Assistance program was declared" ;
                            rdfs:label "is individual assistance program declared" .


###  http://stko-kwg.geog.ucsb.edu/lod/ontology/isIHProgramDeclared
kwg-ont:isIHProgramDeclared rdf:type owl:DatatypeProperty ;
                            rdfs:comment "Denotes whether the Individuals and Households program was declared" ;
                            rdfs:label "is individual and households program declared" .


###  http://stko-kwg.geog.ucsb.edu/lod/ontology/isPAProgramDeclared
kwg-ont:isPAProgramDeclared rdf:type owl:DatatypeProperty ;
                            rdfs:comment "Denotes whether the Public Assistance program was declared" ;
                            rdfs:label "is public assistance program declared" .


###  http://stko-kwg.geog.ucsb.edu/lod/ontology/nielsenMarketZoneDMA
kwg-ont:nielsenMarketZoneDMA rdf:type owl:DatatypeProperty ;
                             rdfs:label "nielsen market zone DMA" .


###  http://stko-kwg.geog.ucsb.edu/lod/ontology/nielsenMarketZoneHHTV
kwg-ont:nielsenMarketZoneHHTV rdf:type owl:DatatypeProperty ;
                              rdfs:label "nielsen market zone HHTV" .


###  http://stko-kwg.geog.ucsb.edu/lod/ontology/nielsenMarketZoneID
kwg-ont:nielsenMarketZoneID rdf:type owl:DatatypeProperty ;
                            rdfs:label "nielsen market zone ID" .


###  http://stko-kwg.geog.ucsb.edu/lod/ontology/nielsenMarketZonePUSA
kwg-ont:nielsenMarketZonePUSA rdf:type owl:DatatypeProperty ;
                              rdfs:label "nielsen market zone PUSA" .


###  http://stko-kwg.geog.ucsb.edu/lod/ontology/nielsenMarketZoneRank
kwg-ont:nielsenMarketZoneRank rdf:type owl:DatatypeProperty ;
                              rdfs:label "nielsen market zone rank" .


###  http://stko-kwg.geog.ucsb.edu/lod/ontology/noHospitalBeds
kwg-ont:noHospitalBeds rdf:type owl:DatatypeProperty ;
                       rdfs:label "no of hospital beds" .


###  http://stko-kwg.geog.ucsb.edu/lod/ontology/noaaDisasterID
kwg-ont:noaaDisasterID rdf:type owl:DatatypeProperty ;
                       rdfs:comment "Disaster ID from NOAA Storm Event dataset" ;
                       rdfs:label "noaa disaster impact ID" .


###  http://stko-kwg.geog.ucsb.edu/lod/ontology/obligatedAmountCat_AB
kwg-ont:obligatedAmountCat_AB rdf:type owl:DatatypeProperty ;
                              rdfs:comment "The Public Assistance grant funding available in dollars to the grantee (State), for sub-grantee approved Project Worksheets in categories A and B, or Emergency Work. Category A: Debris removal; Category B: Emergency protective measures" ;
                              rdfs:label "obligated amount category AB" .


###  http://stko-kwg.geog.ucsb.edu/lod/ontology/obligatedAmountCat_C_G
kwg-ont:obligatedAmountCat_C_G rdf:type owl:DatatypeProperty ;
                               rdfs:comment "The Public Assistance grant funding available in dollars to the grantee (State), for sub-grantee approved Project Worksheets in categories C through G, or Permanent Work. Category C: Roads and bridges; Category D: Water control facilities; Category E: Public buildings and contents; Category F: Public utilities; Category G: Parks, recreational, and other facilities" ;
                               rdfs:label "obligated amount category C-G" .


###  http://stko-kwg.geog.ucsb.edu/lod/ontology/obligatedAmount_HMGP
kwg-ont:obligatedAmount_HMGP rdf:type owl:DatatypeProperty ;
                             rdfs:comment "Total amount obligated under the Hazard Mitigation Grant Program in dollars. The total amount obligated represents the amount obligated for Regular Project Costs, Planning Costs, Initiative Project Costs, Recipient Management Costs, Recipient Admin Costs and Subrecipient Admin Costs" ;
                             rdfs:label "obligated amount hazard mitigation program" .


###  http://stko-kwg.geog.ucsb.edu/lod/ontology/obligatedAmount_PA
kwg-ont:obligatedAmount_PA rdf:type owl:DatatypeProperty ;
                           rdfs:comment "The Public Assistance grant funding available in dollars to the grantee (State), for sub-grantee approved Project Worksheets" ;
                           rdfs:label "obligated amount public assistance" .


###  http://stko-kwg.geog.ucsb.edu/lod/ontology/pharmacyName
kwg-ont:pharmacyName rdf:type owl:DatatypeProperty ;
                     rdfs:label "pharmacy name" .


###  http://stko-kwg.geog.ucsb.edu/lod/ontology/pocValue
kwg-ont:pocValue rdf:type owl:DatatypeProperty ;
                 rdfs:comment "EPA Air Quality Instrument ID" ;
                 rdfs:label "poc value" .


###  http://stko-kwg.geog.ucsb.edu/lod/ontology/publicHealthDepartmentName
kwg-ont:publicHealthDepartmentName rdf:type owl:DatatypeProperty ;
                                   rdfs:label "public health department name" .


###  http://stko-kwg.geog.ucsb.edu/lod/ontology/rank
kwg-ont:rank rdf:type owl:DatatypeProperty ;
             rdfs:comment "Dvisional rank (1-month period)for the measured climate property" ;
             rdfs:label "rank" .


###  http://stko-kwg.geog.ucsb.edu/lod/ontology/siteID
kwg-ont:siteID rdf:type owl:DatatypeProperty ;
               rdfs:comment "EPA Air Quality Sensor ID" ;
               rdfs:label "site ID" .


###  http://stko-kwg.geog.ucsb.edu/lod/ontology/siteName
kwg-ont:siteName rdf:type owl:DatatypeProperty ;
                 rdfs:comment "EPA Air Quality Sensor Name" ;
                 rdfs:label "site name" .


###  http://stko-kwg.geog.ucsb.edu/lod/ontology/telephoneNo
kwg-ont:telephoneNo rdf:type owl:DatatypeProperty ;
                    rdfs:label "telephone no" .


###  http://stko-kwg.geog.ucsb.edu/lod/ontology/totalNumberApproved_IA
kwg-ont:totalNumberApproved_IA rdf:type owl:DatatypeProperty ;
                               rdfs:comment "The number of disaster assistance applications that were approved for Individual Assistance" ;
                               rdfs:label "total number approved individual assistance" .


###  http://stko-kwg.geog.ucsb.edu/lod/ontology/traumaDescriptionForState
kwg-ont:traumaDescriptionForState rdf:type owl:DatatypeProperty ;
                                  rdfs:label "trauma description for state" .


###  http://stko-kwg.geog.ucsb.edu/lod/ontology/traumaDescriptionSource
kwg-ont:traumaDescriptionSource rdf:type owl:DatatypeProperty ;
                                rdfs:label "trauma description source" .


###  http://stko-kwg.geog.ucsb.edu/lod/ontology/website
kwg-ont:website rdf:type owl:DatatypeProperty ;
                rdfs:label "website" .


###  http://stko-kwg.geog.ucsb.edu/lod/ontology/zipCode
kwg-ont:zipCode rdf:type owl:DatatypeProperty ;
                rdfs:label "zip code" .


###  http://stko-kwg.geog.ucsb.edu/lod/ontology/zoneNumber
kwg-ont:zoneNumber rdf:type owl:DatatypeProperty ;
                   rdfs:comment "NOAA national weather zone number from https://www.nws.noaa.gov/directives/sym/pd01005007curr.pdf" ;
                   rdfs:label "zone number" .


###  http://www.opengis.net/ont/geosparql#asWKT
<http://www.opengis.net/ont/geosparql#asWKT> rdf:type owl:DatatypeProperty ;
                                             rdfs:subPropertyOf <http://www.opengis.net/ont/geosparql#hasSerialization> ;
                                             rdfs:isDefinedBy <http://www.opengis.net/ont/geosparql#> ;
                                             skos:definition "The WKT serialization of a Geometry"@en ;
                                             skos:prefLabel "as WKT"@en .


###  http://stko-kwg.geog.ucsb.edu/lod/ontology/hasName
kwg-ont:hasName rdf:type owl:DatatypeProperty ;
                                               rdfs:label "has federal judicial district name" .


###  http://www.opengis.net/ont/geosparql#hasSerialization
<http://www.opengis.net/ont/geosparql#hasSerialization> rdf:type owl:DatatypeProperty ;
                                                        rdfs:isDefinedBy <http://www.opengis.net/ont/geosparql#> ;
                                                        skos:definition "Connects a Geometry object with its text-based serialization."@en ;
                                                        skos:prefLabel "has serialization"@en .


###  http://www.w3.org/2003/01/geo/wgs84_pos#asWKT
wgs84_pos:asWKT rdf:type owl:DatatypeProperty .


###  http://www.w3.org/2006/time#hasXSDDuration
time:hasXSDDuration rdf:type owl:DatatypeProperty ;
                    rdfs:comment "Extent of a temporal entity, expressed using xsd:duration"@en ;
                    rdfs:label "has XSD duration"@en ;
                    skos:definition "Extent of a temporal entity, expressed using xsd:duration"@en ;
                    skos:editorialNote "Feature at risk - added in 2017 revision, and not yet widely used. "@en .


###  http://www.w3.org/2006/time#inXSDDate
time:inXSDDate rdf:type owl:DatatypeProperty ;
               rdfs:label "in XSD date"@en ;
               skos:definition "Position of an instant, expressed using xsd:date"@en .


###  http://www.w3.org/2006/time#inXSDDateTime
time:inXSDDateTime rdf:type owl:DatatypeProperty .


###  http://www.w3.org/2006/time#inXSDDateTimeStamp
time:inXSDDateTimeStamp rdf:type owl:DatatypeProperty ;
                        rdfs:label "in XSD Date-Time-Stamp"@en ;
                        skos:definition "Position of an instant, expressed using xsd:dateTimeStamp"@en .


###  http://www.w3.org/2006/time#inXSDgYear
time:inXSDgYear rdf:type owl:DatatypeProperty ;
                rdfs:label "in XSD g-Year"@en ;
                skos:definition "Position of an instant, expressed using xsd:gYear"@en .


###  http://www.w3.org/2006/time#months
time:months rdf:type owl:DatatypeProperty .


###  http://www.w3.org/ns/sosa/hasABBR
sosa:hasABBR rdf:type owl:DatatypeProperty ;
             rdfs:label "has abbreviation" .


###  http://www.w3.org/ns/sosa/hasSimpleResult
sosa:hasSimpleResult rdf:type owl:DatatypeProperty ;
                     rdfs:label "hasSimpleResult"^^xsd:string .


###  http://www.w3.org/ns/sosa/resultTime
sosa:resultTime rdf:type owl:DatatypeProperty .


#################################################################
#    Classes
#################################################################

###  http://gnis-ld.org/lod/gnis/ontology/County
gnis:County rdf:type owl:Class ;
            rdfs:subClassOf usgs:Division ;
            rdfs:comment "Second-order division of a nation such as parish, borough, county, municipio, or judicial division, and independent cities in Maryland, Missouri, Nevada, and Virginia."@en ,
                         "Source - https://gnis-ld.org/" ;
            rdfs:label "County"@en .


###  http://gnis-ld.org/lod/gnis/ontology/State
gnis:State rdf:type owl:Class ;
           rdfs:subClassOf usgs:Division ;
           rdfs:comment "First-order division of a nation."@en ,
                        "Source - https://gnis-ld.org/" ;
           rdfs:label "State"@en .


###  http://gnis-ld.org/lod/usgs/ontology/Airport
usgs:Airport rdf:type owl:Class ;
             rdfs:subClassOf usgs:BuiltUpArea ;
             rdfs:comment "A facility, on land, where aircraft can take off and land; usually consists of hard-surfaced landing strips, a control tower, hangars, and accommodations for passengers and cargo"@en ;
             rdfs:label "Airport"@en .


###  http://gnis-ld.org/lod/usgs/ontology/Arch
usgs:Arch rdf:type owl:Class ;
          rdfs:subClassOf usgs:BuiltUpArea ,
                          usgs:Terrain ;
          rdfs:comment "A curved structure that supports the weight of material over an open space"@en ,
                       "A naturally occuring, freestanding curved structure that spans an opening"^^xsd:string ;
          rdfs:label "Arch"@en .


###  http://gnis-ld.org/lod/usgs/ontology/Area
usgs:Area rdf:type owl:Class ;
          rdfs:label "Area"@en ,
                     "Source - https://gnis-ld.org/" .


###  http://gnis-ld.org/lod/usgs/ontology/Arroyo
usgs:Arroyo rdf:type owl:Class ;
            rdfs:subClassOf usgs:SurfaceWater ;
            rdfs:comment "Watercourse or channel through which water may occasionally flow (coulee, draw, gully, wash)"@en ;
            rdfs:label "Arroyo"@en .


###  http://gnis-ld.org/lod/usgs/ontology/Bar
usgs:Bar rdf:type owl:Class ;
         rdfs:subClassOf usgs:BuiltUpArea ,
                         usgs:Terrain ;
         rdfs:comment "A natural accumulation of sand, gravel, or other material forming an underwater or exposed embankment"@en ,
                      "A submerged or emerged mound, ridge, or succession of ridges of sand or other material extending across the bottom,and which may obstruct navigation"@en ;
         rdfs:label "Bar"@en .


###  http://gnis-ld.org/lod/usgs/ontology/Basin
usgs:Basin rdf:type owl:Class ;
           rdfs:subClassOf usgs:SurfaceWater ,
                           usgs:Terrain ;
           rdfs:comment "A bowl-shaped depression in the surface of the land or ocean floor"@en ;
           rdfs:label "Basin"@en .


###  http://gnis-ld.org/lod/usgs/ontology/Bay
usgs:Bay rdf:type owl:Class ;
         rdfs:subClassOf usgs:SurfaceWater ;
         rdfs:comment " water area that is an opening of the sea or ocean into the land, or of an estuary, lake, or river into its shore"@en ;
         rdfs:label "Bay"@en .


###  http://gnis-ld.org/lod/usgs/ontology/Beach
usgs:Beach rdf:type owl:Class ;
           rdfs:subClassOf usgs:SurfaceWater ,
                           usgs:Terrain ;
           rdfs:comment "A gently sloping shore which is washed by waves or tides, especially the parts covered by sand or pebbles"@en ;
           rdfs:label "Beach"@en .


###  http://gnis-ld.org/lod/usgs/ontology/Bench
usgs:Bench rdf:type owl:Class ;
           rdfs:subClassOf usgs:Terrain ;
           rdfs:comment "An area of relatively level land on the flank of an elevation such as a hill, ridge, or mountain where the slope of the land rises on one side and descends on the opposite side (level)"@en ;
           rdfs:label "Bench"@en .


###  http://gnis-ld.org/lod/usgs/ontology/Bend
usgs:Bend rdf:type owl:Class ;
          rdfs:subClassOf usgs:SurfaceWater ;
          rdfs:comment "A curve in the course of a stream or the land within the curve"@en ;
          rdfs:label "Bend"@en .


###  http://gnis-ld.org/lod/usgs/ontology/Bridge
usgs:Bridge rdf:type owl:Class ;
            rdfs:subClassOf usgs:BuiltUpArea ;
            rdfs:comment "A structure erected over a depression or obstacle to carry traffic or some facility such as a pipeline"@en ;
            rdfs:label "Bridge"@en .


###  http://gnis-ld.org/lod/usgs/ontology/Building
usgs:Building rdf:type owl:Class ;
              rdfs:subClassOf usgs:BuiltUpArea ;
              rdfs:comment "A permanent walled and roofed construction"@en ;
              rdfs:label "Building"@en .


###  http://gnis-ld.org/lod/usgs/ontology/BuiltUpArea
usgs:BuiltUpArea rdf:type owl:Class ;
                 rdfs:subClassOf <http://www.opengis.net/ont/geosparql#SpatialObject> ;
                 rdfs:comment "An area of intensive use, with much of the land covered by structures"@en ;
                 rdfs:label "Built Up Area"@en .


###  http://gnis-ld.org/lod/usgs/ontology/Canal
usgs:Canal rdf:type owl:Class ;
           rdfs:subClassOf usgs:BuiltUpArea ,
                           usgs:SurfaceWater ;
           rdfs:comment "Manmade waterway used by watercraft or for drainage, irrigation, mining, or water power"@en ;
           rdfs:label "Canal"@en .


###  http://gnis-ld.org/lod/usgs/ontology/Cape
usgs:Cape rdf:type owl:Class ;
          rdfs:subClassOf usgs:Terrain ;
          rdfs:comment "A relatively extensive land area jutting into a water body, which prominently marks a change in or interrupts notably the coastal trend of that water body"@en ;
          rdfs:label "Cape"@en .


###  http://gnis-ld.org/lod/usgs/ontology/Cemetery
usgs:Cemetery rdf:type owl:Class ;
              rdfs:subClassOf usgs:BuiltUpArea ;
              rdfs:comment "A place for burying the dead"@en ;
              rdfs:label "Cemetery"@en .


###  http://gnis-ld.org/lod/usgs/ontology/Census
usgs:Census rdf:type owl:Class ;
            rdfs:subClassOf usgs:Division ;
            rdfs:comment "A statistical area delineated locally specifically for the tabulation of Census Bureau data"@en ,
                         "Source - https://gnis-ld.org/" ;
            rdfs:label "Census"@en .


###  http://gnis-ld.org/lod/usgs/ontology/Channel
usgs:Channel rdf:type owl:Class ;
             rdfs:subClassOf usgs:SurfaceWater ;
             rdfs:comment "Linear deep part of a body of water through which the main volume of water flows and is frequently used as aroute for watercraft (passage, reach, strait, thoroughfare, throughfare)"@en ;
             rdfs:label "Channel"@en .


###  http://gnis-ld.org/lod/usgs/ontology/Church
usgs:Church rdf:type owl:Class ;
            rdfs:subClassOf usgs:BuiltUpArea ;
            rdfs:comment "Building used for religious worship (chapel, mosque, synagogue, tabernacle, temple)."@en ;
            rdfs:label "Church"@en .


###  http://gnis-ld.org/lod/usgs/ontology/CivilGovernment
usgs:CivilGovernment rdf:type owl:Class ;
                     rdfs:label "Civil Government"@en ,
                                "Source - https://gnis-ld.org/" .


###  http://gnis-ld.org/lod/usgs/ontology/Cliff
usgs:Cliff rdf:type owl:Class ;
           rdfs:subClassOf usgs:Terrain ;
           rdfs:comment "Very steep or vertical slope"@en ;
           rdfs:label "Cliff"@en .


###  http://gnis-ld.org/lod/usgs/ontology/Crater
usgs:Crater rdf:type owl:Class ;
            rdfs:subClassOf usgs:Basin ,
                            usgs:Terrain ;
            rdfs:comment "Circular-shaped depression at the summit of a volcanic cone or one on the surface of the land caused by the impact of a meteorite; a manmade depression caused by an explosion"@en ;
            rdfs:label "Crater"@en .


###  http://gnis-ld.org/lod/usgs/ontology/Crossing
usgs:Crossing rdf:type owl:Class ;
              rdfs:subClassOf usgs:BuiltUpArea ;
              rdfs:comment "A place where two or more routes of transportation form a junction or intersection"@en ;
              rdfs:label "Crossing"@en .


###  http://gnis-ld.org/lod/usgs/ontology/Dam
usgs:Dam rdf:type owl:Class ;
         rdfs:subClassOf usgs:BuiltUpArea ,
                         usgs:SurfaceWater ;
         rdfs:comment "Water barrier or embankment built across the course of a stream or into a body of water to control and (or) impound the flow of water"@en ;
         rdfs:label "Dam"@en .


###  http://gnis-ld.org/lod/usgs/ontology/Division
usgs:Division rdf:type owl:Class ;
              rdfs:comment "Source - https://gnis-ld.org/" ;
              rdfs:label "Division" .


###  http://gnis-ld.org/lod/usgs/ontology/EcologicalRegime
usgs:EcologicalRegime rdf:type owl:Class ;
                      rdfs:comment "Source - https://gnis-ld.org/" ;
                      rdfs:label "Ecological Regime" .


###  http://gnis-ld.org/lod/usgs/ontology/Embankment
usgs:Embankment rdf:type owl:Class ;
                rdfs:comment "Source - https://gnis-ld.org/" ;
                rdfs:label "Embankment" .


###  http://gnis-ld.org/lod/usgs/ontology/Feature
usgs:Feature rdf:type owl:Class ;
             rdfs:label "USGS Feature" .


###  http://gnis-ld.org/lod/usgs/ontology/Flat
usgs:Flat rdf:type owl:Class ;
          rdfs:subClassOf usgs:Terrain ;
          rdfs:comment "A level tract lying at a small depth below the surface of water, or alternately covered and left bare by the tide"@en ;
          rdfs:label "Flat"@en .


###  http://gnis-ld.org/lod/usgs/ontology/Forest
usgs:Forest rdf:type owl:Class ;
            rdfs:subClassOf usgs:EcologicalRegime ;
            rdfs:comment "and with a tree-crown areal density (crown closure percentage) of 10 percent or more, are stocked with trees capable of producing timber or other wood products, and exert an influence on the climate or water regime"@en ;
            rdfs:label "Forest"@en ,
                       "Source - https://gnis-ld.org/" .


###  http://gnis-ld.org/lod/usgs/ontology/Gap
usgs:Gap rdf:type owl:Class ;
         rdfs:subClassOf usgs:Terrain ;
         rdfs:comment "A low point or opening between mounts or in a ridge"@en ;
         rdfs:label "Gap"@en .


###  http://gnis-ld.org/lod/usgs/ontology/Glacier
usgs:Glacier rdf:type owl:Class ;
             rdfs:subClassOf usgs:SurfaceWater ;
             rdfs:comment "Body or stream of ice moving outward and downslope from an area of accumulation; an area of relatively permanent snow or ice on the top or side of a mountain or mountainous area"@en ;
             rdfs:label "Glacier"@en .


###  http://gnis-ld.org/lod/usgs/ontology/Gut
usgs:Gut rdf:type owl:Class ;
         rdfs:subClassOf usgs:SurfaceWater ;
         rdfs:comment "A narrow natural passage or contracte strait connecting two bodies of water where no flow can be determined."@en ;
         rdfs:label "Gut"@en .


###  http://gnis-ld.org/lod/usgs/ontology/Harbor
usgs:Harbor rdf:type owl:Class ;
            rdfs:subClassOf usgs:BuiltUpArea ;
            rdfs:comment "An area of water where ships, planes or other watercraft can anchor or dock"@en ;
            rdfs:label "Harbor"@en .


###  http://gnis-ld.org/lod/usgs/ontology/Hospital
usgs:Hospital rdf:type owl:Class ;
              rdfs:subClassOf usgs:BuiltUpArea ,
                              [ rdf:type owl:Restriction ;
                                owl:onProperty kwg-ont:sfWithin ;
                                owl:someValuesFrom kwg-ont:AdministrativeRegion
                              ] ,
                              [ rdf:type owl:Restriction ;
                                owl:onProperty kwg-ont:sfWithin ;
                                owl:someValuesFrom kwg-ont:S2Cell
                              ] ;
              rdfs:comment "Building where the sick or injured may receive medical or surgical attention"@en ;
              rdfs:label "GNIS Hospital"@en .


###  http://gnis-ld.org/lod/usgs/ontology/Island
usgs:Island rdf:type owl:Class ;
            rdfs:subClassOf usgs:Terrain ;
            rdfs:comment "An area of dry or relatively dry land surrounded by water or low wet land"@en ;
            rdfs:label "Island"@en .


###  http://gnis-ld.org/lod/usgs/ontology/Isthmus
usgs:Isthmus rdf:type owl:Class ;
             rdfs:subClassOf usgs:Terrain ;
             rdfs:comment "A narrow strip of land, bordered on both sides by water, connecting two larger land areas"@en ;
             rdfs:label "Isthmus"@en .


###  http://gnis-ld.org/lod/usgs/ontology/Lake
usgs:Lake rdf:type owl:Class ;
          rdfs:subClassOf usgs:SurfaceWater ;
          rdfs:comment "A standing body of water with a predominantly natural shoreliine surrounded by land"@en ;
          rdfs:label "Lake"@en .


###  http://gnis-ld.org/lod/usgs/ontology/Lava
usgs:Lava rdf:type owl:Class ;
          rdfs:subClassOf usgs:Terrain ;
          rdfs:comment "Formations resulting from the consolidation of molten rock on the surface of the Earth"@en ;
          rdfs:label "Lava"@en .


###  http://gnis-ld.org/lod/usgs/ontology/Levee
usgs:Levee rdf:type owl:Class ;
           rdfs:subClassOf usgs:Embankment ;
           rdfs:comment "Natural or manmade embankment flanking alongside a stream"@en ,
                        "Source - https://gnis-ld.org/" ;
           rdfs:label "Levee"@en .


###  http://gnis-ld.org/lod/usgs/ontology/Locale
usgs:Locale rdf:type owl:Class ;
            rdfs:subClassOf usgs:Division ;
            rdfs:comment "A named place not otherwise categorized."@en ,
                         "Source - https://gnis-ld.org/" ;
            rdfs:label "Locale"@en .


###  http://gnis-ld.org/lod/usgs/ontology/Military
usgs:Military rdf:type owl:Class ;
              rdfs:label "Military"@en .


###  http://gnis-ld.org/lod/usgs/ontology/Mine
usgs:Mine rdf:type owl:Class ;
          rdfs:subClassOf usgs:BuiltUpArea ;
          rdfs:comment "An excavation in the earth for the purpose of extracting earth materials"@en ;
          rdfs:label "Mine"@en .


###  http://gnis-ld.org/lod/usgs/ontology/MountainRange
usgs:MountainRange rdf:type owl:Class ;
                   rdfs:subClassOf usgs:Terrain ;
                   rdfs:comment "A series of connected and aligned mountains or mountain ridges"@en ;
                   rdfs:label "Mountain Range"@en .


###  http://gnis-ld.org/lod/usgs/ontology/Ocean
usgs:Ocean rdf:type owl:Class ;
           rdfs:label "Ocean" .


###  http://gnis-ld.org/lod/usgs/ontology/OilField
usgs:OilField rdf:type owl:Class ;
              rdfs:subClassOf usgs:BuiltUpArea ;
              rdfs:comment "An area where petroleum is or was removed from the Earth"@en ;
              rdfs:label "Oil Field"@en .


###  http://gnis-ld.org/lod/usgs/ontology/Park
usgs:Park rdf:type owl:Class ;
          rdfs:subClassOf usgs:BuiltUpArea ;
          rdfs:comment "A place or area developed for public use, recreation, or preservation of a cultural or natural resource."@en ;
          rdfs:label "Park"@en .


###  http://gnis-ld.org/lod/usgs/ontology/Plain
usgs:Plain rdf:type owl:Class ;
           rdfs:subClassOf usgs:Terrain ;
           rdfs:comment "A structure built out into the water, usually with its greatest dimension at right angles to the shore, forming a landing place or a place alongside which vessels can lie."@en ;
           rdfs:label "Plain"@en .


###  http://gnis-ld.org/lod/usgs/ontology/PopulatedPlace
usgs:PopulatedPlace rdf:type owl:Class ;
                    rdfs:subClassOf usgs:BuiltUpArea ;
                    rdfs:comment "Place or area with clustered or scattered buildings and a permanent human population (city, settlement, town, village). A populated place is usually not incorporated and by definition has no legal boundaries. However, a populated place may have a corresponding \"civil\" record, the legal boundaries of which may or may not coincide with the perceived populated place. Distinct from Census and Civil classes."@en ;
                    rdfs:label "Populated Place"@en .


###  http://gnis-ld.org/lod/usgs/ontology/PostOffice
usgs:PostOffice rdf:type owl:Class ;
                rdfs:subClassOf usgs:BuiltUpArea ;
                rdfs:comment "An official facility of the U.S. Postal Service used for processing and distributing mail and other postal material."@en ;
                rdfs:label "Post Office"@en .


###  http://gnis-ld.org/lod/usgs/ontology/Rapids
usgs:Rapids rdf:type owl:Class ;
            rdfs:subClassOf usgs:SurfaceWater ;
            rdfs:comment "An area of broken, fast flowing water in a stream, where the slope of the bed increases (but without a prominent break of slope which might result in a waterfall), or where a gently dipping bar of harder rock outcrops."@en ;
            rdfs:label "Rapids"@en .


###  http://gnis-ld.org/lod/usgs/ontology/Reserve
usgs:Reserve rdf:type owl:Class ;
             rdfs:subClassOf usgs:Division ;
             rdfs:comment "A tract of land set aside for a specific use (does not include forests, civil divisions, parks)."@en ,
                          "Source - https://gnis-ld.org/" ;
             rdfs:label "Reserve"@en .


###  http://gnis-ld.org/lod/usgs/ontology/Reservoir
usgs:Reservoir rdf:type owl:Class ;
               rdfs:subClassOf usgs:SurfaceWater ;
               rdfs:comment "A constructed basin formed to contain water or other liquids."@en ;
               rdfs:label "Reservoir"@en .


###  http://gnis-ld.org/lod/usgs/ontology/Ridge
usgs:Ridge rdf:type owl:Class ;
           rdfs:subClassOf usgs:Terrain ;
           rdfs:comment "A long and narrow upland with steep sides; Elevation with a narrow, elongated crest which can be part of a hill or mountain (crest, cuesta, escarpment, hogback, lae, rim, spur)."@en ;
           rdfs:label "Ridge"@en .


###  http://gnis-ld.org/lod/usgs/ontology/Rock
usgs:Rock rdf:type owl:Class ;
          rdfs:subClassOf usgs:Terrain ;
          rdfs:comment "An isolated concreted mass of stony material or a single large stone, usually one constituting a danger to navigation. It may be always submerged, always uncovered, or alternately covered and uncovered by the tide."@en ;
          rdfs:label "Rock"@en .


###  http://gnis-ld.org/lod/usgs/ontology/School
usgs:School rdf:type owl:Class ;
            rdfs:subClassOf usgs:BuiltUpArea ;
            rdfs:comment "Building or group of buildings used as an institution for study, teaching, and learning."@en ;
            rdfs:label "School"@en .


###  http://gnis-ld.org/lod/usgs/ontology/Sea
usgs:Sea rdf:type owl:Class ;
         rdfs:subClassOf usgs:Ocean ;
         rdfs:comment "A body of salt water usaly surrounded by land but often connected to the Ocean"@en ;
         rdfs:label "Sea"@en .


###  http://gnis-ld.org/lod/usgs/ontology/Slope
usgs:Slope rdf:type owl:Class ;
           rdfs:subClassOf usgs:Terrain ;
           rdfs:comment "A gently inclined part of the Earth's surface (grade, pitch)."@en ;
           rdfs:label "Slope"@en .


###  http://gnis-ld.org/lod/usgs/ontology/Spring
usgs:Spring rdf:type owl:Class ;
            rdfs:subClassOf usgs:SurfaceWater ;
            rdfs:comment "A place where water issues from the ground naturally"@en ;
            rdfs:label "Spring"@en .


###  http://gnis-ld.org/lod/usgs/ontology/Stream
usgs:Stream rdf:type owl:Class ;
            rdfs:subClassOf usgs:SurfaceWater ;
            rdfs:comment "Linear body of water flowing on the Earth's surface."@en ;
            rdfs:label "Stream"@en .


###  http://gnis-ld.org/lod/usgs/ontology/Summit
usgs:Summit rdf:type owl:Class ;
            rdfs:subClassOf usgs:Terrain ;
            rdfs:comment "Prominent elevation rising above the surrounding level of the Earth's surface."@en ;
            rdfs:label "Summit"@en .


###  http://gnis-ld.org/lod/usgs/ontology/SurfaceWater
usgs:SurfaceWater rdf:type owl:Class ;
                  rdfs:subClassOf <http://www.opengis.net/ont/geosparql#SpatialObject> ;
                  rdfs:label "Surface Water"@en .


###  http://gnis-ld.org/lod/usgs/ontology/Swamp
usgs:Swamp rdf:type owl:Class ;
           rdfs:subClassOf usgs:SurfaceWater ;
           rdfs:comment "Poorly drained wetland, fresh or saltwater, wooded or grassy, possibly covered with open water."@en ;
           rdfs:label "Swamp"@en .


###  http://gnis-ld.org/lod/usgs/ontology/Terrain
usgs:Terrain rdf:type owl:Class ;
             rdfs:subClassOf <http://www.opengis.net/ont/geosparql#SpatialObject> ;
             rdfs:label "Terrain"@en .


###  http://gnis-ld.org/lod/usgs/ontology/Tower
usgs:Tower rdf:type owl:Class ;
           rdfs:subClassOf usgs:BuiltUpArea ;
           rdfs:comment "A tall framework or structure, the height of which is required by its function; generally used for observation, storage, or electronic transmission."@en ;
           rdfs:label "Tower"@en .


###  http://gnis-ld.org/lod/usgs/ontology/Trail
usgs:Trail rdf:type owl:Class ;
           rdfs:subClassOf usgs:BuiltUpArea ;
           rdfs:comment "A cleared path, beaten track, or improved surface, as through woods or wilderness, not usually trafficed by vehicles because of width, seasonal conditions, or access restrictions."@en ;
           rdfs:label "Trail"@en .


###  http://gnis-ld.org/lod/usgs/ontology/Tunnel
usgs:Tunnel rdf:type owl:Class ;
            rdfs:subClassOf usgs:BuiltUpArea ;
            rdfs:comment "An underground or underwater passage."@en ;
            rdfs:label "Tunnel"@en .


###  http://gnis-ld.org/lod/usgs/ontology/Unknown
usgs:Unknown rdf:type owl:Class ;
             rdfs:comment "Unknown feature type"@en ;
             rdfs:label "Unknown"@en .


###  http://gnis-ld.org/lod/usgs/ontology/Valley
usgs:Valley rdf:type owl:Class ;
            rdfs:subClassOf usgs:Terrain ;
            rdfs:comment "An elongated depression in the earth's surface which generally slopes from one end to the other."@en ;
            rdfs:label "Valley"@en .


###  http://gnis-ld.org/lod/usgs/ontology/Waterfall
usgs:Waterfall rdf:type owl:Class ;
               rdfs:subClassOf usgs:SurfaceWater ;
               rdfs:comment "A vertical or near vertical descent of water over a step or ledge in the bed of a river."@en ;
               rdfs:label "Waterfall"@en .


###  http://gnis-ld.org/lod/usgs/ontology/Well
usgs:Well rdf:type owl:Class ;
          rdfs:subClassOf usgs:BuiltUpArea ;
          rdfs:comment "A pit or hole dug or bored into the earth for the extraction of oil, water, other fluids, or gases."@en ;
          rdfs:label "Well"@en .


###  http://gnis-ld.org/lod/usgs/ontology/Woodland
usgs:Woodland rdf:type owl:Class ;
              rdfs:subClassOf usgs:Forest ;
              rdfs:comment "Land having a cover of trees, shrubs, or both."@en ,
                           "Source - https://gnis-ld.org/" ;
              rdfs:label "Woodland"@en .


###  http://qudt.org/2.1/schema/qudt#Quantity
<http://qudt.org/2.1/schema/qudt#Quantity> rdf:type owl:Class ;
                                           rdfs:label "Quantity" .


###  http://qudt.org/2.1/schema/qudt#QuantityValue
<http://qudt.org/2.1/schema/qudt#QuantityValue> rdf:type owl:Class ;
                                                rdfs:label "Quantity Value" .


###  http://qudt.org/2.1/schema/qudt#Unit
<http://qudt.org/2.1/schema/qudt#Unit> rdf:type owl:Class ;
                                       rdfs:label "Unit" .


###  http://stko-kwg.geog.ucsb.edu/lod/ontology/AdministrativeLevel
kwg-ont:AdministrativeLevel rdf:type owl:Class ;
                            rdfs:label "Administrative Level" .


###  http://stko-kwg.geog.ucsb.edu/lod/ontology/AdministrativeRegion
kwg-ont:AdministrativeRegion rdf:type owl:Class ;
                             rdfs:subClassOf kwg-ont:Region ,
                                             <http://www.opengis.net/ont/geosparql#Feature> ;
                             rdfs:comment "Source - Global Administrative area database (GADM) (https://gadm.org/data.html)" ;
                             rdfs:label "Administrative Region" .


###  http://stko-kwg.geog.ucsb.edu/lod/ontology/AdministrativeRegion_0
kwg-ont:AdministrativeRegion_0 rdf:type owl:Class ;
                               rdfs:subClassOf kwg-ont:AdministrativeRegion ,
                                               [ rdf:type owl:Restriction ;
                                                 owl:onProperty <http://www.opengis.net/ont/geosparql#hasGeometry> ;
                                                 owl:allValuesFrom <http://www.opengis.net/ont/geosparql#Geometry>
                                               ] ;
                               rdfs:comment "Administrative Region Level 0 - earth" ,
                                            "Source - Global Administrative area database (GADM) (https://gadm.org/data.html)" ;
                               rdfs:label "Administrative Region Level 0" .


###  http://stko-kwg.geog.ucsb.edu/lod/ontology/AdministrativeRegion_1
kwg-ont:AdministrativeRegion_1 rdf:type owl:Class ;
                               rdfs:subClassOf kwg-ont:AdministrativeRegion ,
                                               [ rdf:type owl:Restriction ;
                                                 owl:onProperty <http://www.opengis.net/ont/geosparql#hasGeometry> ;
                                                 owl:allValuesFrom <http://www.opengis.net/ont/geosparql#Geometry>
                                               ] ;
                               rdfs:comment "Administrative Region Level 1 - national level" ,
                                            "Source - Global Administrative area database (GADM) (https://gadm.org/data.html)" ;
                               rdfs:label "Administrative Region Level 1" .


###  http://stko-kwg.geog.ucsb.edu/lod/ontology/AdministrativeRegion_2
kwg-ont:AdministrativeRegion_2 rdf:type owl:Class ;
                               rdfs:subClassOf kwg-ont:AdministrativeRegion ,
                                               [ rdf:type owl:Restriction ;
                                                 owl:onProperty <http://www.opengis.net/ont/geosparql#hasGeometry> ;
                                                 owl:allValuesFrom <http://www.opengis.net/ont/geosparql#Geometry>
                                               ] ;
                               rdfs:comment "Administrative Region Level 2 - state/province/equivalent level" ,
                                            "Source - Global Administrative area database (GADM) (https://gadm.org/data.html)" ;
                               rdfs:label "Administrative Region Level 2" ;
                               owl:backwardCompatibleWith "Administrative Region Level 2 - state/province/equivalent level" .


###  http://stko-kwg.geog.ucsb.edu/lod/ontology/AdministrativeRegion_3
kwg-ont:AdministrativeRegion_3 rdf:type owl:Class ;
                               rdfs:subClassOf kwg-ont:AdministrativeRegion ,
                                               sosa:FeatureOfInterest ,
                                               [ rdf:type owl:Restriction ;
                                                 owl:onProperty <http://www.opengis.net/ont/geosparql#hasDefaultGeometry> ;
                                                 owl:allValuesFrom <http://www.opengis.net/ont/geosparql#Geometry>
                                               ] ,
                                               [ rdf:type owl:Restriction ;
                                                 owl:onProperty <http://www.opengis.net/ont/geosparql#hasGeometry> ;
                                                 owl:allValuesFrom <http://www.opengis.net/ont/geosparql#Geometry>
                                               ] ;
                               rdfs:comment "Administrative Region Level 3 - county/district/equivalent level" ,
                                            "Source - Global Administrative area database (GADM) (https://gadm.org/data.html)" ;
                               rdfs:label "Administrative Region Level 3" .


###  http://stko-kwg.geog.ucsb.edu/lod/ontology/AdministrativeRegion_4
kwg-ont:AdministrativeRegion_4 rdf:type owl:Class ;
                               rdfs:subClassOf kwg-ont:AdministrativeRegion ,
                                               [ rdf:type owl:Restriction ;
                                                 owl:onProperty <http://www.opengis.net/ont/geosparql#hasGeometry> ;
                                                 owl:allValuesFrom <http://www.opengis.net/ont/geosparql#Geometry>
                                               ] ;
                               rdfs:comment "Administrative Region Level 4 - smaller level" ,
                                            "Source - Global Administrative area database (GADM) (https://gadm.org/data.html)" ;
                               rdfs:label "Administrative Region Level 4" .


###  http://stko-kwg.geog.ucsb.edu/lod/ontology/AdministrativeRegion_5
kwg-ont:AdministrativeRegion_5 rdf:type owl:Class ;
                               rdfs:subClassOf kwg-ont:AdministrativeRegion ,
                                               [ rdf:type owl:Restriction ;
                                                 owl:onProperty <http://www.opengis.net/ont/geosparql#hasGeometry> ;
                                                 owl:allValuesFrom <http://www.opengis.net/ont/geosparql#Geometry>
                                               ] ;
                               rdfs:comment "Administrative Region Level 5 - smaller level" ,
                                            "Source - Global Administrative area database (GADM) (https://gadm.org/data.html)" ;
                               rdfs:label "Administrative Region Level 5" .


###  http://stko-kwg.geog.ucsb.edu/lod/ontology/AdministrativeRegion_6
kwg-ont:AdministrativeRegion_6 rdf:type owl:Class ;
                               rdfs:subClassOf kwg-ont:AdministrativeRegion ,
                                               [ rdf:type owl:Restriction ;
                                                 owl:onProperty <http://www.opengis.net/ont/geosparql#hasGeometry> ;
                                                 owl:allValuesFrom <http://www.opengis.net/ont/geosparql#Geometry>
                                               ] ;
                               rdfs:comment "Administrative Region Level 6 - smaller level" ,
                                            "Source - Global Administrative area database (GADM) (https://gadm.org/data.html)" ;
                               rdfs:label "Administrative Region Level 6" .


###  http://stko-kwg.geog.ucsb.edu/lod/ontology/AirPollutant
kwg-ont:AirPollutant rdf:type owl:Class ;
                     rdfs:subClassOf sosa:ObservableProperty ;
                     rdfs:comment "Source - EPA (https://www.epa.gov/outdoor-air-quality-data)" ;
                     rdfs:label "EPA Air Pollutant Type" .


###  http://stko-kwg.geog.ucsb.edu/lod/ontology/AirQualityInstrument
kwg-ont:AirQualityInstrument rdf:type owl:Class ;
                             rdfs:subClassOf sosa:Sensor ;
                             rdfs:comment "Source - EPA (https://www.epa.gov/outdoor-air-quality-data)" ;
                             rdfs:label "EPA Air Quality Instrument/Sensor" .


###  http://stko-kwg.geog.ucsb.edu/lod/ontology/AirQualityObservation
kwg-ont:AirQualityObservation rdf:type owl:Class ;
                              rdfs:subClassOf sosa:Observation ,
                                              [ rdf:type owl:Restriction ;
                                                owl:onProperty sosa:observedProperty ;
                                                owl:allValuesFrom kwg-ont:AirPollutant
                                              ] ;
                              rdfs:comment "Source - EPA (https://www.epa.gov/outdoor-air-quality-data)" ;
                              rdfs:label "EPA Air Quality Observation" .


###  http://stko-kwg.geog.ucsb.edu/lod/ontology/AirQualityObservationCollection
kwg-ont:AirQualityObservationCollection rdf:type owl:Class ;
                                        rdfs:subClassOf sosa:ObservationCollection ,
                                                        [ rdf:type owl:Restriction ;
                                                          owl:onProperty sosa:hasMember ;
                                                          owl:allValuesFrom kwg-ont:AirQualityObservation
                                                        ] ,
                                                        [ rdf:type owl:Restriction ;
                                                          owl:onProperty sosa:observedProperty ;
                                                          owl:allValuesFrom kwg-ont:AirPollutant
                                                        ] ;
                                        rdfs:comment "Source - EPA (https://www.epa.gov/outdoor-air-quality-data)" ;
                                        rdfs:label "EPA Air Quality Observation Collection" .


###  http://stko-kwg.geog.ucsb.edu/lod/ontology/AirQualitySite
kwg-ont:AirQualitySite rdf:type owl:Class ;
                       rdfs:subClassOf sosa:Platform ,
                                       [ rdf:type owl:Restriction ;
                                         owl:onProperty kwg-ont:sfWithin ;
                                         owl:someValuesFrom kwg-ont:AdministrativeRegion
                                       ] ,
                                       [ rdf:type owl:Restriction ;
                                         owl:onProperty kwg-ont:sfWithin ;
                                         owl:someValuesFrom kwg-ont:S2Cell
                                       ] ,
                                       [ rdf:type owl:Restriction ;
                                         owl:onProperty <http://www.opengis.net/ont/geosparql#hasDefaultGeometry> ;
                                         owl:allValuesFrom <http://www.opengis.net/ont/geosparql#Geometry>
                                       ] ,
                                       [ rdf:type owl:Restriction ;
                                         owl:onProperty <http://www.opengis.net/ont/geosparql#hasGeometry> ;
                                         owl:allValuesFrom <http://www.opengis.net/ont/geosparql#Geometry>
                                       ] ,
                                       [ rdf:type owl:Restriction ;
                                         owl:onProperty sosa:hosts ;
                                         owl:allValuesFrom kwg-ont:AirQualityInstrument
                                       ] ;
                       rdfs:comment "Source - EPA (https://www.epa.gov/outdoor-air-quality-data)" ;
                       rdfs:label "EPA Air Quality Site" .


###  http://stko-kwg.geog.ucsb.edu/lod/ontology/BlueskyModel
kwg-ont:BlueskyModel rdf:type owl:Class ;
                     rdfs:subClassOf sosa:Sensor ;
                     rdfs:comment "Source - Bluesky forecast (https://tools.airfire.org/websky/v1/#status)" ;
                     rdfs:label "Bluesky Model" .


###  http://stko-kwg.geog.ucsb.edu/lod/ontology/BlueskyModeledWildfire
kwg-ont:BlueskyModeledWildfire rdf:type owl:Class ;
                               rdfs:subClassOf <http://www.opengis.net/ont/geosparql#Feature> ,
                                               sosa:FeatureOfInterest ,
                                               [ rdf:type owl:Restriction ;
                                                 owl:onProperty kwg-ont:hasTemporalScope ;
                                                 owl:someValuesFrom time:Instant
                                               ] ,
                                               [ rdf:type owl:Restriction ;
                                                 owl:onProperty kwg-ont:spatialRelation ;
                                                 owl:someValuesFrom kwg-ont:AdministrativeRegion_3
                                               ] ,
                                               [ rdf:type owl:Restriction ;
                                                 owl:onProperty kwg-ont:spatialRelation ;
                                                 owl:someValuesFrom kwg-ont:S2Cell
                                               ] ,
                                               [ rdf:type owl:Restriction ;
                                                 owl:onProperty <http://www.opengis.net/ont/geosparql#hasDefaultGeometry> ;
                                                 owl:allValuesFrom <http://www.opengis.net/ont/geosparql#Geometry>
                                               ] ,
                                               [ rdf:type owl:Restriction ;
                                                 owl:onProperty <http://www.opengis.net/ont/geosparql#hasGeometry> ;
                                                 owl:allValuesFrom <http://www.opengis.net/ont/geosparql#Geometry>
                                               ] ;
                               rdfs:comment "Source - Bluesky forecast (https://tools.airfire.org/websky/v1/#status)" ;
                               rdfs:label "Bluesky Modeled Wildfire" .


###  http://stko-kwg.geog.ucsb.edu/lod/ontology/BlueskyWildfireObservableProperty
kwg-ont:BlueskyWildfireObservableProperty rdf:type owl:Class ;
                                          rdfs:subClassOf sosa:ObservableProperty ;
                                          rdfs:comment "Source - Bluesky forecast (https://tools.airfire.org/websky/v1/#status)" ;
                                          rdfs:label "Bluesky Wildfire Observable Property" .


###  http://stko-kwg.geog.ucsb.edu/lod/ontology/BlueskyWildfireObservation
kwg-ont:BlueskyWildfireObservation rdf:type owl:Class ;
                                   rdfs:subClassOf sosa:Observation ,
                                                   [ rdf:type owl:Restriction ;
                                                     owl:onProperty sosa:hasFeatureOfInterest ;
                                                     owl:allValuesFrom kwg-ont:BlueskyModeledWildfire
                                                   ] ,
                                                   [ rdf:type owl:Restriction ;
                                                     owl:onProperty sosa:observedProperty ;
                                                     owl:allValuesFrom kwg-ont:BlueskyWildfireObservableProperty
                                                   ] ;
                                   rdfs:comment "Source - Bluesky forecast (https://tools.airfire.org/websky/v1/#status)" ;
                                   rdfs:label "Blueky Wildfire Observation" .


###  http://stko-kwg.geog.ucsb.edu/lod/ontology/BlueskyWildfireObservationCollection
kwg-ont:BlueskyWildfireObservationCollection rdf:type owl:Class ;
                                             rdfs:subClassOf sosa:ObservationCollection ,
                                                             [ rdf:type owl:Restriction ;
                                                               owl:onProperty sosa:hasMember ;
                                                               owl:allValuesFrom kwg-ont:BlueskyWildfireObservation
                                                             ] ,
                                                             [ rdf:type owl:Restriction ;
                                                               owl:onProperty sosa:madeBySensor ;
                                                               owl:allValuesFrom kwg-ont:BlueskyModel
                                                             ] ,
                                                             [ rdf:type owl:Restriction ;
                                                               owl:onProperty sosa:phenomenonTime ;
                                                               owl:allValuesFrom time:Instant
                                                             ] ;
                                             rdfs:comment "Source - Bluesky forecast (https://tools.airfire.org/websky/v1/#status)" ;
                                             rdfs:label "Bluesky Wildfire Observation Collection" .


###  http://stko-kwg.geog.ucsb.edu/lod/ontology/Cell
kwg-ont:Cell rdf:type owl:Class ;
             rdfs:subClassOf <http://www.opengis.net/ont/geosparql#SpatialObject> ;
             rdfs:comment "A unit defined in a discrete global grid system (DGG) to partition the Earths surface." ;
             rdfs:label "Cell" .


###  http://stko-kwg.geog.ucsb.edu/lod/ontology/CensusACS5YearEstimatesObservation
kwg-ont:CensusACS5YearEstimatesObservation rdf:type owl:Class ;
                                           rdfs:subClassOf sosa:Observation ,
                                                           [ rdf:type owl:Restriction ;
                                                             owl:onProperty sosa:observedProperty ;
                                                             owl:allValuesFrom kwg-ont:CensusObservableProperty
                                                           ] ;
                                           rdfs:comment "American Community Survey 5-Year Estimate Observation" ,
                                                        "Source - US Census Bureau (https://www.census.gov/data/datasets.html)" ;
                                           rdfs:label "American Community Survey 5-Year Estimate Observation" .


###  http://stko-kwg.geog.ucsb.edu/lod/ontology/CensusACS5YearEstimatesObservationCollection
kwg-ont:CensusACS5YearEstimatesObservationCollection rdf:type owl:Class ;
                                                     rdfs:subClassOf sosa:ObservationCollection ,
                                                                     [ rdf:type owl:Restriction ;
                                                                       owl:onProperty sosa:hasFeatureOfInterest ;
                                                                       owl:allValuesFrom kwg-ont:USCensusMSA
                                                                     ] ,
                                                                     [ rdf:type owl:Restriction ;
                                                                       owl:onProperty sosa:hasMember ;
                                                                       owl:allValuesFrom kwg-ont:CensusACS5YearEstimatesObservation
                                                                     ] ;
                                                     rdfs:comment "American Community Survey 5-Year Estimates Observation Collection" ,
                                                                  "Source - US Census Bureau (https://www.census.gov/data/datasets.html)" ;
                                                     rdfs:label "American Community Survey 5-Year Estimates" .


###  http://stko-kwg.geog.ucsb.edu/lod/ontology/CensusObservableProperty
kwg-ont:CensusObservableProperty rdf:type owl:Class ;
                                 rdfs:subClassOf sosa:ObservableProperty ;
                                 rdfs:comment "American Community Survey 5-Year Estimate Observed Property" ,
                                              "Source - US Census Bureau (https://www.census.gov/data/datasets.html)" ;
                                 rdfs:label "American Community Survey 5-Year Estimate Property" .


###  http://stko-kwg.geog.ucsb.edu/lod/ontology/ChiefJudge
kwg-ont:ChiefJudge rdf:type owl:Class ;
                   rdfs:comment "Source - HIFLD (https://hifld-geoplatform.opendata.arcgis.com/datasets/us-district-court-jurisdictions/explore?location=40.830482%2C-90.571266%2C4.68, https://www.uscourts.gov/about-federal-courts/federal-courts-public/court-website-links)" ;
                   rdfs:label "Chief Judge" .


###  http://stko-kwg.geog.ucsb.edu/lod/ontology/ClimateDivisionObservationCollection
kwg-ont:ClimateDivisionObservationCollection rdf:type owl:Class ;
                                             rdfs:subClassOf sosa:ObservationCollection ,
                                                             [ rdf:type owl:Restriction ;
                                                               owl:onProperty sosa:hasFeatureOfInterest ;
                                                               owl:allValuesFrom kwg-ont:USClimateDivision
                                                             ] ,
                                                             [ rdf:type owl:Restriction ;
                                                               owl:onProperty sosa:hasMember ;
                                                               owl:allValuesFrom kwg-ont:ClimateDivisionPropertyObservationCollection
                                                             ] ;
                                             rdfs:comment "Observation Collection for each individual climate division" ,
                                                          "Source - NOAA (https://www.ncdc.noaa.gov/cag/divisional/mapping)" ;
                                             rdfs:label "Climate Division Observation Collection" .


###  http://stko-kwg.geog.ucsb.edu/lod/ontology/ClimateDivisionObservationResult
kwg-ont:ClimateDivisionObservationResult rdf:type owl:Class ;
                                         rdfs:subClassOf sosa:Result ;
                                         rdfs:comment "Source - NOAA (https://www.ncdc.noaa.gov/cag/divisional/mapping)" ;
                                         rdfs:label "Climate DIvision Observation Result" .


###  http://stko-kwg.geog.ucsb.edu/lod/ontology/ClimateDivisionPropertyObservationCollection
kwg-ont:ClimateDivisionPropertyObservationCollection rdf:type owl:Class ;
                                                     rdfs:subClassOf sosa:ObservationCollection ,
                                                                     [ rdf:type owl:Restriction ;
                                                                       owl:onProperty sosa:hasMember ;
                                                                       owl:allValuesFrom kwg-ont:ClimateObservation
                                                                     ] ,
                                                                     [ rdf:type owl:Restriction ;
                                                                       owl:onProperty sosa:observedProperty ;
                                                                       owl:allValuesFrom kwg-ont:ClimateObservableProperty
                                                                     ] ;
                                                     rdfs:comment "Observation Collection for each individual climate division boundary and climate property" ,
                                                                  "Source - NOAA (https://www.ncdc.noaa.gov/cag/divisional/mapping)" ;
                                                     rdfs:label "Climate Division Property Observation Collection" .


###  http://stko-kwg.geog.ucsb.edu/lod/ontology/ClimateObservableProperty
kwg-ont:ClimateObservableProperty rdf:type owl:Class ;
                                  rdfs:subClassOf sosa:ObservableProperty ;
                                  rdfs:comment "Climate Properties measured by NOAA for their Climate Division Boundaries" ,
                                               "Source - NOAA (https://www.ncdc.noaa.gov/cag/divisional/mapping)" ;
                                  rdfs:label "Climate Observable Property" .


###  http://stko-kwg.geog.ucsb.edu/lod/ontology/ClimateObservation
kwg-ont:ClimateObservation rdf:type owl:Class ;
                           rdfs:subClassOf sosa:Observation ,
                                           [ rdf:type owl:Restriction ;
                                             owl:onProperty sosa:observedProperty ;
                                             owl:allValuesFrom kwg-ont:ClimateObservableProperty
                                           ] ;
                           rdfs:comment "NOAA Climate Division individual observations" ,
                                        "Source - NOAA (https://www.ncdc.noaa.gov/cag/divisional/mapping)" ;
                           rdfs:label "Climate Observation" .


###  http://stko-kwg.geog.ucsb.edu/lod/ontology/ComplexFire
kwg-ont:ComplexFire rdf:type owl:Class ;
                    rdfs:subClassOf kwg-ont:Fire ;
                    rdfs:label "Complex Fire" .


###  http://stko-kwg.geog.ucsb.edu/lod/ontology/CrisisCounselling
kwg-ont:CrisisCounselling rdf:type owl:Class ;
                          rdfs:subClassOf kwg-ont:Program ;
                          rdfs:comment "Source - OpenFEMA (https://www.fema.gov/about/openfema/data-sets)" ;
                          rdfs:label "Crisis Counselling" .


###  http://stko-kwg.geog.ucsb.edu/lod/ontology/CroplandObservableProperty
kwg-ont:CroplandObservableProperty rdf:type owl:Class ;
                                   rdfs:subClassOf sosa:ObservableProperty ;
                                   rdfs:comment "Source - https://nassgeodata.gmu.edu/CropScape/" ;
                                   rdfs:label "Cropland Observable Property" .


###  http://stko-kwg.geog.ucsb.edu/lod/ontology/CroplandObservation
kwg-ont:CroplandObservation rdf:type owl:Class ;
                            rdfs:subClassOf sosa:Observation ,
                                            [ rdf:type owl:Restriction ;
                                              owl:onProperty sosa:observedProperty ;
                                              owl:allValuesFrom kwg-ont:CroplandObservableProperty
                                            ] ;
                            rdfs:comment "Source - https://nassgeodata.gmu.edu/CropScape/" ;
                            rdfs:label "Cropland Observation" .


###  http://stko-kwg.geog.ucsb.edu/lod/ontology/CroplandObservationCollection
kwg-ont:CroplandObservationCollection rdf:type owl:Class ;
                                      rdfs:subClassOf sosa:ObservationCollection ,
                                                      [ rdf:type owl:Restriction ;
                                                        owl:onProperty sosa:hasFeatureOfInterest ;
                                                        owl:allValuesFrom kwg-ont:S2Cell
                                                      ] ,
                                                      [ rdf:type owl:Restriction ;
                                                        owl:onProperty sosa:hasMember ;
                                                        owl:allValuesFrom kwg-ont:CroplandObservation
                                                      ] ,
                                                      [ rdf:type owl:Restriction ;
                                                        owl:onProperty sosa:phenomenonTime ;
                                                        owl:allValuesFrom time:TemporalEntity
                                                      ] ;
                                      rdfs:comment "Source - https://nassgeodata.gmu.edu/CropScape/" ;
                                      rdfs:label "Cropland Observation Collection" .


###  http://stko-kwg.geog.ucsb.edu/lod/ontology/CroplandResult
kwg-ont:CroplandResult rdf:type owl:Class ;
                       rdfs:subClassOf sosa:Result ;
                       rdfs:comment "Source - https://nassgeodata.gmu.edu/CropScape/" ;
                       rdfs:label "Cropland Result" .


###  http://stko-kwg.geog.ucsb.edu/lod/ontology/DebrisRemoval-PA-A
kwg-ont:DebrisRemoval-PA-A rdf:type owl:Class ;
                           rdfs:subClassOf kwg-ont:PublicAssistance ;
                           rdfs:comment "Source - OpenFEMA (https://www.fema.gov/about/openfema/data-sets)" ;
                           rdfs:label "Debris Removal (PA-A)" .


###  http://stko-kwg.geog.ucsb.edu/lod/ontology/Declaration
kwg-ont:Declaration rdf:type owl:Class ;
                    rdfs:comment "Source - OpenFEMA (https://www.fema.gov/about/openfema/data-sets)" ,
                                 "The class that is used to represent all instances of declaration from the OpenFEMA dataset" ;
                    rdfs:label "FEMA Declaration" .


###  http://stko-kwg.geog.ucsb.edu/lod/ontology/DirectFederalAssistance
kwg-ont:DirectFederalAssistance rdf:type owl:Class ;
                                rdfs:subClassOf kwg-ont:Program ;
                                rdfs:comment "Source - OpenFEMA (https://www.fema.gov/about/openfema/data-sets)" ;
                                rdfs:label "Direct Federal Assistance" .


###  http://stko-kwg.geog.ucsb.edu/lod/ontology/DisasterHousing
kwg-ont:DisasterHousing rdf:type owl:Class ;
                        rdfs:subClassOf kwg-ont:Program ;
                        rdfs:comment "Source - OpenFEMA (https://www.fema.gov/about/openfema/data-sets)" ;
                        rdfs:label "Disaster Housing" .


###  http://stko-kwg.geog.ucsb.edu/lod/ontology/DisasterUnemploymentAssistance
kwg-ont:DisasterUnemploymentAssistance rdf:type owl:Class ;
                                       rdfs:subClassOf kwg-ont:Program ;
                                       rdfs:comment "Source - OpenFEMA (https://www.fema.gov/about/openfema/data-sets)" ;
                                       rdfs:label "Disaster Unemployment-Assistance" .


###  http://stko-kwg.geog.ucsb.edu/lod/ontology/DoD
kwg-ont:DoD rdf:type owl:Class ;
            rdfs:subClassOf kwg-ont:Program ;
            rdfs:comment "Source - OpenFEMA (https://www.fema.gov/about/openfema/data-sets)" ;
            rdfs:label "DoD" .


###  http://stko-kwg.geog.ucsb.edu/lod/ontology/DroughtIntensity
kwg-ont:DroughtIntensity rdf:type owl:Class ;
                         rdfs:subClassOf sosa:ObservableProperty ;
                         rdfs:comment "Source - https://droughtmonitor.unl.edu/DmData/GISData.aspx" ;
                         rdfs:label "Drought Intensity" .


###  http://stko-kwg.geog.ucsb.edu/lod/ontology/DroughtZone
kwg-ont:DroughtZone rdf:type owl:Class ;
                    rdfs:subClassOf kwg-ont:Hazard ,
                                    <http://www.opengis.net/ont/geosparql#Feature> ,
                                    <https://undrr.org/hazard/hip/Drought> ,
                                    [ rdf:type owl:Restriction ;
                                      owl:onProperty kwg-ont:hasTemporalScope ;
                                      owl:someValuesFrom time:TemporalEntity
                                    ] ,
                                    [ rdf:type owl:Restriction ;
                                      owl:onProperty kwg-ont:spatialRelation ;
                                      owl:someValuesFrom kwg-ont:AdministrativeRegion_3
                                    ] ,
                                    [ rdf:type owl:Restriction ;
                                      owl:onProperty kwg-ont:spatialRelation ;
                                      owl:someValuesFrom kwg-ont:S2Cell
                                    ] ,
                                    [ rdf:type owl:Restriction ;
                                      owl:onProperty <http://www.opengis.net/ont/geosparql#hasDefaultGeometry> ;
                                      owl:someValuesFrom <http://www.opengis.net/ont/geosparql#Geometry>
                                    ] ,
                                    [ rdf:type owl:Restriction ;
                                      owl:onProperty <http://www.opengis.net/ont/geosparql#hasGeometry> ;
                                      owl:someValuesFrom <http://www.opengis.net/ont/geosparql#Geometry>
                                    ] ;
                    rdfs:comment "Source - https://droughtmonitor.unl.edu/DmData/GISData.aspx" ;
                    rdfs:label "Drought Zone" .


###  http://stko-kwg.geog.ucsb.edu/lod/ontology/DroughtZoneOverlapObservation
kwg-ont:DroughtZoneOverlapObservation rdf:type owl:Class ;
                                      rdfs:subClassOf sosa:Observation ,
                                                      [ rdf:type owl:Restriction ;
                                                        owl:onProperty sosa:observedProperty ;
                                                        owl:allValuesFrom kwg-ont:DroughtIntensity
                                                      ] ;
                                      rdfs:comment "Source - https://droughtmonitor.unl.edu/DmData/GISData.aspx" ;
                                      rdfs:label "Drought Zone Overlap Observation" .


###  http://stko-kwg.geog.ucsb.edu/lod/ontology/DroughtZoneOverlapObservationCollection
kwg-ont:DroughtZoneOverlapObservationCollection rdf:type owl:Class ;
                                                rdfs:subClassOf sosa:ObservationCollection ,
                                                                [ rdf:type owl:Restriction ;
                                                                  owl:onProperty sosa:hasFeatureOfInterest ;
                                                                  owl:allValuesFrom kwg-ont:S2Cell
                                                                ] ,
                                                                [ rdf:type owl:Restriction ;
                                                                  owl:onProperty sosa:hasMember ;
                                                                  owl:allValuesFrom kwg-ont:DroughtZoneOverlapObservation
                                                                ] ;
                                                rdfs:comment "Source - https://droughtmonitor.unl.edu/DmData/GISData.aspx" ;
                                                rdfs:label "Drought Zone Overlap Observation Collection" .


###  http://stko-kwg.geog.ucsb.edu/lod/ontology/Earthquake
kwg-ont:Earthquake rdf:type owl:Class ;
                   rdfs:subClassOf kwg-ont:Hazard ,
                                   <http://www.opengis.net/ont/geosparql#Feature> ,
                                   sosa:FeatureOfInterest ,
                                   <https://undrr.org/hazard/hip/EarthquakeSurfaceRupture> ,
                                   [ rdf:type owl:Restriction ;
                                     owl:onProperty kwg-ont:hasTemporalScope ;
                                     owl:someValuesFrom time:Instant
                                   ] ,
                                   [ rdf:type owl:Restriction ;
                                     owl:onProperty kwg-ont:sfWithin ;
                                     owl:someValuesFrom kwg-ont:AdministrativeRegion_3
                                   ] ,
                                   [ rdf:type owl:Restriction ;
                                     owl:onProperty kwg-ont:sfWithin ;
                                     owl:someValuesFrom kwg-ont:S2Cell
                                   ] ,
                                   [ rdf:type owl:Restriction ;
                                     owl:onProperty <http://www.opengis.net/ont/geosparql#hasDefaultGeometry> ;
                                     owl:someValuesFrom <http://www.opengis.net/ont/geosparql#Geometry>
                                   ] ,
                                   [ rdf:type owl:Restriction ;
                                     owl:onProperty <http://www.opengis.net/ont/geosparql#hasGeometry> ;
                                     owl:someValuesFrom <http://www.opengis.net/ont/geosparql#Geometry>
                                   ] ;
                   rdfs:comment "Source - USGS (https://earthquake.usgs.gov/earthquakes/search/)" ;
                   rdfs:label "Earthquake" .


###  http://stko-kwg.geog.ucsb.edu/lod/ontology/EarthquakeObservableProperty
kwg-ont:EarthquakeObservableProperty rdf:type owl:Class ;
                                     rdfs:subClassOf sosa:ObservableProperty ;
                                     rdfs:comment "Source - USGS (https://earthquake.usgs.gov/earthquakes/search/)" ;
                                     rdfs:label "Earthquake Observable Property" .


###  http://stko-kwg.geog.ucsb.edu/lod/ontology/EarthquakeObservationCollection
kwg-ont:EarthquakeObservationCollection rdf:type owl:Class ;
                                        rdfs:subClassOf sosa:ObservationCollection ,
                                                        [ rdf:type owl:Restriction ;
                                                          owl:onProperty sosa:hasFeatureOfInterest ;
                                                          owl:allValuesFrom kwg-ont:Earthquake
                                                        ] ,
                                                        [ rdf:type owl:Restriction ;
                                                          owl:onProperty sosa:hasMember ;
                                                          owl:allValuesFrom sosa:EarthquakeObservation
                                                        ] ,
                                                        [ rdf:type owl:Restriction ;
                                                          owl:onProperty sosa:phenomenonTime ;
                                                          owl:allValuesFrom time:Instant
                                                        ] ;
                                        rdfs:comment "Source - USGS (https://earthquake.usgs.gov/earthquakes/search/)" ;
                                        rdfs:label "Earthquake Observation Collection" .


###  http://stko-kwg.geog.ucsb.edu/lod/ontology/EmergencyDeclaration
kwg-ont:EmergencyDeclaration rdf:type owl:Class ;
                             rdfs:subClassOf kwg-ont:Declaration ;
                             rdfs:comment "Source - OpenFEMA (https://www.fema.gov/about/openfema/data-sets)" ;
                             rdfs:label "Emergency Declaration" .


###  http://stko-kwg.geog.ucsb.edu/lod/ontology/EventSegment
kwg-ont:EventSegment rdf:type owl:Class ;
                     rdfs:subClassOf [ rdf:type owl:Restriction ;
                                       owl:onProperty kwg-ont:endsAt ;
                                       owl:someValuesFrom kwg-ont:Fix
                                     ] ;
                     rdfs:comment "Source - NOAA (https://www.ncdc.noaa.gov/stormevents/ftp.jsp)" ;
                     rdfs:label "NOAA Hazard Event Segment" .


###  http://stko-kwg.geog.ucsb.edu/lod/ontology/FEMADisaster
kwg-ont:FEMADisaster rdf:type owl:Class ;
                     rdfs:subClassOf kwg-ont:Hazard ,
                                     <http://www.opengis.net/ont/geosparql#Feature> ;
                     rdfs:comment "Source - OpenFEMA (https://www.fema.gov/about/openfema/data-sets)" ,
                                  "The class that is used to represent all emergency, fire and major disasters from the OpemFEMA dataset" ;
                     rdfs:label "Disaster from FEMA" .


###  http://stko-kwg.geog.ucsb.edu/lod/ontology/FederalJudicalDistrict
kwg-ont:FederalJudicalDistrict rdf:type owl:Class ;
                               rdfs:subClassOf kwg-ont:Region ,
                                               <http://www.opengis.net/ont/geosparql#Feature> ,
                                               [ rdf:type owl:Restriction ;
                                                 owl:onProperty <http://www.opengis.net/ont/geosparql#spatialRelation> ;
                                                 owl:someValuesFrom kwg-ont:AdministrativeRegion_3
                                               ] ,
                                               [ rdf:type owl:Restriction ;
                                                 owl:onProperty <http://www.opengis.net/ont/geosparql#spatialRelation> ;
                                                 owl:someValuesFrom kwg-ont:S2Cell
                                               ] ,
                                               [ rdf:type owl:Restriction ;
                                                 owl:onProperty <http://www.opengis.net/ont/geosparql#hasDefaultGeometry> ;
                                                 owl:allValuesFrom <http://www.opengis.net/ont/geosparql#Geometry>
                                               ] ,
                                               [ rdf:type owl:Restriction ;
                                                 owl:onProperty <http://www.opengis.net/ont/geosparql#hasGeometry> ;
                                                 owl:allValuesFrom <http://www.opengis.net/ont/geosparql#Geometry>
                                               ] ;
                               rdfs:comment "Source - HIFLD (https://hifld-geoplatform.opendata.arcgis.com/datasets/us-district-court-jurisdictions/explore?location=40.830482%2C-90.571266%2C4.68, https://www.uscourts.gov/about-federal-courts/federal-courts-public/court-website-links)" ;
                               rdfs:label "Federal Judicial District" .


###  http://stko-kwg.geog.ucsb.edu/lod/ontology/Fire
kwg-ont:Fire rdf:type owl:Class ;
             rdfs:subClassOf kwg-ont:Hazard ;
             rdfs:label "Fire" .


###  http://stko-kwg.geog.ucsb.edu/lod/ontology/FireCause
kwg-ont:FireCause rdf:type owl:Class ;
                  rdfs:comment "A classification of an event that causes a fire, e.g. \"human-caused\"" ,
                               "Source - NIFC (https://data-nifc.opendata.arcgis.com/ )" ;
                  rdfs:label "NIFC Fire Cause" .


###  http://stko-kwg.geog.ucsb.edu/lod/ontology/FireManagementAssistance-PA-I
kwg-ont:FireManagementAssistance-PA-I rdf:type owl:Class ;
                                      rdfs:subClassOf kwg-ont:PublicAssistance ;
                                      rdfs:comment "Source - OpenFEMA (https://www.fema.gov/about/openfema/data-sets)" ;
                                      rdfs:label "Fire Management Assistance (PA-I)" .


###  http://stko-kwg.geog.ucsb.edu/lod/ontology/FireManagementDeclaration
kwg-ont:FireManagementDeclaration rdf:type owl:Class ;
                                  rdfs:subClassOf kwg-ont:Declaration ;
                                  rdfs:comment "Source - OpenFEMA (https://www.fema.gov/about/openfema/data-sets)" ;
                                  rdfs:label "Fire Management Declaration" .


###  http://stko-kwg.geog.ucsb.edu/lod/ontology/FireMappingAssessmentLabel
kwg-ont:FireMappingAssessmentLabel rdf:type owl:Class ;
                                   rdfs:comment "Source - MTBS (https://mtbs.gov/direct-downloadhttps://mtbs.gov/direct-download)" ;
                                   rdfs:label "MTBS Fire Mapping Assessment Label" .


###  http://stko-kwg.geog.ucsb.edu/lod/ontology/Fix
kwg-ont:Fix rdf:type owl:Class ;
            rdfs:subClassOf [ rdf:type owl:Restriction ;
                              owl:onProperty <http://www.opengis.net/ont/geosparql#hasDefaultGeometry> ;
                              owl:allValuesFrom <http://www.opengis.net/ont/geosparql#Geometry>
                            ] ,
                            [ rdf:type owl:Restriction ;
                              owl:onProperty <http://www.opengis.net/ont/geosparql#hasGeometry> ;
                              owl:allValuesFrom <http://www.opengis.net/ont/geosparql#Geometry>
                            ] ;
            rdfs:comment "Source - NOAA (https://www.ncdc.noaa.gov/stormevents/ftp.jsp)" ;
            rdfs:label "NOAA Hazard Fix" .


###  http://stko-kwg.geog.ucsb.edu/lod/ontology/Geometry
kwg-ont:Geometry rdf:type owl:Class ;
                 rdfs:label "Geometry" .


###  http://stko-kwg.geog.ucsb.edu/lod/ontology/GeometryCollection
kwg-ont:GeometryCollection rdf:type owl:Class ;
                           rdfs:subClassOf <http://www.opengis.net/ont/geosparql#SpatialObject> ;
                           rdfs:label "Geometry Collection" .


###  http://stko-kwg.geog.ucsb.edu/lod/ontology/Hazard
kwg-ont:Hazard rdf:type owl:Class ;
               rdfs:comment "Hazard" ,
                            "The general hazard event class in KWG" ,
                            "event" ;
               rdfs:label "Hazard" .


###  http://stko-kwg.geog.ucsb.edu/lod/ontology/HazardEpisode
kwg-ont:HazardEpisode rdf:type owl:Class ;
                      rdfs:comment "Source - NOAA (https://www.ncdc.noaa.gov/stormevents/ftp.jsp)" ;
                      rdfs:label "NOAA Hazard Episode" .


###  http://stko-kwg.geog.ucsb.edu/lod/ontology/HazardMitigation
kwg-ont:HazardMitigation rdf:type owl:Class ;
                         rdfs:subClassOf kwg-ont:Program ;
                         rdfs:comment "Source - OpenFEMA (https://www.fema.gov/about/openfema/data-sets)" ;
                         rdfs:label "Hazard Mitigation" .


###  http://stko-kwg.geog.ucsb.edu/lod/ontology/HealthCareFacility
kwg-ont:HealthCareFacility rdf:type owl:Class ;
                           rdfs:subClassOf <http://www.opengis.net/ont/geosparql#Feature> ;
                           rdfs:label "Health Care Facility" .


###  http://stko-kwg.geog.ucsb.edu/lod/ontology/HelipadAvailability
kwg-ont:HelipadAvailability rdf:type owl:Class ;
                            rdfs:comment "Source - https://hifld-geoplatform.opendata.arcgis.com/datasets/hospitals-2/about" ;
                            rdfs:label "Helipad Availability" .


###  http://stko-kwg.geog.ucsb.edu/lod/ontology/Hospital
kwg-ont:Hospital rdf:type owl:Class ;
                 rdfs:subClassOf kwg-ont:HealthCareFacility ,
                                 [ rdf:type owl:Restriction ;
                                   owl:onProperty <http://www.opengis.net/ont/geosparql#hasDefaultGeometry> ;
                                   owl:allValuesFrom <http://www.opengis.net/ont/geosparql#Geometry>
                                 ] ,
                                 [ rdf:type owl:Restriction ;
                                   owl:onProperty <http://www.opengis.net/ont/geosparql#hasGeometry> ;
                                   owl:allValuesFrom <http://www.opengis.net/ont/geosparql#Geometry>
                                 ] ;
                 rdfs:comment "Source - https://hifld-geoplatform.opendata.arcgis.com/datasets/hospitals-2/about" ;
                 rdfs:label "Hospital" .


###  http://stko-kwg.geog.ucsb.edu/lod/ontology/HospitalStatus
kwg-ont:HospitalStatus rdf:type owl:Class ;
                       rdfs:comment "Source - https://hifld-geoplatform.opendata.arcgis.com/datasets/hospitals-2/about" ;
                       rdfs:label "Hospital Status" .


###  http://stko-kwg.geog.ucsb.edu/lod/ontology/HospitalType
kwg-ont:HospitalType rdf:type owl:Class ;
                     rdfs:comment "Source - https://hifld-geoplatform.opendata.arcgis.com/datasets/hospitals-2/about" ;
                     rdfs:label "Hospital Type" .


###  http://stko-kwg.geog.ucsb.edu/lod/ontology/HousingAssistance
kwg-ont:HousingAssistance rdf:type owl:Class ;
                          rdfs:subClassOf kwg-ont:Program ;
                          rdfs:comment "Source - OpenFEMA (https://www.fema.gov/about/openfema/data-sets)" ;
                          rdfs:label "Housing Assistance" .


###  http://stko-kwg.geog.ucsb.edu/lod/ontology/ImpactObservableProperty
kwg-ont:ImpactObservableProperty rdf:type owl:Class ;
                                 rdfs:subClassOf sosa:ObservableProperty ;
                                 rdfs:comment "Source - NOAA (https://www.ncdc.noaa.gov/stormevents/ftp.jsp)" ;
                                 rdfs:label "Impact Observable Property" .


###  http://stko-kwg.geog.ucsb.edu/lod/ontology/ImpactObservation
kwg-ont:ImpactObservation rdf:type owl:Class ;
                          rdfs:subClassOf sosa:Observation ,
                                          [ rdf:type owl:Restriction ;
                                            owl:onProperty sosa:observedProperty ;
                                            owl:allValuesFrom kwg-ont:ImpactObservableProperty
                                          ] ;
                          rdfs:comment "Source - NOAA (https://www.ncdc.noaa.gov/stormevents/ftp.jsp)" ;
                          rdfs:label "Impact Observation" .


###  http://stko-kwg.geog.ucsb.edu/lod/ontology/ImpactObservationCollection
kwg-ont:ImpactObservationCollection rdf:type owl:Class ;
                                    rdfs:subClassOf sosa:ObservationCollection ,
                                                    [ rdf:type owl:Restriction ;
                                                      owl:onProperty sosa:hasFeatureOfInterest ;
                                                      owl:allValuesFrom kwg-ont:NOAAHazardEvent
                                                    ] ,
                                                    [ rdf:type owl:Restriction ;
                                                      owl:onProperty sosa:hasMember ;
                                                      owl:allValuesFrom kwg-ont:ImpactObservation
                                                    ] ,
                                                    [ rdf:type owl:Restriction ;
                                                      owl:onProperty sosa:phenomenonTime ;
                                                      owl:allValuesFrom time:TemporalEntity
                                                    ] ;
                                    rdfs:comment "Source - NOAA (https://www.ncdc.noaa.gov/stormevents/ftp.jsp)" ;
                                    rdfs:label "Impact Observation Collection" .


###  http://stko-kwg.geog.ucsb.edu/lod/ontology/IndividualAndFamilyGrant
kwg-ont:IndividualAndFamilyGrant rdf:type owl:Class ;
                                 rdfs:subClassOf kwg-ont:Program ;
                                 rdfs:comment "Source - OpenFEMA (https://www.fema.gov/about/openfema/data-sets)" ;
                                 rdfs:label "Individual & Family Grant" .


###  http://stko-kwg.geog.ucsb.edu/lod/ontology/IndividualAssistance
kwg-ont:IndividualAssistance rdf:type owl:Class ;
                             rdfs:subClassOf kwg-ont:Program ;
                             rdfs:comment "Source - OpenFEMA (https://www.fema.gov/about/openfema/data-sets)" ;
                             rdfs:label "Individual Assistance" .


###  http://stko-kwg.geog.ucsb.edu/lod/ontology/IndividualAssistance-PA-C
kwg-ont:IndividualAssistance-PA-C rdf:type owl:Class ;
                                  rdfs:subClassOf kwg-ont:PublicAssistance ;
                                  rdfs:comment "Source - OpenFEMA (https://www.fema.gov/about/openfema/data-sets)" ;
                                  rdfs:label "Individual Assistance (PA-C)" .


###  http://stko-kwg.geog.ucsb.edu/lod/ontology/IndividualsAndHouseholds
kwg-ont:IndividualsAndHouseholds rdf:type owl:Class ;
                                 rdfs:subClassOf kwg-ont:Program ;
                                 rdfs:comment "Source - OpenFEMA (https://www.fema.gov/about/openfema/data-sets)" ;
                                 rdfs:label "Individuals & Households" .


###  http://stko-kwg.geog.ucsb.edu/lod/ontology/JudgeInfo
kwg-ont:JudgeInfo rdf:type owl:Class ;
                   rdfs:comment "Source - HIFLD (https://hifld-geoplatform.opendata.arcgis.com/datasets/us-district-court-jurisdictions/explore?location=40.830482%2C-90.571266%2C4.68, https://www.uscourts.gov/about-federal-courts/federal-courts-public/court-website-links)" ;
                   rdfs:label "Judge Info" .


###  http://stko-kwg.geog.ucsb.edu/lod/ontology/KWGCellLevel11
kwg-ont:KWGCellLevel11 rdf:type owl:Class ;
                       rdfs:subClassOf kwg-ont:S2Cell ;
                       rdfs:comment "S2 Cell Level 11" ,
                                    "Source - https://s2geometry.io/" ;
                       rdfs:label "S2 Cell Level 11" .


###  http://stko-kwg.geog.ucsb.edu/lod/ontology/KWGCellLevel13
kwg-ont:KWGCellLevel13 rdf:type owl:Class ;
                       rdfs:subClassOf kwg-ont:S2Cell ;
                       rdfs:comment "S2 Cell Level 13" ,
                                    "Source - https://s2geometry.io/" ;
                       rdfs:label "S2 Cell Level 13" .


###  http://stko-kwg.geog.ucsb.edu/lod/ontology/KWGCellLevel9
kwg-ont:KWGCellLevel9 rdf:type owl:Class ;
                      rdfs:subClassOf kwg-ont:S2Cell ;
                      rdfs:comment "S2 Cell Level 9" ,
                                   "Source - https://s2geometry.io/" ;
                      rdfs:label "S2 Cell Level 9" .


###  http://stko-kwg.geog.ucsb.edu/lod/ontology/LSADArea
kwg-ont:LSADArea rdf:type owl:Class ;
                 rdfs:comment "For legal entities, the LSAD reflects the term that appears in legal documentation pertaining to the entity, such as a treaty, charter, legislation, resolution, or ordinance. For statistical entities, the LSAD is the term assigned by the Census Bureau or other agency defining the entity. The LSAD code is a two-character field that corresponds to a description of the legal or statistical type of entity and identifies whether the LSAD term should be capitalized and should precede or follow the name of the geographic entity." ,
                              "Source - US Census Bureau (https://www.census.gov/data/datasets.html)" ;
                 rdfs:label "Legal/Statistical Area Description (LSAD)" .


###  http://stko-kwg.geog.ucsb.edu/lod/ontology/MTBSComplexFire
kwg-ont:MTBSComplexFire rdf:type owl:Class ;
                        rdfs:subClassOf kwg-ont:ComplexFire ,
                                        kwg-ont:MTBSFire ;
                        rdfs:comment "Source - MTBS (https://mtbs.gov/direct-downloadhttps://mtbs.gov/direct-download)" ;
                        rdfs:label "MTBS Complex Fire" .


###  http://stko-kwg.geog.ucsb.edu/lod/ontology/MTBSFire
kwg-ont:MTBSFire rdf:type owl:Class ;
                 rdfs:subClassOf kwg-ont:Fire ,
                                 <http://www.opengis.net/ont/geosparql#Feature> ,
                                 sosa:FeatureOfInterest ;
                 rdfs:comment "Source - MTBS (https://mtbs.gov/direct-downloadhttps://mtbs.gov/direct-download)" ;
                 rdfs:label "MTBS Fire" .


###  http://stko-kwg.geog.ucsb.edu/lod/ontology/MTBSFireObservableProperty
kwg-ont:MTBSFireObservableProperty rdf:type owl:Class ;
                                   rdfs:subClassOf sosa:ObservableProperty ;
                                   rdfs:comment "Source - MTBS (https://mtbs.gov/direct-downloadhttps://mtbs.gov/direct-download)" ;
                                   rdfs:label "MTBS Fire Observable Property" .


###  http://stko-kwg.geog.ucsb.edu/lod/ontology/MTBSFireObservation
kwg-ont:MTBSFireObservation rdf:type owl:Class ;
                            rdfs:subClassOf sosa:Observation ,
                                            [ rdf:type owl:Restriction ;
                                              owl:onProperty sosa:observedProperty ;
                                              owl:allValuesFrom kwg-ont:MTBSFireObservableProperty
                                            ] ;
                            rdfs:comment "Source - MTBS (https://mtbs.gov/direct-downloadhttps://mtbs.gov/direct-download)" ;
                            rdfs:label "MTBS Fire Observation" .


###  http://stko-kwg.geog.ucsb.edu/lod/ontology/MTBSFireObservationCollection
kwg-ont:MTBSFireObservationCollection rdf:type owl:Class ;
                                      rdfs:subClassOf sosa:ObservationCollection ,
                                                      [ rdf:type owl:Restriction ;
                                                        owl:onProperty sosa:hasMember ;
                                                        owl:allValuesFrom kwg-ont:MTBSFireObservation
                                                      ] ,
                                                      [ rdf:type owl:Restriction ;
                                                        owl:onProperty sosa:phenomenonTime ;
                                                        owl:allValuesFrom time:TemporalEntity
                                                      ] ;
                                      rdfs:comment "Source - MTBS (https://mtbs.gov/direct-downloadhttps://mtbs.gov/direct-download)" ;
                                      rdfs:label "MTBS Fire Observation Collection" .


###  http://stko-kwg.geog.ucsb.edu/lod/ontology/MTBSOutOfAreaResponseFire
kwg-ont:MTBSOutOfAreaResponseFire rdf:type owl:Class ;
                                  rdfs:subClassOf kwg-ont:MTBSFire ,
                                                  kwg-ont:OutOfAreaResponseFire ;
                                  rdfs:comment "Source - MTBS (https://mtbs.gov/direct-downloadhttps://mtbs.gov/direct-download)" ;
                                  rdfs:label "MTBS Out Of Area Response Fire" .


###  http://stko-kwg.geog.ucsb.edu/lod/ontology/MTBSPrescribedFire
kwg-ont:MTBSPrescribedFire rdf:type owl:Class ;
                           rdfs:subClassOf kwg-ont:MTBSFire ,
                                           kwg-ont:PrescribedFire ;
                           rdfs:comment "Source - MTBS (https://mtbs.gov/direct-downloadhttps://mtbs.gov/direct-download)" ;
                           rdfs:label "MTBS Prescribed Fire" .


###  http://stko-kwg.geog.ucsb.edu/lod/ontology/MTBSUnknownFire
kwg-ont:MTBSUnknownFire rdf:type owl:Class ;
                        rdfs:subClassOf kwg-ont:MTBSFire ;
                        rdfs:comment "Source - MTBS (https://mtbs.gov/direct-downloadhttps://mtbs.gov/direct-download)" ;
                        rdfs:label "MTBS Unknown Fire" .


###  http://stko-kwg.geog.ucsb.edu/lod/ontology/MTBSWildfire
kwg-ont:MTBSWildfire rdf:type owl:Class ;
                     rdfs:subClassOf kwg-ont:MTBSFire ,
                                     kwg-ont:Wildfire ;
                     rdfs:comment "Source - MTBS (https://mtbs.gov/direct-downloadhttps://mtbs.gov/direct-download)" ;
                     rdfs:label "MTBS Wildfire" .


###  http://stko-kwg.geog.ucsb.edu/lod/ontology/MTBSWildlandFireUse
kwg-ont:MTBSWildlandFireUse rdf:type owl:Class ;
                            rdfs:subClassOf kwg-ont:MTBSFire ,
                                            kwg-ont:WildlandFireUse ;
                            rdfs:comment "Source - MTBS (https://mtbs.gov/direct-downloadhttps://mtbs.gov/direct-download)" ;
                            rdfs:label "MTBS Wildland Fire" .


###  http://stko-kwg.geog.ucsb.edu/lod/ontology/MagnitudeObservableProperty
kwg-ont:MagnitudeObservableProperty rdf:type owl:Class ;
                                    rdfs:subClassOf sosa:ObservableProperty ;
                                    rdfs:comment "Source - NOAA (https://www.ncdc.noaa.gov/stormevents/ftp.jsp)" ;
                                    rdfs:label "Magnitude Obervable Property" .


###  http://stko-kwg.geog.ucsb.edu/lod/ontology/MagnitudeObservation
kwg-ont:MagnitudeObservation rdf:type owl:Class ;
                             rdfs:subClassOf sosa:Observation ,
                                             [ rdf:type owl:Restriction ;
                                               owl:onProperty sosa:observedProperty ;
                                               owl:allValuesFrom kwg-ont:MagnitudeObservableProperty
                                             ] ;
                             rdfs:comment "Source - NOAA (https://www.ncdc.noaa.gov/stormevents/ftp.jsp)" ;
                             rdfs:label "Magnitude Observation" .


###  http://stko-kwg.geog.ucsb.edu/lod/ontology/MagnitudeObservationCollection
kwg-ont:MagnitudeObservationCollection rdf:type owl:Class ;
                                       rdfs:subClassOf sosa:ObservationCollection ,
                                                       [ rdf:type owl:Restriction ;
                                                         owl:onProperty sosa:hasFeatureOfInterest ;
                                                         owl:allValuesFrom kwg-ont:NOAAHazardEvent
                                                       ] ,
                                                       [ rdf:type owl:Restriction ;
                                                         owl:onProperty sosa:hasMember ;
                                                         owl:allValuesFrom kwg-ont:MagnitudeObservation
                                                       ] ,
                                                       [ rdf:type owl:Restriction ;
                                                         owl:onProperty sosa:phenomenonTime ;
                                                         owl:allValuesFrom time:TemporalEntity
                                                       ] ;
                                       rdfs:comment "Source - NOAA (https://www.ncdc.noaa.gov/stormevents/ftp.jsp)" ;
                                       rdfs:label "Magnitude Observation Collection" .


###  http://stko-kwg.geog.ucsb.edu/lod/ontology/MajorDisasterDeclaration
kwg-ont:MajorDisasterDeclaration rdf:type owl:Class ;
                                 rdfs:subClassOf kwg-ont:Declaration ;
                                 rdfs:comment "Source - OpenFEMA (https://www.fema.gov/about/openfema/data-sets)" ;
                                 rdfs:label "Major Disaster Declaration" .


###  http://stko-kwg.geog.ucsb.edu/lod/ontology/MappingProgram
kwg-ont:MappingProgram rdf:type owl:Class ;
                       rdfs:comment "Source - MTBS (https://mtbs.gov/direct-downloadhttps://mtbs.gov/direct-download)" ;
                       rdfs:label "MTBS Mapping Label" .


###  http://stko-kwg.geog.ucsb.edu/lod/ontology/NIFCFire
kwg-ont:NIFCFire rdf:type owl:Class ;
                 rdfs:subClassOf kwg-ont:Fire ,
                                 <http://www.opengis.net/ont/geosparql#Feature> ,
                                 sosa:FeatureOfInterest ;
                 rdfs:comment "Any fire that covers a geographically-significant amount of land." ,
                              "Source - NIFC (https://data-nifc.opendata.arcgis.com/ )" ;
                 rdfs:label "NIFC Fire" .


###  http://stko-kwg.geog.ucsb.edu/lod/ontology/NIFCFireObservableProperty
kwg-ont:NIFCFireObservableProperty rdf:type owl:Class ;
                                   rdfs:subClassOf sosa:ObservableProperty ;
                                   rdfs:comment "Source - NIFC (https://data-nifc.opendata.arcgis.com/ )" ;
                                   rdfs:label "NIFC Fire Observable Property" .


###  http://stko-kwg.geog.ucsb.edu/lod/ontology/NIFCFireObservation
kwg-ont:NIFCFireObservation rdf:type owl:Class ;
                            rdfs:subClassOf sosa:Observation ,
                                            [ rdf:type owl:Restriction ;
                                              owl:onProperty sosa:observedProperty ;
                                              owl:allValuesFrom kwg-ont:NIFCFireObservableProperty
                                            ] ;
                            rdfs:comment "An observation of a fire, extracted from the NIFC historical fire dataset." ,
                                         "Source - NIFC (https://data-nifc.opendata.arcgis.com/ )" ;
                            rdfs:label "NIFC Fire Observation" .


###  http://stko-kwg.geog.ucsb.edu/lod/ontology/NIFCIncidentComplexFire
kwg-ont:NIFCIncidentComplexFire rdf:type owl:Class ;
                                rdfs:subClassOf kwg-ont:ComplexFire ,
                                                kwg-ont:NIFCFire ;
                                rdfs:comment "An incident consisting of multiple fires." ,
                                             "Source - NIFC (https://data-nifc.opendata.arcgis.com/ )" ;
                                rdfs:label "NIFC Incident Complex Fire" .


###  http://stko-kwg.geog.ucsb.edu/lod/ontology/NIFCPrescribedFire
kwg-ont:NIFCPrescribedFire rdf:type owl:Class ;
                           rdfs:subClassOf kwg-ont:NIFCFire ,
                                           kwg-ont:PrescribedFire ;
                           rdfs:comment "An intentionally-set fire." ,
                                        "Source - NIFC (https://data-nifc.opendata.arcgis.com/ )" ;
                           rdfs:label "NIFC Prescribed Fire" .


###  http://stko-kwg.geog.ucsb.edu/lod/ontology/NIFCWildfire
kwg-ont:NIFCWildfire rdf:type owl:Class ;
                     rdfs:subClassOf kwg-ont:NIFCFire ,
                                     kwg-ont:Wildfire ;
                     rdfs:comment "An unintentional fire or a fire that is declared a wildfire" ,
                                  "Source - NIFC (https://data-nifc.opendata.arcgis.com/ )" ;
                     rdfs:label "NIFC Wildfire" .


###  http://stko-kwg.geog.ucsb.edu/lod/ontology/NOAAAstronomicalLowTide
kwg-ont:NOAAAstronomicalLowTide rdf:type owl:Class ;
                                rdfs:subClassOf kwg-ont:NOAAHazardEvent ;
                                rdfs:comment "Source - NOAA (https://www.ncdc.noaa.gov/stormevents/ftp.jsp)" ;
                                rdfs:label "NOAA Astronomical Low Tide" .


###  http://stko-kwg.geog.ucsb.edu/lod/ontology/NOAAAvalanche
kwg-ont:NOAAAvalanche rdf:type owl:Class ;
                      rdfs:subClassOf kwg-ont:NOAAHazardEvent ;
                      rdfs:comment "Source - NOAA (https://www.ncdc.noaa.gov/stormevents/ftp.jsp)" ;
                      rdfs:label "NOAA Avalanche" .


###  http://stko-kwg.geog.ucsb.edu/lod/ontology/NOAABlizzard
kwg-ont:NOAABlizzard rdf:type owl:Class ;
                     rdfs:subClassOf kwg-ont:NOAAHazardEvent ;
                     rdfs:comment "Source - NOAA (https://www.ncdc.noaa.gov/stormevents/ftp.jsp)" ;
                     rdfs:label "NOAA Blizzard" .


###  http://stko-kwg.geog.ucsb.edu/lod/ontology/NOAACoastalFlood
kwg-ont:NOAACoastalFlood rdf:type owl:Class ;
                         rdfs:subClassOf kwg-ont:NOAAHazardEvent ;
                         rdfs:comment "Source - NOAA (https://www.ncdc.noaa.gov/stormevents/ftp.jsp)" ;
                         rdfs:label "NOAA Coastal Flood" .


###  http://stko-kwg.geog.ucsb.edu/lod/ontology/NOAAColdWindChill
kwg-ont:NOAAColdWindChill rdf:type owl:Class ;
                          rdfs:subClassOf kwg-ont:NOAAHazardEvent ;
                          rdfs:comment "Source - NOAA (https://www.ncdc.noaa.gov/stormevents/ftp.jsp)" ;
                          rdfs:label "NOAA Cold/Wind Chill" .


###  http://stko-kwg.geog.ucsb.edu/lod/ontology/NOAADebrisFlow
kwg-ont:NOAADebrisFlow rdf:type owl:Class ;
                       rdfs:subClassOf kwg-ont:NOAAHazardEvent ;
                       rdfs:comment "Source - NOAA (https://www.ncdc.noaa.gov/stormevents/ftp.jsp)" ;
                       rdfs:label "NOAA Debris Flow" .


###  http://stko-kwg.geog.ucsb.edu/lod/ontology/NOAADenseFog
kwg-ont:NOAADenseFog rdf:type owl:Class ;
                     rdfs:subClassOf kwg-ont:NOAAHazardEvent ;
                     rdfs:comment "Source - NOAA (https://www.ncdc.noaa.gov/stormevents/ftp.jsp)" ;
                     rdfs:label "NOAA Dense Fog" .


###  http://stko-kwg.geog.ucsb.edu/lod/ontology/NOAADenseSmoke
kwg-ont:NOAADenseSmoke rdf:type owl:Class ;
                       rdfs:subClassOf kwg-ont:NOAAHazardEvent ;
                       rdfs:comment "Source - NOAA (https://www.ncdc.noaa.gov/stormevents/ftp.jsp)" ;
                       rdfs:label "NOAA Dense Smoke" .


###  http://stko-kwg.geog.ucsb.edu/lod/ontology/NOAADrought
kwg-ont:NOAADrought rdf:type owl:Class ;
                    rdfs:subClassOf kwg-ont:NOAAHazardEvent ;
                    rdfs:comment "Source - NOAA (https://www.ncdc.noaa.gov/stormevents/ftp.jsp)" ;
                    rdfs:label "NOAA Drought" .


###  http://stko-kwg.geog.ucsb.edu/lod/ontology/NOAADustDevil
kwg-ont:NOAADustDevil rdf:type owl:Class ;
                      rdfs:subClassOf kwg-ont:NOAAHazardEvent ;
                      rdfs:comment "Source - NOAA (https://www.ncdc.noaa.gov/stormevents/ftp.jsp)" ;
                      rdfs:label "NOAA Dust Devil" .


###  http://stko-kwg.geog.ucsb.edu/lod/ontology/NOAADustStorm
kwg-ont:NOAADustStorm rdf:type owl:Class ;
                      rdfs:subClassOf kwg-ont:NOAAHazardEvent ;
                      rdfs:comment "Source - NOAA (https://www.ncdc.noaa.gov/stormevents/ftp.jsp)" ;
                      rdfs:label "NOAA Dust Storm" .


###  http://stko-kwg.geog.ucsb.edu/lod/ontology/NOAAExcessiveHeat
kwg-ont:NOAAExcessiveHeat rdf:type owl:Class ;
                          rdfs:subClassOf kwg-ont:NOAAHazardEvent ;
                          rdfs:comment "Source - NOAA (https://www.ncdc.noaa.gov/stormevents/ftp.jsp)" ;
                          rdfs:label "NOAA Excessive Heat" .


###  http://stko-kwg.geog.ucsb.edu/lod/ontology/NOAAExtremeColdWindChill
kwg-ont:NOAAExtremeColdWindChill rdf:type owl:Class ;
                                 rdfs:subClassOf kwg-ont:NOAAHazardEvent ;
                                 rdfs:comment "Source - NOAA (https://www.ncdc.noaa.gov/stormevents/ftp.jsp)" ;
                                 rdfs:label "NOAA Extreme Cold/Wind Chill" .


###  http://stko-kwg.geog.ucsb.edu/lod/ontology/NOAAFlashFlood
kwg-ont:NOAAFlashFlood rdf:type owl:Class ;
                       rdfs:subClassOf kwg-ont:NOAAHazardEvent ;
                       rdfs:comment "Source - NOAA (https://www.ncdc.noaa.gov/stormevents/ftp.jsp)" ;
                       rdfs:label "NOAA Flash Flood" .


###  http://stko-kwg.geog.ucsb.edu/lod/ontology/NOAAFlood
kwg-ont:NOAAFlood rdf:type owl:Class ;
                  rdfs:subClassOf kwg-ont:NOAAHazardEvent ;
                  rdfs:comment "Source - NOAA (https://www.ncdc.noaa.gov/stormevents/ftp.jsp)" ;
                  rdfs:label "NOAA Flood" .


###  http://stko-kwg.geog.ucsb.edu/lod/ontology/NOAAFreezingFog
kwg-ont:NOAAFreezingFog rdf:type owl:Class ;
                        rdfs:subClassOf kwg-ont:NOAAHazardEvent ;
                        rdfs:comment "Source - NOAA (https://www.ncdc.noaa.gov/stormevents/ftp.jsp)" ;
                        rdfs:label "NOAA Freezing Fog" .


###  http://stko-kwg.geog.ucsb.edu/lod/ontology/NOAAFrostFreeze
kwg-ont:NOAAFrostFreeze rdf:type owl:Class ;
                        rdfs:subClassOf kwg-ont:NOAAHazardEvent ;
                        rdfs:comment "Source - NOAA (https://www.ncdc.noaa.gov/stormevents/ftp.jsp)" ;
                        rdfs:label "NOAA Frost/Freeze" .


###  http://stko-kwg.geog.ucsb.edu/lod/ontology/NOAAFunnelCloud
kwg-ont:NOAAFunnelCloud rdf:type owl:Class ;
                        rdfs:subClassOf kwg-ont:NOAAHazardEvent ;
                        rdfs:comment "Source - NOAA (https://www.ncdc.noaa.gov/stormevents/ftp.jsp)" ;
                        rdfs:label "NOAA Funnel Cloud" .


###  http://stko-kwg.geog.ucsb.edu/lod/ontology/NOAAHail
kwg-ont:NOAAHail rdf:type owl:Class ;
                 rdfs:subClassOf kwg-ont:NOAAHazardEvent ;
                 rdfs:comment "Source - NOAA (https://www.ncdc.noaa.gov/stormevents/ftp.jsp)" ;
                 rdfs:label "NOAA Hail" .


###  http://stko-kwg.geog.ucsb.edu/lod/ontology/NOAAHazard
kwg-ont:NOAAHazard rdf:type owl:Class ;
                   rdfs:comment "This is also the general NOAA Hurricane class that carries the distinct named hurricane instances." ;
                   rdfs:label "NOAA Hazard" .


###  http://stko-kwg.geog.ucsb.edu/lod/ontology/NOAAHazardEvent
kwg-ont:NOAAHazardEvent rdf:type owl:Class ;
                        rdfs:subClassOf kwg-ont:Hazard ,
                                        <http://www.opengis.net/ont/geosparql#Feature> ,
                                        sosa:FeatureOfInterest ,
                                        <https://undrr.org/hazard/hip/MetereologicalAndHydrological> ;
                        rdfs:comment "Source - NOAA (https://www.ncdc.noaa.gov/stormevents/ftp.jsp)" ;
                        rdfs:label "NOAA Hazard Event" .


###  http://stko-kwg.geog.ucsb.edu/lod/ontology/NOAAHeat
kwg-ont:NOAAHeat rdf:type owl:Class ;
                 rdfs:subClassOf kwg-ont:NOAAHazardEvent ;
                 rdfs:comment "Source - NOAA (https://www.ncdc.noaa.gov/stormevents/ftp.jsp)" ;
                 rdfs:label "NOAA Heat" .


###  http://stko-kwg.geog.ucsb.edu/lod/ontology/NOAAHeavyRain
kwg-ont:NOAAHeavyRain rdf:type owl:Class ;
                      rdfs:subClassOf kwg-ont:NOAAHazardEvent ;
                      rdfs:comment "Source - NOAA (https://www.ncdc.noaa.gov/stormevents/ftp.jsp)" ;
                      rdfs:label "NOAA Heavy Rain" .


###  http://stko-kwg.geog.ucsb.edu/lod/ontology/NOAAHeavySnow
kwg-ont:NOAAHeavySnow rdf:type owl:Class ;
                      rdfs:subClassOf kwg-ont:NOAAHazardEvent ;
                      rdfs:comment "Source - NOAA (https://www.ncdc.noaa.gov/stormevents/ftp.jsp)" ;
                      rdfs:label "NOAA Heavy Snow" .


###  http://stko-kwg.geog.ucsb.edu/lod/ontology/NOAAHighSurf
kwg-ont:NOAAHighSurf rdf:type owl:Class ;
                     rdfs:subClassOf kwg-ont:NOAAHazardEvent ;
                     rdfs:comment "Source - NOAA (https://www.ncdc.noaa.gov/stormevents/ftp.jsp)" ;
                     rdfs:label "NOAA High Surf" .


###  http://stko-kwg.geog.ucsb.edu/lod/ontology/NOAAHighWind
kwg-ont:NOAAHighWind rdf:type owl:Class ;
                     rdfs:subClassOf kwg-ont:NOAAHazardEvent ;
                     rdfs:comment "Source - NOAA (https://www.ncdc.noaa.gov/stormevents/ftp.jsp)" ;
                     rdfs:label "NOAA High Wind" .


###  http://stko-kwg.geog.ucsb.edu/lod/ontology/NOAAHurricane
kwg-ont:NOAAHurricane rdf:type owl:Class ;
                      rdfs:subClassOf kwg-ont:NOAAHazardEvent ;
                      rdfs:comment "Source - NOAA (https://www.ncdc.noaa.gov/stormevents/ftp.jsp)" ;
                      rdfs:label "NOAA Hurricane" .


###  http://stko-kwg.geog.ucsb.edu/lod/ontology/NOAAIceStorm
kwg-ont:NOAAIceStorm rdf:type owl:Class ;
                     rdfs:subClassOf kwg-ont:NOAAHazardEvent ;
                     rdfs:comment "Source - NOAA (https://www.ncdc.noaa.gov/stormevents/ftp.jsp)" ;
                     rdfs:label "NOAA Ice Storm" .


###  http://stko-kwg.geog.ucsb.edu/lod/ontology/NOAALake-EffectSnow
kwg-ont:NOAALake-EffectSnow rdf:type owl:Class ;
                            rdfs:subClassOf kwg-ont:NOAAHazardEvent ;
                            rdfs:comment "Source - NOAA (https://www.ncdc.noaa.gov/stormevents/ftp.jsp)" ;
                            rdfs:label "NOAA Lake-Effect Snow" .


###  http://stko-kwg.geog.ucsb.edu/lod/ontology/NOAALakeshoreFlood
kwg-ont:NOAALakeshoreFlood rdf:type owl:Class ;
                           rdfs:subClassOf kwg-ont:NOAAHazardEvent ;
                           rdfs:comment "Source - NOAA (https://www.ncdc.noaa.gov/stormevents/ftp.jsp)" ;
                           rdfs:label "NOAA Lakeshore Flood" .


###  http://stko-kwg.geog.ucsb.edu/lod/ontology/NOAALightning
kwg-ont:NOAALightning rdf:type owl:Class ;
                      rdfs:subClassOf kwg-ont:NOAAHazardEvent ;
                      rdfs:comment "Source - NOAA (https://www.ncdc.noaa.gov/stormevents/ftp.jsp)" ;
                      rdfs:label "NOAA Lightning" .


###  http://stko-kwg.geog.ucsb.edu/lod/ontology/NOAAMarineHail
kwg-ont:NOAAMarineHail rdf:type owl:Class ;
                       rdfs:subClassOf kwg-ont:NOAAHazardEvent ;
                       rdfs:comment "Source - NOAA (https://www.ncdc.noaa.gov/stormevents/ftp.jsp)" ;
                       rdfs:label "NOAA Marine Hail" .


###  http://stko-kwg.geog.ucsb.edu/lod/ontology/NOAAMarineHighWind
kwg-ont:NOAAMarineHighWind rdf:type owl:Class ;
                           rdfs:subClassOf kwg-ont:NOAAHazardEvent ;
                           rdfs:comment "Source - NOAA (https://www.ncdc.noaa.gov/stormevents/ftp.jsp)" ;
                           rdfs:label "NOAA Marine High Wind" .


###  http://stko-kwg.geog.ucsb.edu/lod/ontology/NOAAMarineHurricaneTyphoon
kwg-ont:NOAAMarineHurricaneTyphoon rdf:type owl:Class ;
                                   rdfs:subClassOf kwg-ont:NOAAHazardEvent ;
                                   rdfs:comment "Source - NOAA (https://www.ncdc.noaa.gov/stormevents/ftp.jsp)" ;
                                   rdfs:label "NOAA Marine Hurricane/Typhoon" .


###  http://stko-kwg.geog.ucsb.edu/lod/ontology/NOAAMarineStrongWind
kwg-ont:NOAAMarineStrongWind rdf:type owl:Class ;
                             rdfs:subClassOf kwg-ont:NOAAHazardEvent ;
                             rdfs:comment "Source - NOAA (https://www.ncdc.noaa.gov/stormevents/ftp.jsp)" ;
                             rdfs:label "NOAA Marine Strong Wind" .


###  http://stko-kwg.geog.ucsb.edu/lod/ontology/NOAAMarineThunderstormWind
kwg-ont:NOAAMarineThunderstormWind rdf:type owl:Class ;
                                   rdfs:subClassOf kwg-ont:NOAAHazardEvent ;
                                   rdfs:comment "Source - NOAA (https://www.ncdc.noaa.gov/stormevents/ftp.jsp)" ;
                                   rdfs:label "NOAA Marine Thunderstorm Wind" .


###  http://stko-kwg.geog.ucsb.edu/lod/ontology/NOAAMarineTropicalDepression
kwg-ont:NOAAMarineTropicalDepression rdf:type owl:Class ;
                                     rdfs:subClassOf kwg-ont:NOAAHazardEvent ;
                                     rdfs:comment "Source - NOAA (https://www.ncdc.noaa.gov/stormevents/ftp.jsp)" ;
                                     rdfs:label "NOAA Marine Tropical Depression" .


###  http://stko-kwg.geog.ucsb.edu/lod/ontology/NOAAMarineTropicalStorm
kwg-ont:NOAAMarineTropicalStorm rdf:type owl:Class ;
                                rdfs:subClassOf kwg-ont:NOAAHazardEvent ;
                                rdfs:comment "Source - NOAA (https://www.ncdc.noaa.gov/stormevents/ftp.jsp)" ;
                                rdfs:label "NOAA Marine Tropical Storm" .


###  http://stko-kwg.geog.ucsb.edu/lod/ontology/NOAARipCurrent
kwg-ont:NOAARipCurrent rdf:type owl:Class ;
                       rdfs:subClassOf kwg-ont:NOAAHazardEvent ;
                       rdfs:comment "Source - NOAA (https://www.ncdc.noaa.gov/stormevents/ftp.jsp)" ;
                       rdfs:label "NOAA Rip Current" .


###  http://stko-kwg.geog.ucsb.edu/lod/ontology/NOAASleet
kwg-ont:NOAASleet rdf:type owl:Class ;
                  rdfs:subClassOf kwg-ont:NOAAHazardEvent ;
                  rdfs:comment "Source - NOAA (https://www.ncdc.noaa.gov/stormevents/ftp.jsp)" ;
                  rdfs:label "NOAA Sleet" .


###  http://stko-kwg.geog.ucsb.edu/lod/ontology/NOAASneakerwave
kwg-ont:NOAASneakerwave rdf:type owl:Class ;
                        rdfs:subClassOf kwg-ont:NOAAHazardEvent ;
                        rdfs:comment "Source - NOAA (https://www.ncdc.noaa.gov/stormevents/ftp.jsp)" ;
                        rdfs:label "NOAA Sneakerwave" .


###  http://stko-kwg.geog.ucsb.edu/lod/ontology/NOAAStormSurgeTide
kwg-ont:NOAAStormSurgeTide rdf:type owl:Class ;
                           rdfs:subClassOf kwg-ont:NOAAHazardEvent ;
                           rdfs:comment "Source - NOAA (https://www.ncdc.noaa.gov/stormevents/ftp.jsp)" ;
                           rdfs:label "NOAA Storm Surge/Tide" .


###  http://stko-kwg.geog.ucsb.edu/lod/ontology/NOAAStrongWind
kwg-ont:NOAAStrongWind rdf:type owl:Class ;
                       rdfs:subClassOf kwg-ont:NOAAHazardEvent ;
                       rdfs:comment "Source - NOAA (https://www.ncdc.noaa.gov/stormevents/ftp.jsp)" ;
                       rdfs:label "NOAA Strong Wind" .


###  http://stko-kwg.geog.ucsb.edu/lod/ontology/NOAAThunderstormWind
kwg-ont:NOAAThunderstormWind rdf:type owl:Class ;
                             rdfs:subClassOf kwg-ont:NOAAHazardEvent ;
                             rdfs:comment "Source - NOAA (https://www.ncdc.noaa.gov/stormevents/ftp.jsp)" ;
                             rdfs:label "NOAA Thunderstorm Wind" .


###  http://stko-kwg.geog.ucsb.edu/lod/ontology/NOAATornado
kwg-ont:NOAATornado rdf:type owl:Class ;
                    rdfs:subClassOf kwg-ont:NOAAHazardEvent ;
                    rdfs:comment "Source - NOAA (https://www.ncdc.noaa.gov/stormevents/ftp.jsp)" ;
                    rdfs:label "NOAA Tornado" .


###  http://stko-kwg.geog.ucsb.edu/lod/ontology/NOAATropicalDepression
kwg-ont:NOAATropicalDepression rdf:type owl:Class ;
                               rdfs:subClassOf kwg-ont:NOAAHazardEvent ;
                               rdfs:comment "Source - NOAA (https://www.ncdc.noaa.gov/stormevents/ftp.jsp)" ;
                               rdfs:label "NOAA Tropical Depression" .


###  http://stko-kwg.geog.ucsb.edu/lod/ontology/NOAATropicalStorm
kwg-ont:NOAATropicalStorm rdf:type owl:Class ;
                          rdfs:subClassOf kwg-ont:NOAAHazardEvent ;
                          rdfs:comment "Source - NOAA (https://www.ncdc.noaa.gov/stormevents/ftp.jsp)" ;
                          rdfs:label "NOAA Tropical Storm" .


###  http://stko-kwg.geog.ucsb.edu/lod/ontology/NOAAWaterspout
kwg-ont:NOAAWaterspout rdf:type owl:Class ;
                       rdfs:subClassOf kwg-ont:NOAAHazardEvent ;
                       rdfs:comment "Source - NOAA (https://www.ncdc.noaa.gov/stormevents/ftp.jsp)" ;
                       rdfs:label "NOAA Waterspout" .


###  http://stko-kwg.geog.ucsb.edu/lod/ontology/NOAAWildfire
kwg-ont:NOAAWildfire rdf:type owl:Class ;
                     rdfs:subClassOf kwg-ont:NOAAHazardEvent ,
                                     kwg-ont:Wildfire ;
                     rdfs:comment "Source - NOAA (https://www.ncdc.noaa.gov/stormevents/ftp.jsp)" ;
                     rdfs:label "NOAA Wildfire" .


###  http://stko-kwg.geog.ucsb.edu/lod/ontology/NOAAWinterStorm
kwg-ont:NOAAWinterStorm rdf:type owl:Class ;
                        rdfs:subClassOf kwg-ont:NOAAHazardEvent ;
                        rdfs:comment "Source - NOAA (https://www.ncdc.noaa.gov/stormevents/ftp.jsp)" ;
                        rdfs:label "NOAA Winter Storm" .


###  http://stko-kwg.geog.ucsb.edu/lod/ontology/NOAAWinterWeather
kwg-ont:NOAAWinterWeather rdf:type owl:Class ;
                          rdfs:subClassOf kwg-ont:NOAAHazardEvent ;
                          rdfs:comment "Source - NOAA (https://www.ncdc.noaa.gov/stormevents/ftp.jsp)" ;
                          rdfs:label "NOAA Winter Weather" .


###  http://stko-kwg.geog.ucsb.edu/lod/ontology/NWZone
kwg-ont:NWZone rdf:type owl:Class ;
               rdfs:subClassOf kwg-ont:Region ,
                               <http://www.opengis.net/ont/geosparql#Feature> ,
                               [ rdf:type owl:Restriction ;
                                 owl:onProperty kwg-ont:spatialRelation ;
                                 owl:someValuesFrom kwg-ont:AdministrativeRegion_3
                               ] ,
                               [ rdf:type owl:Restriction ;
                                 owl:onProperty kwg-ont:spatialRelation ;
                                 owl:someValuesFrom kwg-ont:S2Cell
                               ] ,
                               [ rdf:type owl:Restriction ;
                                 owl:onProperty <http://www.opengis.net/ont/geosparql#hasDefaultGeometry> ;
                                 owl:allValuesFrom <http://www.opengis.net/ont/geosparql#Geometry>
                               ] ,
                               [ rdf:type owl:Restriction ;
                                 owl:onProperty <http://www.opengis.net/ont/geosparql#hasGeometry> ;
                                 owl:allValuesFrom <http://www.opengis.net/ont/geosparql#Geometry>
                               ] ;
               rdfs:comment "Source - https://www.weather.gov/gis/PublicZones" ;
               rdfs:label "National Weather Zone" .


###  http://stko-kwg.geog.ucsb.edu/lod/ontology/NielsenMarketZone
kwg-ont:NielsenMarketZone rdf:type owl:Class ;
                          rdfs:subClassOf kwg-ont:Region ,
                                          <http://www.opengis.net/ont/geosparql#Feature> ,
                                          [ rdf:type owl:Restriction ;
                                            owl:onProperty kwg-ont:spatialRelation ;
                                            owl:someValuesFrom kwg-ont:AdministrativeRegion_3
                                          ] ,
                                          [ rdf:type owl:Restriction ;
                                            owl:onProperty kwg-ont:spatialRelation ;
                                            owl:someValuesFrom kwg-ont:S2Cell
                                          ] ,
                                          [ rdf:type owl:Restriction ;
                                            owl:onProperty <http://www.opengis.net/ont/geosparql#hasDefaultGeometry> ;
                                            owl:allValuesFrom <http://www.opengis.net/ont/geosparql#Geometry>
                                          ] ,
                                          [ rdf:type owl:Restriction ;
                                            owl:onProperty <http://www.opengis.net/ont/geosparql#hasGeometry> ;
                                            owl:allValuesFrom <http://www.opengis.net/ont/geosparql#Geometry>
                                          ] ;
                          rdfs:comment "DMA (Designated Market Area) regions are the geographic areas in the U.S. in which local television viewing is measured by Nielsen." ,
                                       "Source - Nielsen (https://www.nielsen.com/us/en/contact-us/intl-campaigns/dma-maps/)" ;
                          rdfs:label "Nielsen Market Zone" .


###  http://stko-kwg.geog.ucsb.edu/lod/ontology/Other
kwg-ont:Other rdf:type owl:Class ;
              rdfs:subClassOf kwg-ont:Program ;
              rdfs:comment "Source - OpenFEMA (https://www.fema.gov/about/openfema/data-sets)" ;
              rdfs:label "Other" .


###  http://stko-kwg.geog.ucsb.edu/lod/ontology/OutOfAreaResponseFire
kwg-ont:OutOfAreaResponseFire rdf:type owl:Class ;
                              rdfs:subClassOf kwg-ont:Fire ;
                              rdfs:label "Out Of Area Response Fire" .


###  http://stko-kwg.geog.ucsb.edu/lod/ontology/Pharmacy
kwg-ont:Pharmacy rdf:type owl:Class ;
                 rdfs:subClassOf kwg-ont:HealthCareFacility ,
                                 [ rdf:type owl:Restriction ;
                                   owl:onProperty kwg-ont:sfWithin ;
                                   owl:someValuesFrom kwg-ont:AdministrativeRegion
                                 ] ,
                                 [ rdf:type owl:Restriction ;
                                   owl:onProperty kwg-ont:spatialRelation ;
                                   owl:someValuesFrom kwg-ont:S2Cell
                                 ] ,
                                 [ rdf:type owl:Restriction ;
                                   owl:onProperty <http://www.opengis.net/ont/geosparql#hasDefaultGeometry> ;
                                   owl:allValuesFrom <http://www.opengis.net/ont/geosparql#Geometry>
                                 ] ,
                                 [ rdf:type owl:Restriction ;
                                   owl:onProperty <http://www.opengis.net/ont/geosparql#hasGeometry> ;
                                   owl:allValuesFrom <http://www.opengis.net/ont/geosparql#Geometry>
                                 ] ;
                 rdfs:comment "https://hifld-geoplatform.opendata.arcgis.com/documents/geoplatform::pharmacies/about" ;
                 rdfs:label "Pharmacy" .


###  http://stko-kwg.geog.ucsb.edu/lod/ontology/PharmacyType
kwg-ont:PharmacyType rdf:type owl:Class ;
                     rdfs:comment "https://hifld-geoplatform.opendata.arcgis.com/documents/geoplatform::pharmacies/about" ;
                     rdfs:label "Pharmacy Type" .


###  http://stko-kwg.geog.ucsb.edu/lod/ontology/PrescribedFire
kwg-ont:PrescribedFire rdf:type owl:Class ;
                       rdfs:subClassOf kwg-ont:Fire ;
                       rdfs:label "Prescribed Fire" .


###  http://stko-kwg.geog.ucsb.edu/lod/ontology/Program
kwg-ont:Program rdf:type owl:Class ;
                rdfs:comment "Source - OpenFEMA (https://www.fema.gov/about/openfema/data-sets)" ,
                             "The class that is used to denote all relief/assistance programs in the OpenFEMA dataset" ;
                rdfs:label "Program" .


###  http://stko-kwg.geog.ucsb.edu/lod/ontology/ProtectiveMeasures-PA-B
kwg-ont:ProtectiveMeasures-PA-B rdf:type owl:Class ;
                                rdfs:subClassOf kwg-ont:PublicAssistance ;
                                rdfs:comment "Source - OpenFEMA (https://www.fema.gov/about/openfema/data-sets)" ;
                                rdfs:label "Protective Measures (PA-B)" .


###  http://stko-kwg.geog.ucsb.edu/lod/ontology/PublicAssistance
kwg-ont:PublicAssistance rdf:type owl:Class ;
                         rdfs:subClassOf kwg-ont:Program ;
                         rdfs:comment "Source - OpenFEMA (https://www.fema.gov/about/openfema/data-sets)" ;
                         rdfs:label "Public Assistance" .


###  http://stko-kwg.geog.ucsb.edu/lod/ontology/PublicBuildings-PA-F
kwg-ont:PublicBuildings-PA-F rdf:type owl:Class ;
                             rdfs:subClassOf kwg-ont:PublicAssistance ;
                             rdfs:comment "Source - OpenFEMA (https://www.fema.gov/about/openfema/data-sets)" ;
                             rdfs:label "Public Buildings (PA-F)" .


###  http://stko-kwg.geog.ucsb.edu/lod/ontology/PublicHealthDepartment
kwg-ont:PublicHealthDepartment rdf:type owl:Class ;
                               rdfs:subClassOf kwg-ont:HealthCareFacility ,
                                               [ rdf:type owl:Restriction ;
                                                 owl:onProperty kwg-ont:sfWithin ;
                                                 owl:someValuesFrom kwg-ont:AdministrativeRegion
                                               ] ,
                                               [ rdf:type owl:Restriction ;
                                                 owl:onProperty kwg-ont:spatialRelation ;
                                                 owl:someValuesFrom kwg-ont:S2Cell
                                               ] ,
                                               [ rdf:type owl:Restriction ;
                                                 owl:onProperty <http://www.opengis.net/ont/geosparql#hasDefaultGeometry> ;
                                                 owl:allValuesFrom <http://www.opengis.net/ont/geosparql#Geometry>
                                               ] ,
                                               [ rdf:type owl:Restriction ;
                                                 owl:onProperty <http://www.opengis.net/ont/geosparql#hasGeometry> ;
                                                 owl:allValuesFrom <http://www.opengis.net/ont/geosparql#Geometry>
                                               ] ;
                               rdfs:comment "https://hifld-geoplatform.opendata.arcgis.com/datasets/geoplatform::public-health-departments/about" ;
                               rdfs:label "Public Health Department" .


###  http://stko-kwg.geog.ucsb.edu/lod/ontology/PublicHealthObservableProperty
kwg-ont:PublicHealthObservableProperty rdf:type owl:Class ;
                                       rdfs:subClassOf sosa:ObservableProperty ;
                                       rdfs:comment "Source - https://nccd.cdc.gov/DHDSPAtlas/?state=County" ;
                                       rdfs:label "Public Health Observable Property" .


###  http://stko-kwg.geog.ucsb.edu/lod/ontology/PublicHealthObservation
kwg-ont:PublicHealthObservation rdf:type owl:Class ;
                                rdfs:subClassOf sosa:Observation ,
                                                [ rdf:type owl:Restriction ;
                                                  owl:onProperty sosa:observedProperty ;
                                                  owl:allValuesFrom kwg-ont:PublicHealthObservableProperty
                                                ] ;
                                rdfs:comment "Source - https://nccd.cdc.gov/DHDSPAtlas/?state=County" ;
                                rdfs:label "Public Health Observation" .


###  http://stko-kwg.geog.ucsb.edu/lod/ontology/PublicHealthObservationCollection
kwg-ont:PublicHealthObservationCollection rdf:type owl:Class ;
                                          rdfs:subClassOf sosa:ObservationCollection ,
                                                          [ rdf:type owl:Restriction ;
                                                            owl:onProperty sosa:hasFeatureOfInterest ;
                                                            owl:allValuesFrom kwg-ont:AdministrativeRegion_3
                                                          ] ,
                                                          [ rdf:type owl:Restriction ;
                                                            owl:onProperty sosa:hasMember ;
                                                            owl:allValuesFrom kwg-ont:PublicHealthObservation
                                                          ] ,
                                                          [ rdf:type owl:Restriction ;
                                                            owl:onProperty sosa:phenomenonTime ;
                                                            owl:allValuesFrom time:TemporalEntity
                                                          ] ;
                                          rdfs:comment "Source - https://nccd.cdc.gov/DHDSPAtlas/?state=County" ;
                                          rdfs:label "Public Health Observation Collection" .


###  http://stko-kwg.geog.ucsb.edu/lod/ontology/PublicUtilitiesPA-G
kwg-ont:PublicUtilitiesPA-G rdf:type owl:Class ;
                            rdfs:subClassOf kwg-ont:PublicAssistance ;
                            rdfs:comment "Source - OpenFEMA (https://www.fema.gov/about/openfema/data-sets)" ;
                            rdfs:label "Public Utilities (PA-G)" .


###  http://stko-kwg.geog.ucsb.edu/lod/ontology/Quantity
kwg-ont:Quantity rdf:type owl:Class ;
                 rdfs:subClassOf <http://qudt.org/2.1/schema/qudt#QuantityValue> .


###  http://stko-kwg.geog.ucsb.edu/lod/ontology/RecreationalOrOther-PA-H
kwg-ont:RecreationalOrOther-PA-H rdf:type owl:Class ;
                                 rdfs:subClassOf kwg-ont:PublicAssistance ;
                                 rdfs:comment "Source - OpenFEMA (https://www.fema.gov/about/openfema/data-sets)" ;
                                 rdfs:label "Recreational or Other (PA-H)" .


###  http://stko-kwg.geog.ucsb.edu/lod/ontology/Region
kwg-ont:Region rdf:type owl:Class ;
               rdfs:comment "A geographic entity created by the selection of characteristics that are relevant to an area of interest. It can have geometries including point, polyline and polygon." ;
               rdfs:label "Region" .


###  http://stko-kwg.geog.ucsb.edu/lod/ontology/RegionalCircuit
kwg-ont:RegionalCircuit rdf:type owl:Class ;
                        rdfs:comment "Source - HIFLD (https://hifld-geoplatform.opendata.arcgis.com/datasets/us-district-court-jurisdictions/explore?location=40.830482%2C-90.571266%2C4.68, https://www.uscourts.gov/about-federal-courts/federal-courts-public/court-website-links)" ;
                        rdfs:label "Regional Circuit" .


###  http://stko-kwg.geog.ucsb.edu/lod/ontology/RoadSegment
kwg-ont:RoadSegment rdf:type owl:Class ;
                    rdfs:subClassOf <http://www.opengis.net/ont/geosparql#Feature> ,
                                    [ rdf:type owl:Restriction ;
                                      owl:onProperty kwg-ont:sfTouches ;
                                      owl:someValuesFrom kwg-ont:RoadSegment
                                    ] ,
                                    [ rdf:type owl:Restriction ;
                                      owl:onProperty kwg-ont:spatialRelation ;
                                      owl:someValuesFrom kwg-ont:AdministrativeRegion_3
                                    ] ,
                                    [ rdf:type owl:Restriction ;
                                      owl:onProperty kwg-ont:spatialRelation ;
                                      owl:someValuesFrom kwg-ont:S2Cell
                                    ] ,
                                    [ rdf:type owl:Restriction ;
                                      owl:onProperty <http://www.opengis.net/ont/geosparql#hasDefaultGeometry> ;
                                      owl:allValuesFrom <http://www.opengis.net/ont/geosparql#Geometry>
                                    ] ,
                                    [ rdf:type owl:Restriction ;
                                      owl:onProperty <http://www.opengis.net/ont/geosparql#hasGeometry> ;
                                      owl:allValuesFrom <http://www.opengis.net/ont/geosparql#Geometry>
                                    ] ;
                    rdfs:comment "Source - https://data-usdot.opendata.arcgis.com/datasets/usdot::national-highway-planning-network/about" ;
                    rdfs:label "Road Segment" .


###  http://stko-kwg.geog.ucsb.edu/lod/ontology/RoadSegmentNode
kwg-ont:RoadSegmentNode rdf:type owl:Class ;
                        rdfs:subClassOf <http://www.opengis.net/ont/geosparql#Feature> ,
                                        [ rdf:type owl:Restriction ;
                                          owl:onProperty <http://www.opengis.net/ont/geosparql#hasDefaultGeometry> ;
                                          owl:allValuesFrom <http://www.opengis.net/ont/geosparql#Geometry>
                                        ] ,
                                        [ rdf:type owl:Restriction ;
                                          owl:onProperty <http://www.opengis.net/ont/geosparql#hasGeometry> ;
                                          owl:allValuesFrom <http://www.opengis.net/ont/geosparql#Geometry>
                                        ] ;
                        rdfs:comment "Source - https://data-usdot.opendata.arcgis.com/datasets/usdot::national-highway-planning-network/about" ;
                        rdfs:label "Road Segment Node" .


###  http://stko-kwg.geog.ucsb.edu/lod/ontology/RoadType
kwg-ont:RoadType rdf:type owl:Class ;
                 rdfs:comment "Source - https://www.census.gov/library/reference/code-lists/route-type-codes.html" ;
                 rdfs:label "Road Type" .


###  http://stko-kwg.geog.ucsb.edu/lod/ontology/RoadsAndBridges-PA-D
kwg-ont:RoadsAndBridges-PA-D rdf:type owl:Class ;
                             rdfs:subClassOf kwg-ont:PublicAssistance ;
                             rdfs:comment "Source - OpenFEMA (https://www.fema.gov/about/openfema/data-sets)" ;
                             rdfs:label "Roads & Bridges (PA-D)" .


###  http://stko-kwg.geog.ucsb.edu/lod/ontology/S2Cell
kwg-ont:S2Cell rdf:type owl:Class ;
               rdfs:subClassOf kwg-ont:Cell ,
                               sosa:FeatureOfInterest ,
                               [ rdf:type owl:Restriction ;
                                 owl:onProperty <http://www.opengis.net/ont/geosparql#hasDefaultGeometry> ;
                                 owl:allValuesFrom <http://www.opengis.net/ont/geosparql#Geometry>
                               ] ,
                               [ rdf:type owl:Restriction ;
                                 owl:onProperty <http://www.opengis.net/ont/geosparql#hasGeometry> ;
                                 owl:allValuesFrom <http://www.opengis.net/ont/geosparql#Geometry>
                               ] ;
               rdfs:comment "S2 Cell" ,
                            "Source - https://s2geometry.io/" ;
               rdfs:label "S2 Cell" .


###  http://stko-kwg.geog.ucsb.edu/lod/ontology/SmallBusinessAdministration
kwg-ont:SmallBusinessAdministration rdf:type owl:Class ;
                                    rdfs:subClassOf kwg-ont:Program ;
                                    rdfs:comment "Source - OpenFEMA (https://www.fema.gov/about/openfema/data-sets)" ;
                                    rdfs:label "Small Business Administration" .


###  http://stko-kwg.geog.ucsb.edu/lod/ontology/SmokePlumeObservableProperty
kwg-ont:SmokePlumeObservableProperty rdf:type owl:Class ;
                                     rdfs:subClassOf sosa:ObservableProperty ;
                                     rdfs:comment "Source - https://satepsanone.nesdis.noaa.gov/pub/FIRE/web/HMS/Smoke_Polygons/Shapefile/" ;
                                     rdfs:label "Smoke Plume Observable Property" .


###  http://stko-kwg.geog.ucsb.edu/lod/ontology/SmokePlumeObservation
kwg-ont:SmokePlumeObservation rdf:type owl:Class ;
                              rdfs:subClassOf sosa:Observation ,
                                              [ rdf:type owl:Restriction ;
                                                owl:onProperty sosa:hasFeatureOfInterest ;
                                                owl:allValuesFrom kwg-ont:SmokePlumeSnapshot
                                              ] ,
                                              [ rdf:type owl:Restriction ;
                                                owl:onProperty sosa:observedProperty ;
                                                owl:allValuesFrom kwg-ont:SmokePlumeObservableProperty
                                              ] ;
                              rdfs:comment "Source - https://satepsanone.nesdis.noaa.gov/pub/FIRE/web/HMS/Smoke_Polygons/Shapefile/" ;
                              rdfs:label "Smoke Plume Observation" .


###  http://stko-kwg.geog.ucsb.edu/lod/ontology/SmokePlumeSnapshot
kwg-ont:SmokePlumeSnapshot rdf:type owl:Class ;
                           rdfs:subClassOf kwg-ont:Hazard ,
                                           <http://www.opengis.net/ont/geosparql#Feature> ,
                                           sosa:FeatureOfInterest ,
                                           <https://undrr.org/hazard/hip/Smoke> ,
                                           [ rdf:type owl:Restriction ;
                                             owl:onProperty kwg-ont:spatialRelation ;
                                             owl:someValuesFrom kwg-ont:AdministrativeRegion_3
                                           ] ,
                                           [ rdf:type owl:Restriction ;
                                             owl:onProperty kwg-ont:spatialRelation ;
                                             owl:someValuesFrom kwg-ont:S2Cell
                                           ] ,
                                           [ rdf:type owl:Restriction ;
                                             owl:onProperty kwg-ont:hasTemporalScope ;
                                             owl:allValuesFrom time:TemporalEntity
                                           ] ,
                                           [ rdf:type owl:Restriction ;
                                             owl:onProperty <http://www.opengis.net/ont/geosparql#hasDefaultGeometry> ;
                                             owl:allValuesFrom <http://www.opengis.net/ont/geosparql#Geometry>
                                           ] ,
                                           [ rdf:type owl:Restriction ;
                                             owl:onProperty <http://www.opengis.net/ont/geosparql#hasGeometry> ;
                                             owl:allValuesFrom <http://www.opengis.net/ont/geosparql#Geometry>
                                           ] ;
                           rdfs:comment "Source - https://satepsanone.nesdis.noaa.gov/pub/FIRE/web/HMS/Smoke_Polygons/Shapefile/" ;
                           rdfs:label "Smoke Plume Snapshot" .


###  http://stko-kwg.geog.ucsb.edu/lod/ontology/SoilMapUnit
kwg-ont:SoilMapUnit rdf:type owl:Class ;
                    rdfs:subClassOf <http://www.opengis.net/ont/geosparql#Feature> ,
                                    sosa:FeatureOfInterest ;
                    rdfs:comment "Source - NRCS-USDA (https://www.nrcs.usda.gov/wps/portal/nrcs/detail/soils/survey/?cid=nrcs142p2_053627)" ;
                    rdfs:label "Soil Map Unit"^^xsd:string .


###  http://stko-kwg.geog.ucsb.edu/lod/ontology/SoilMapUnitObservableProperty
kwg-ont:SoilMapUnitObservableProperty rdf:type owl:Class ;
                                      rdfs:subClassOf sosa:ObservableProperty ;
                                      rdfs:comment "Source - NRCS-USDA (https://www.nrcs.usda.gov/wps/portal/nrcs/detail/soils/survey/?cid=nrcs142p2_053627)" ;
                                      rdfs:label "Soil Map Unit Observable Property" .


###  http://stko-kwg.geog.ucsb.edu/lod/ontology/SoilMapUnitObservation
kwg-ont:SoilMapUnitObservation rdf:type owl:Class ;
                               rdfs:subClassOf sosa:Observation ,
                                               [ rdf:type owl:Restriction ;
                                                 owl:onProperty sosa:observedProperty ;
                                                 owl:allValuesFrom kwg-ont:SoilMapUnitObservableProperty
                                               ] ;
                               rdfs:comment "Source - NRCS-USDA (https://www.nrcs.usda.gov/wps/portal/nrcs/detail/soils/survey/?cid=nrcs142p2_053627)" ;
                               rdfs:label "Soil Map Unit Observation" .


###  http://stko-kwg.geog.ucsb.edu/lod/ontology/SoilMapUnitObservationCollection
kwg-ont:SoilMapUnitObservationCollection rdf:type owl:Class ;
                                         rdfs:subClassOf sosa:ObservationCollection ,
                                                         [ rdf:type owl:Restriction ;
                                                           owl:onProperty sosa:hasMember ;
                                                           owl:someValuesFrom kwg-ont:SoilMapUnitObservation
                                                         ] ,
                                                         [ rdf:type owl:Restriction ;
                                                           owl:onProperty sosa:hasMember ;
                                                           owl:someValuesFrom kwg-ont:SoilMapUnitOverlapObservation
                                                         ] ,
                                                         [ rdf:type owl:Restriction ;
                                                           owl:onProperty sosa:hasFeatureOfInterest ;
                                                           owl:allValuesFrom kwg-ont:SoilMapUnit
                                                         ] ;
                                         rdfs:comment "Source - NRCS-USDA (https://www.nrcs.usda.gov/wps/portal/nrcs/detail/soils/survey/?cid=nrcs142p2_053627)" ;
                                         rdfs:label "Soil Map Unit Observation Collection" .


###  http://stko-kwg.geog.ucsb.edu/lod/ontology/SoilMapUnitOverlapObservation
kwg-ont:SoilMapUnitOverlapObservation rdf:type owl:Class ;
                                      rdfs:subClassOf sosa:Observation ;
                                      rdfs:comment "Source - NRCS-USDA (https://www.nrcs.usda.gov/wps/portal/nrcs/detail/soils/survey/?cid=nrcs142p2_053627)" ,
                                                   "This is a computed value within KWG" ;
                                      rdfs:label "Soil Map Unit Overlap Observation" .


###  http://stko-kwg.geog.ucsb.edu/lod/ontology/StormTrack
kwg-ont:StormTrack rdf:type owl:Class ;
                   rdfs:subClassOf <http://www.opengis.net/ont/geosparql#Feature> ,
                                   sosa:FeatureOfInterest ,
                                   [ rdf:type owl:Restriction ;
                                     owl:onProperty kwg-ont:hasTemporalScope ;
                                     owl:allValuesFrom time:TemporalEntity
                                   ] ;
                   rdfs:comment "Source: https://coast.noaa.gov/hurricanes" ;
                   rdfs:label "Storm Track" .


###  http://stko-kwg.geog.ucsb.edu/lod/ontology/StormTrackObservableProperty
kwg-ont:StormTrackObservableProperty rdf:type owl:Class ;
                                     rdfs:subClassOf sosa:ObservableProperty ;
                                     rdfs:comment "Source: https://coast.noaa.gov/hurricanes" ;
                                     rdfs:label "Storm Track Observable Property" .


###  http://stko-kwg.geog.ucsb.edu/lod/ontology/StormTrackObservation
kwg-ont:StormTrackObservation rdf:type owl:Class ;
                              rdfs:subClassOf sosa:Observation ,
                                              [ rdf:type owl:Restriction ;
                                                owl:onProperty sosa:observedProperty ;
                                                owl:allValuesFrom kwg-ont:StormTrackObservableProperty
                                              ] ;
                              rdfs:comment "Source: https://coast.noaa.gov/hurricanes" ;
                              rdfs:label "Storm Track Observation" .


###  http://stko-kwg.geog.ucsb.edu/lod/ontology/StormTrackObservationCollection
kwg-ont:StormTrackObservationCollection rdf:type owl:Class ;
                                        rdfs:subClassOf sosa:ObservationCollection ,
                                                        [ rdf:type owl:Restriction ;
                                                          owl:onProperty sosa:hasFeatureOfInterest ;
                                                          owl:allValuesFrom kwg-ont:StormTrack
                                                        ] ,
                                                        [ rdf:type owl:Restriction ;
                                                          owl:onProperty sosa:hasMember ;
                                                          owl:allValuesFrom kwg-ont:StormTrackObservation
                                                        ] ,
                                                        [ rdf:type owl:Restriction ;
                                                          owl:onProperty sosa:phenomenonTime ;
                                                          owl:allValuesFrom time:Interval
                                                        ] ;
                                        rdfs:comment "Source: https://coast.noaa.gov/hurricanes" ;
                                        rdfs:label "Storm Track Observation Collection" .


###  http://stko-kwg.geog.ucsb.edu/lod/ontology/StormTracklet
kwg-ont:StormTracklet rdf:type owl:Class ;
                      rdfs:subClassOf <http://www.opengis.net/ont/geosparql#Feature> ,
                                      sosa:FeatureOfInterest ,
                                      [ rdf:type owl:Restriction ;
                                        owl:onProperty kwg-ont:hasTemporalScope ;
                                        owl:allValuesFrom time:TemporalEntity
                                      ] ,
                                      [ rdf:type owl:Restriction ;
                                        owl:onProperty kwg-ont:spatialRelation ;
                                        owl:allValuesFrom kwg-ont:AdministrativeRegion_3
                                      ] ,
                                      [ rdf:type owl:Restriction ;
                                        owl:onProperty kwg-ont:spatialRelation ;
                                        owl:allValuesFrom kwg-ont:S2Cell
                                      ] ,
                                      [ rdf:type owl:Restriction ;
                                        owl:onProperty <http://www.opengis.net/ont/geosparql#hasDefaultGeometry> ;
                                        owl:allValuesFrom <http://www.opengis.net/ont/geosparql#Geometry>
                                      ] ,
                                      [ rdf:type owl:Restriction ;
                                        owl:onProperty <http://www.opengis.net/ont/geosparql#hasGeometry> ;
                                        owl:allValuesFrom <http://www.opengis.net/ont/geosparql#Geometry>
                                      ] ;
                      rdfs:comment "Source: https://coast.noaa.gov/hurricanes" ;
                      rdfs:label "Storm Tracklet" .


###  http://stko-kwg.geog.ucsb.edu/lod/ontology/StormTrackletObservableProperty
kwg-ont:StormTrackletObservableProperty rdf:type owl:Class ;
                                        rdfs:subClassOf sosa:ObservableProperty ;
                                        rdfs:comment "Source: https://coast.noaa.gov/hurricanes" ;
                                        rdfs:label "Storm Tracklet Observable Property" .


###  http://stko-kwg.geog.ucsb.edu/lod/ontology/StormTrackletObservation
kwg-ont:StormTrackletObservation rdf:type owl:Class ;
                                 rdfs:subClassOf sosa:Observation ,
                                                 [ rdf:type owl:Restriction ;
                                                   owl:onProperty sosa:observedProperty ;
                                                   owl:allValuesFrom kwg-ont:StormTrackletObservableProperty
                                                 ] ;
                                 rdfs:comment "Source: https://coast.noaa.gov/hurricanes" ;
                                 rdfs:label "Storm Tracklet Observation" .


###  http://stko-kwg.geog.ucsb.edu/lod/ontology/StormTrackletObservationCollection
kwg-ont:StormTrackletObservationCollection rdf:type owl:Class ;
                                           rdfs:subClassOf sosa:ObservationCollection ,
                                                           [ rdf:type owl:Restriction ;
                                                             owl:onProperty sosa:hasFeatureOfInterest ;
                                                             owl:allValuesFrom kwg-ont:StormTracklet
                                                           ] ,
                                                           [ rdf:type owl:Restriction ;
                                                             owl:onProperty sosa:hasMember ;
                                                             owl:allValuesFrom kwg-ont:StormTrackletObservation
                                                           ] ,
                                                           [ rdf:type owl:Restriction ;
                                                             owl:onProperty sosa:phenomenonTime ;
                                                             owl:allValuesFrom time:Instant
                                                           ] ;
                                           rdfs:comment "Source: https://coast.noaa.gov/hurricanes" ;
                                           rdfs:label "Storm Tracklet Observation Collection" .


###  http://stko-kwg.geog.ucsb.edu/lod/ontology/TornadoMagnitudeObservationCollection
kwg-ont:TornadoMagnitudeObservationCollection rdf:type owl:Class ;
                                              rdfs:subClassOf kwg-ont:MagnitudeObservationCollection ;
                                              rdfs:comment "Source - NOAA (https://www.ncdc.noaa.gov/stormevents/ftp.jsp)" ;
                                              rdfs:label "Tornado Magnitude Observation Collection" .


###  http://stko-kwg.geog.ucsb.edu/lod/ontology/TraumaCareLevel
kwg-ont:TraumaCareLevel rdf:type owl:Class ;
                        rdfs:comment "Source - https://hifld-geoplatform.opendata.arcgis.com/datasets/geoplatform::trauma-levels-1/explore" ;
                        rdfs:label "Trauma Care Level" .


###  http://stko-kwg.geog.ucsb.edu/lod/ontology/TraumaCenter
kwg-ont:TraumaCenter rdf:type owl:Class ;
                     rdfs:subClassOf kwg-ont:Hospital ;
                     rdfs:label "Trauma Center" .


###  http://stko-kwg.geog.ucsb.edu/lod/ontology/TraumaDescription
kwg-ont:TraumaDescription rdf:type owl:Class ;
                          rdfs:comment "Source - https://hifld-geoplatform.opendata.arcgis.com/datasets/geoplatform::trauma-levels-1/explore" ;
                          rdfs:label "Trauma Description" .


###  http://stko-kwg.geog.ucsb.edu/lod/ontology/USCensusMSA
kwg-ont:USCensusMSA rdf:type owl:Class ;
                    rdfs:subClassOf kwg-ont:Region ,
                                    <http://www.opengis.net/ont/geosparql#Feature> ,
                                    sosa:FeatureOfInterest ,
                                    [ rdf:type owl:Restriction ;
                                      owl:onProperty kwg-ont:spatialRelation ;
                                      owl:someValuesFrom kwg-ont:AdministrativeRegion_2
                                    ] ,
                                    [ rdf:type owl:Restriction ;
                                      owl:onProperty kwg-ont:spatialRelation ;
                                      owl:someValuesFrom kwg-ont:S2Cell
                                    ] ,
                                    [ rdf:type owl:Restriction ;
                                      owl:onProperty kwg-ont:hasTemporalScope ;
                                      owl:allValuesFrom time:Instant
                                    ] ,
                                    [ rdf:type owl:Restriction ;
                                      owl:onProperty <http://www.opengis.net/ont/geosparql#hasDefaultGeometry> ;
                                      owl:allValuesFrom <http://www.opengis.net/ont/geosparql#Geometry>
                                    ] ,
                                    [ rdf:type owl:Restriction ;
                                      owl:onProperty <http://www.opengis.net/ont/geosparql#hasGeometry> ;
                                      owl:allValuesFrom <http://www.opengis.net/ont/geosparql#Geometry>
                                    ] ;
                    rdfs:comment "Source - US Census Bureau (https://www.census.gov/data/datasets.html)" ,
                                 "The general concept of a metropolitan or micropolitan statistical area is that of a core area containing a substantial population nucleus, together with adjacent communities having a high degree of economic and social integration with that core." ;
                    rdfs:label "Metropolitan and micropolitan statistical areas" .


###  http://stko-kwg.geog.ucsb.edu/lod/ontology/USClimateDivision
kwg-ont:USClimateDivision rdf:type owl:Class ;
                          rdfs:subClassOf kwg-ont:Region ,
                                          <http://www.opengis.net/ont/geosparql#Feature> ,
                                          sosa:FeatureOfInterest ,
                                          [ rdf:type owl:Restriction ;
                                            owl:onProperty kwg-ont:spatialRelation ;
                                            owl:someValuesFrom kwg-ont:AdministrativeRegion_3
                                          ] ,
                                          [ rdf:type owl:Restriction ;
                                            owl:onProperty kwg-ont:spatialRelation ;
                                            owl:someValuesFrom kwg-ont:S2Cell
                                          ] ,
                                          [ rdf:type owl:Restriction ;
                                            owl:onProperty <http://www.opengis.net/ont/geosparql#hasDefaultGeometry> ;
                                            owl:allValuesFrom <http://www.opengis.net/ont/geosparql#Geometry>
                                          ] ,
                                          [ rdf:type owl:Restriction ;
                                            owl:onProperty <http://www.opengis.net/ont/geosparql#hasGeometry> ;
                                            owl:allValuesFrom <http://www.opengis.net/ont/geosparql#Geometry>
                                          ] ;
                          rdfs:comment "Source - NOAA (https://psl.noaa.gov/data/usclimdivs/boundaries.html)" ;
                          rdfs:label "US Climate Division" .


###  http://stko-kwg.geog.ucsb.edu/lod/ontology/USPresident
kwg-ont:USPresident rdf:type owl:Class ;
                    rdfs:comment "Source - HIFLD (https://hifld-geoplatform.opendata.arcgis.com/datasets/us-district-court-jurisdictions/explore?location=40.830482%2C-90.571266%2C4.68, https://www.uscourts.gov/about-federal-courts/federal-courts-public/court-website-links)" ;
                    rdfs:label "US President" .


###  http://stko-kwg.geog.ucsb.edu/lod/ontology/VulnerabilityObservableProperty
kwg-ont:VulnerabilityObservableProperty rdf:type owl:Class ;
                                        rdfs:subClassOf sosa:ObservableProperty ;
                                        rdfs:comment "Source - https://www.atsdr.cdc.gov/placeandhealth/svi/data_documentation_download.html" ;
                                        rdfs:label "Vulnerability Observable Property" .


###  http://stko-kwg.geog.ucsb.edu/lod/ontology/VulnerabilityObservation
kwg-ont:VulnerabilityObservation rdf:type owl:Class ;
                                 rdfs:subClassOf sosa:Observation ,
                                                 [ rdf:type owl:Restriction ;
                                                   owl:onProperty sosa:observedProperty ;
                                                   owl:allValuesFrom kwg-ont:VulnerabilityObservableProperty
                                                 ] ;
                                 rdfs:comment "Source - https://www.atsdr.cdc.gov/placeandhealth/svi/data_documentation_download.html" ;
                                 rdfs:label "Vulnerability Observation" .


###  http://stko-kwg.geog.ucsb.edu/lod/ontology/WaterControlFacilities-PA-E
kwg-ont:WaterControlFacilities-PA-E rdf:type owl:Class ;
                                    rdfs:subClassOf kwg-ont:PublicAssistance ;
                                    rdfs:comment "Source - OpenFEMA (https://www.fema.gov/about/openfema/data-sets)" ;
                                    rdfs:label "Water Control Facilities (PA-E)" .


###  http://stko-kwg.geog.ucsb.edu/lod/ontology/Wildfire
kwg-ont:Wildfire rdf:type owl:Class ;
                 rdfs:subClassOf kwg-ont:Fire ,
                                 <https://undrr.org/hazard/hip/Wildfires> ;
                 rdfs:label "Wildfire" .


###  http://stko-kwg.geog.ucsb.edu/lod/ontology/WildlandFireUse
kwg-ont:WildlandFireUse rdf:type owl:Class ;
                        rdfs:subClassOf kwg-ont:Fire ;
                        rdfs:label "Wildland Fire" .


###  http://stko-kwg.geog.ucsb.edu/lod/ontology/WindMagnitudeObservationCollection
kwg-ont:WindMagnitudeObservationCollection rdf:type owl:Class ;
                                           rdfs:subClassOf kwg-ont:MagnitudeObservationCollection ;
                                           rdfs:comment "Source - NOAA (https://www.ncdc.noaa.gov/stormevents/ftp.jsp)" ;
                                           rdfs:label "Wind Magnitude Observation Collection" .


###  http://stko-kwg.geog.ucsb.edu/lod/ontology/ZipCodeArea
kwg-ont:ZipCodeArea rdf:type owl:Class ;
                    rdfs:subClassOf kwg-ont:Region ,
                                    <http://www.opengis.net/ont/geosparql#Feature> ,
                                    [ rdf:type owl:Restriction ;
                                      owl:onProperty kwg-ont:spatialRelation ;
                                      owl:someValuesFrom kwg-ont:AdministrativeRegion_3
                                    ] ,
                                    [ rdf:type owl:Restriction ;
                                      owl:onProperty kwg-ont:spatialRelation ;
                                      owl:someValuesFrom kwg-ont:S2Cell
                                    ] ,
                                    [ rdf:type owl:Restriction ;
                                      owl:onProperty <http://www.opengis.net/ont/geosparql#hasDefaultGeometry> ;
                                      owl:allValuesFrom <http://www.opengis.net/ont/geosparql#Geometry>
                                    ] ,
                                    [ rdf:type owl:Restriction ;
                                      owl:onProperty <http://www.opengis.net/ont/geosparql#hasGeometry> ;
                                      owl:allValuesFrom <http://www.opengis.net/ont/geosparql#Geometry>
                                    ] ;
                    rdfs:comment "Source - https://gadm.org/data.html" ,
                                 "Source - https://www.openstreetmap.org/" ;
                    rdfs:label "Zip Code Area" .


###  http://www.opengis.net/ont/geosparql#Feature
<http://www.opengis.net/ont/geosparql#Feature> rdf:type owl:Class ;
                                               rdfs:subClassOf <http://www.opengis.net/ont/geosparql#SpatialObject> ;
                                               owl:disjointWith <http://www.opengis.net/ont/geosparql#Geometry> ;
                                               rdfs:isDefinedBy <http://www.opengis.net/ont/geosparql#> ;
                                               rdfs:label "Feature" ;
                                               skos:definition "A discrete spatial phenomenon in a universe of discourse."@en ;
                                               skos:note "A Feature represents a uniquely identifiable phenomenon, for example a river or an apple. While such phenomena (and therefore the Features used to represent them) are bounded, their boundaries may be crisp (e.g., the declared boundaries of a state), vague (e.g., the delineation of a valley versus its neighboring mountains), and change with time (e.g., a storm front). While discrete in nature, Features may be created from continuous observations, such as an isochrone that determines the region that can be reached by ambulance within 5 minutes."@en ;
                                               skos:prefLabel "Feature"@en .


###  http://www.opengis.net/ont/geosparql#Geometry
<http://www.opengis.net/ont/geosparql#Geometry> rdf:type owl:Class ;
                                                rdfs:subClassOf <http://www.opengis.net/ont/geosparql#SpatialObject> ;
                                                rdfs:isDefinedBy <http://www.opengis.net/ont/geosparql#> ;
                                                skos:definition "A coherent set of direct positions in Euclidian space. A direct position holds the coordinates for a position within a Coordinate Reference System (CRS)."@en ;
                                                skos:note "Geometry can be used as a representation of the shape, extent or location of a Feature, or can exist as a self-contained entity."@en ;
                                                skos:prefLabel "Geometry"@en .


###  http://www.opengis.net/ont/geosparql#SpatialObject
<http://www.opengis.net/ont/geosparql#SpatialObject> rdf:type owl:Class ;
                                                     rdfs:isDefinedBy <http://www.opengis.net/ont/geosparql#> ;
                                                     rdfs:label "Spatial Object" ;
                                                     skos:definition "Anything spatial (having or being a shape, position or an extent)."@en ;
                                                     skos:note "Subclasses are expected to be used for instance data."@en ;
                                                     skos:prefLabel "Spatial Object"@en .


###  http://www.opengis.net/ont/sf#LineString
sf:LineString rdf:type owl:Class ;
              rdfs:subClassOf <http://www.opengis.net/ont/geosparql#Geometry> .


###  http://www.opengis.net/ont/sf#Point
sf:Point rdf:type owl:Class ;
         rdfs:subClassOf <http://www.opengis.net/ont/geosparql#Geometry> .


###  http://www.w3.org/2006/time#Duration
time:Duration rdf:type owl:Class ;
              rdfs:subClassOf time:TemporalDuration ;
              rdfs:comment "Duration of a temporal extent expressed as a number scaled by a temporal unit"@en ;
              rdfs:label "Time duration"@en ;
              skos:definition "Duration of a temporal extent expressed as a number scaled by a temporal unit"@en ;
              skos:note "Alternative to time:DurationDescription to support description of a temporal duration other than using a calendar/clock system."@en .


###  http://www.w3.org/2006/time#Instant
time:Instant rdf:type owl:Class ;
             rdfs:subClassOf time:TemporalEntity ,
                             [ rdf:type owl:Restriction ;
                               owl:onProperty time:inXSDDateTime ;
                               owl:allValuesFrom xsd:dateTime
                             ] ;
             rdfs:comment "A temporal entity with zero extent or duration"@en ;
             rdfs:label "Time instant"@en ;
             skos:definition "A temporal entity with zero extent or duration"@en .


###  http://www.w3.org/2006/time#Interval
time:Interval rdf:type owl:Class ;
              rdfs:subClassOf time:TemporalEntity ;
              rdfs:comment "A temporal entity with an extent or duration"@en ;
              rdfs:label "Time interval"@en ;
              skos:definition "A temporal entity with an extent or duration"@en .


###  http://www.w3.org/2006/time#TemporalDuration
time:TemporalDuration rdf:type owl:Class ;
                      rdfs:comment "Time extent; duration of a time interval separate from its particular start position"@en ;
                      rdfs:label "Temporal duration"@en ;
                      skos:definition "Time extent; duration of a time interval separate from its particular start position"@en .


###  http://www.w3.org/2006/time#TemporalEntity
time:TemporalEntity rdf:type owl:Class ;
                    rdfs:comment "A temporal interval or instant."@en ;
                    rdfs:label "Temporal entity"@en ;
                    skos:definition "A temporal interval or instant."@en .


###  http://www.w3.org/ns/sosa/EarthquakeObservation
sosa:EarthquakeObservation rdf:type owl:Class ;
                           rdfs:subClassOf sosa:Observation ,
                                           [ rdf:type owl:Restriction ;
                                             owl:onProperty sosa:observedProperty ;
                                             owl:allValuesFrom kwg-ont:EarthquakeObservableProperty
                                           ] ;
                           rdfs:comment "Source - USGS (https://earthquake.usgs.gov/earthquakes/search/)" ;
                           rdfs:label "Earthquake Observation" .


###  http://www.w3.org/ns/sosa/FeatureOfInterest
sosa:FeatureOfInterest rdf:type owl:Class ;
                       rdfs:label "Feature Of Interest" .


###  http://www.w3.org/ns/sosa/ObservableProperty
sosa:ObservableProperty rdf:type owl:Class ;
                        rdfs:label "Observable Property" .


###  http://www.w3.org/ns/sosa/Observation
sosa:Observation rdf:type owl:Class ;
                 rdfs:label "Observation" .


###  http://www.w3.org/ns/sosa/ObservationCollection
sosa:ObservationCollection rdf:type owl:Class ;
                           rdfs:label "Observation Collection" .


###  http://www.w3.org/ns/sosa/Platform
sosa:Platform rdf:type owl:Class ;
              rdfs:label "Platform" .


###  http://www.w3.org/ns/sosa/Result
sosa:Result rdf:type owl:Class .


###  http://www.w3.org/ns/sosa/Sensor
sosa:Sensor rdf:type owl:Class ;
            rdfs:label "Sensor" .


###  https://undrr.org/hazard/hip/Drought
<https://undrr.org/hazard/hip/Drought> rdf:type owl:Class .


###  https://undrr.org/hazard/hip/EarthquakeSurfaceRupture
<https://undrr.org/hazard/hip/EarthquakeSurfaceRupture> rdf:type owl:Class .


###  https://undrr.org/hazard/hip/MetereologicalAndHydrological
<https://undrr.org/hazard/hip/MetereologicalAndHydrological> rdf:type owl:Class .


###  https://undrr.org/hazard/hip/Smoke
<https://undrr.org/hazard/hip/Smoke> rdf:type owl:Class .


###  https://undrr.org/hazard/hip/Wildfires
<https://undrr.org/hazard/hip/Wildfires> rdf:type owl:Class .


#################################################################
#    Individuals
#################################################################

###  http://stko-kwg.geog.ucsb.edu/lod/resource/LSADArea.M1
kwgr:LSADArea.M1 rdf:type owl:NamedIndividual ,
                          kwg-ont:LSADArea ;
                 rdfs:comment "ACS label: Metro Area (suffix)" ;
                 rdfs:label "Metropolitan Statistical Area" .


###  http://stko-kwg.geog.ucsb.edu/lod/resource/LSADArea.M2
kwgr:LSADArea.M2 rdf:type owl:NamedIndividual ,
                          kwg-ont:LSADArea ;
                 rdfs:comment "ACS label: Micro Area (suffix)" ;
                 rdfs:label "Micropolitan Statistical Area" .


###  http://stko-kwg.geog.ucsb.edu/lod/resource/administrativeLevel.LOCAL
kwgr:administrativeLevel.LOCAL rdf:type owl:NamedIndividual ,
                                        kwg-ont:AdministrativeLevel ;
                               rdfs:label "local" .


###  http://stko-kwg.geog.ucsb.edu/lod/resource/administrativeLevel.OTHER
kwgr:administrativeLevel.OTHER rdf:type owl:NamedIndividual ,
                                        kwg-ont:AdministrativeLevel ;
                               rdfs:label "other" .


###  http://stko-kwg.geog.ucsb.edu/lod/resource/administrativeLevel.STATE
kwgr:administrativeLevel.STATE rdf:type owl:NamedIndividual ,
                                        kwg-ont:AdministrativeLevel ;
                               rdfs:label "state" .


###  http://stko-kwg.geog.ucsb.edu/lod/resource/administrativeLevel.TRIBAL
kwgr:administrativeLevel.TRIBAL rdf:type owl:NamedIndividual ,
                                         kwg-ont:AdministrativeLevel ;
                                rdfs:label "tribal" .


###  http://stko-kwg.geog.ucsb.edu/lod/resource/airQualityObservableProperty.CO
kwgr:airQualityObservableProperty.CO rdf:type owl:NamedIndividual ,
                                              kwg-ont:AirPollutant ;
                                     rdfs:label "Daily Max 8-hour CO Concentration" .


###  http://stko-kwg.geog.ucsb.edu/lod/resource/airQualityObservableProperty.NO2
kwgr:airQualityObservableProperty.NO2 rdf:type owl:NamedIndividual ,
                                               kwg-ont:AirPollutant ;
                                      rdfs:label "Daily Max 1-hour NO2 Concentration" .


###  http://stko-kwg.geog.ucsb.edu/lod/resource/airQualityObservableProperty.Ozone
kwgr:airQualityObservableProperty.Ozone rdf:type owl:NamedIndividual ,
                                                 kwg-ont:AirPollutant ;
                                        rdfs:label "Daily Max 8-hour Ozone Concentration" .


###  http://stko-kwg.geog.ucsb.edu/lod/resource/airQualityObservableProperty.PM10
kwgr:airQualityObservableProperty.PM10 rdf:type owl:NamedIndividual ,
                                                kwg-ont:AirPollutant ;
                                       rdfs:label "Daily Mean.PM10 Concentration" .


###  http://stko-kwg.geog.ucsb.edu/lod/resource/airQualityObservableProperty.PM25
kwgr:airQualityObservableProperty.PM25 rdf:type owl:NamedIndividual ,
                                                kwg-ont:AirPollutant ;
                                       rdfs:label "Daily Mean PM2.5 Concentration" .


###  http://stko-kwg.geog.ucsb.edu/lod/resource/airQualityObservableProperty.Pb
kwgr:airQualityObservableProperty.Pb rdf:type owl:NamedIndividual ,
                                              kwg-ont:AirPollutant ;
                                     rdfs:label "Daily Mean Pb Concentration" .


###  http://stko-kwg.geog.ucsb.edu/lod/resource/airQualityObservableProperty.SO2
kwgr:airQualityObservableProperty.SO2 rdf:type owl:NamedIndividual ,
                                               kwg-ont:AirPollutant ;
                                      rdfs:label "Daily Max 1-hour SO2 Concentration" .


###  http://stko-kwg.geog.ucsb.edu/lod/resource/blueskyObservableProperty.PM10ModeledDailyEmission
kwgr:blueskyObservableProperty.PM10ModeledDailyEmission rdf:type owl:NamedIndividual ,
                                                                 kwg-ont:BlueskyWildfireObservableProperty ;
                                                        rdfs:label "Modeled PM10 Daily Emission" .


###  http://stko-kwg.geog.ucsb.edu/lod/resource/blueskyObservableProperty.PM25ModeledDailyEmission
kwgr:blueskyObservableProperty.PM25ModeledDailyEmission rdf:type owl:NamedIndividual ,
                                                                 kwg-ont:BlueskyWildfireObservableProperty ;
                                                        rdfs:label "Modeled PM2.5 Daily Emission" .


###  http://stko-kwg.geog.ucsb.edu/lod/resource/blueskyObservableProperty.modeledGrowthArea
kwgr:blueskyObservableProperty.modeledGrowthArea rdf:type owl:NamedIndividual ,
                                                          kwg-ont:BlueskyWildfireObservableProperty ;
                                                 rdfs:label "Modeled Growth Area" .


###  http://stko-kwg.geog.ucsb.edu/lod/resource/blueskyObservableProperty.modeledGrowthNumLocation
kwgr:blueskyObservableProperty.modeledGrowthNumLocation rdf:type owl:NamedIndividual ,
                                                                 kwg-ont:BlueskyWildfireObservableProperty ;
                                                        rdfs:label "Modeled Growth Number of Locations" .


###  http://stko-kwg.geog.ucsb.edu/lod/resource/censusObservableProperty.femalePopulation
kwgr:censusObservableProperty.femalePopulation rdf:type owl:NamedIndividual ,
                                                        kwg-ont:CensusObservableProperty ;
                                               rdfs:comment "ACS label: SEX BY AGE: Female: Total population -- (Estimate)" ;
                                               rdfs:isDefinedBy "ACS variable: B01001e26" ;
                                               rdfs:label "female population" .


###  http://stko-kwg.geog.ucsb.edu/lod/resource/censusObservableProperty.householdUnits
kwgr:censusObservableProperty.householdUnits rdf:type owl:NamedIndividual ,
                                                      kwg-ont:CensusObservableProperty ;
                                             rdfs:comment "ACS label: HOUSEHOLD TYPE BY UNITS IN STRUCTURE: Total: Households -- (Estimate)" ;
                                             rdfs:isDefinedBy "ACS variable: B11011e1" ;
                                             rdfs:label "household units" .


###  http://stko-kwg.geog.ucsb.edu/lod/resource/censusObservableProperty.malePopulation
kwgr:censusObservableProperty.malePopulation rdf:type owl:NamedIndividual ,
                                                      kwg-ont:CensusObservableProperty ;
                                             rdfs:comment "ACS label: SEX BY AGE: Male: Total population -- (Estimate)" ;
                                             rdfs:isDefinedBy "ACS variable: B01001e2" ;
                                             rdfs:label "male population" .


###  http://stko-kwg.geog.ucsb.edu/lod/resource/censusObservableProperty.totalPopulation
kwgr:censusObservableProperty.totalPopulation rdf:type owl:NamedIndividual ,
                                                       kwg-ont:CensusObservableProperty ;
                                              rdfs:comment "ACS label: SEX BY AGE: Total: Total population -- (Estimate)" ;
                                              rdfs:isDefinedBy "ACS variable: B01001e1" ;
                                              rdfs:label "total population" .


###  http://stko-kwg.geog.ucsb.edu/lod/resource/children
kwgr:children rdf:type owl:NamedIndividual ,
                       kwg-ont:HospitalType ;
              rdfs:label "children" .


###  http://stko-kwg.geog.ucsb.edu/lod/resource/chronicDisease
kwgr:chronicDisease rdf:type owl:NamedIndividual ,
                             kwg-ont:HospitalType ;
                    rdfs:label "chronic disease" .


###  http://stko-kwg.geog.ucsb.edu/lod/resource/climateObservableProperty.CDD
kwgr:climateObservableProperty.CDD rdf:type owl:NamedIndividual ,
                                            kwg-ont:ClimateObservableProperty ;
                                   rdfs:label "cooling degree days" .


###  http://stko-kwg.geog.ucsb.edu/lod/resource/climateObservableProperty.HDD
kwgr:climateObservableProperty.HDD rdf:type owl:NamedIndividual ,
                                            kwg-ont:ClimateObservableProperty ;
                                   rdfs:label "heating degree days" .


###  http://stko-kwg.geog.ucsb.edu/lod/resource/climateObservableProperty.PDSI
kwgr:climateObservableProperty.PDSI rdf:type owl:NamedIndividual ,
                                             kwg-ont:ClimateObservableProperty ;
                                    rdfs:label "palmer drought severity index (PDSI)" .


###  http://stko-kwg.geog.ucsb.edu/lod/resource/climateObservableProperty.PHDI
kwgr:climateObservableProperty.PHDI rdf:type owl:NamedIndividual ,
                                             kwg-ont:ClimateObservableProperty ;
                                    rdfs:label "palmer hydrological drought index (PHDI)" .


###  http://stko-kwg.geog.ucsb.edu/lod/resource/climateObservableProperty.PMDI
kwgr:climateObservableProperty.PMDI rdf:type owl:NamedIndividual ,
                                             kwg-ont:ClimateObservableProperty ;
                                    rdfs:label "palmer modified drought index (PMDI)" .


###  http://stko-kwg.geog.ucsb.edu/lod/resource/climateObservableProperty.PZI
kwgr:climateObservableProperty.PZI rdf:type owl:NamedIndividual ,
                                            kwg-ont:ClimateObservableProperty ;
                                   rdfs:label "palmer z-index (PZI)" .


###  http://stko-kwg.geog.ucsb.edu/lod/resource/climateObservableProperty.avgTemp
kwgr:climateObservableProperty.avgTemp rdf:type owl:NamedIndividual ,
                                                kwg-ont:ClimateObservableProperty ;
                                       rdfs:label "average temperature" .


###  http://stko-kwg.geog.ucsb.edu/lod/resource/climateObservableProperty.maxTemp
kwgr:climateObservableProperty.maxTemp rdf:type owl:NamedIndividual ,
                                                kwg-ont:ClimateObservableProperty ;
                                       rdfs:label "maximum temperature" .


###  http://stko-kwg.geog.ucsb.edu/lod/resource/climateObservableProperty.minTemp
kwgr:climateObservableProperty.minTemp rdf:type owl:NamedIndividual ,
                                                kwg-ont:ClimateObservableProperty ;
                                       rdfs:label "minimum temperature" .


###  http://stko-kwg.geog.ucsb.edu/lod/resource/climateObservableProperty.precipitation
kwgr:climateObservableProperty.precipitation rdf:type owl:NamedIndividual ,
                                                      kwg-ont:ClimateObservableProperty ;
                                             rdfs:label "precipitation" .


###  http://stko-kwg.geog.ucsb.edu/lod/resource/closed
kwgr:closed rdf:type owl:NamedIndividual ,
                     kwg-ont:HospitalStatus ;
            rdfs:label "closed" .


###  http://stko-kwg.geog.ucsb.edu/lod/resource/criticalAccess
kwgr:criticalAccess rdf:type owl:NamedIndividual ,
                             kwg-ont:HospitalType ;
                    rdfs:label "critical access" .


###  http://stko-kwg.geog.ucsb.edu/lod/resource/croplandObservableProperty.alfalfaArea
kwgr:croplandObservableProperty.alfalfaArea rdf:type owl:NamedIndividual ,
                                                     kwg-ont:CroplandObservableProperty ;
                                            rdfs:label "alfalfa area" .


###  http://stko-kwg.geog.ucsb.edu/lod/resource/croplandObservableProperty.almondsArea
kwgr:croplandObservableProperty.almondsArea rdf:type owl:NamedIndividual ,
                                                     kwg-ont:CroplandObservableProperty ;
                                            rdfs:label "almonds area" .


###  http://stko-kwg.geog.ucsb.edu/lod/resource/croplandObservableProperty.applesArea
kwgr:croplandObservableProperty.applesArea rdf:type owl:NamedIndividual ,
                                                    kwg-ont:CroplandObservableProperty ;
                                           rdfs:label "apples area" .


###  http://stko-kwg.geog.ucsb.edu/lod/resource/croplandObservableProperty.apricotsArea
kwgr:croplandObservableProperty.apricotsArea rdf:type owl:NamedIndividual ,
                                                      kwg-ont:CroplandObservableProperty ;
                                             rdfs:label "apricots area" .


###  http://stko-kwg.geog.ucsb.edu/lod/resource/croplandObservableProperty.aquacultureArea
kwgr:croplandObservableProperty.aquacultureArea rdf:type owl:NamedIndividual ,
                                                         kwg-ont:CroplandObservableProperty ;
                                                rdfs:label "aquaculture area" .


###  http://stko-kwg.geog.ucsb.edu/lod/resource/croplandObservableProperty.asparagusArea
kwgr:croplandObservableProperty.asparagusArea rdf:type owl:NamedIndividual ,
                                                       kwg-ont:CroplandObservableProperty ;
                                              rdfs:label "asparagus area" .


###  http://stko-kwg.geog.ucsb.edu/lod/resource/croplandObservableProperty.avocadosArea
kwgr:croplandObservableProperty.avocadosArea rdf:type owl:NamedIndividual ,
                                                      kwg-ont:CroplandObservableProperty ;
                                             rdfs:label "avocados area" .


###  http://stko-kwg.geog.ucsb.edu/lod/resource/croplandObservableProperty.backgroundArea
kwgr:croplandObservableProperty.backgroundArea rdf:type owl:NamedIndividual ,
                                                        kwg-ont:CroplandObservableProperty ;
                                               rdfs:label "background area" .


###  http://stko-kwg.geog.ucsb.edu/lod/resource/croplandObservableProperty.barleyArea
kwgr:croplandObservableProperty.barleyArea rdf:type owl:NamedIndividual ,
                                                    kwg-ont:CroplandObservableProperty ;
                                           rdfs:label "barley area" .


###  http://stko-kwg.geog.ucsb.edu/lod/resource/croplandObservableProperty.barrenArea
kwgr:croplandObservableProperty.barrenArea rdf:type owl:NamedIndividual ,
                                                    kwg-ont:CroplandObservableProperty ;
                                           rdfs:label "barren area" .


###  http://stko-kwg.geog.ucsb.edu/lod/resource/croplandObservableProperty.blueberriesArea
kwgr:croplandObservableProperty.blueberriesArea rdf:type owl:NamedIndividual ,
                                                         kwg-ont:CroplandObservableProperty ;
                                                rdfs:label "blueberries area" .


###  http://stko-kwg.geog.ucsb.edu/lod/resource/croplandObservableProperty.broccoliArea
kwgr:croplandObservableProperty.broccoliArea rdf:type owl:NamedIndividual ,
                                                      kwg-ont:CroplandObservableProperty ;
                                             rdfs:label "broccoli area" .


###  http://stko-kwg.geog.ucsb.edu/lod/resource/croplandObservableProperty.buckwheatArea
kwgr:croplandObservableProperty.buckwheatArea rdf:type owl:NamedIndividual ,
                                                       kwg-ont:CroplandObservableProperty ;
                                              rdfs:label "buckwheat area" .


###  http://stko-kwg.geog.ucsb.edu/lod/resource/croplandObservableProperty.cabbageArea
kwgr:croplandObservableProperty.cabbageArea rdf:type owl:NamedIndividual ,
                                                     kwg-ont:CroplandObservableProperty ;
                                            rdfs:label "cabbage area" .


###  http://stko-kwg.geog.ucsb.edu/lod/resource/croplandObservableProperty.camelinaArea
kwgr:croplandObservableProperty.camelinaArea rdf:type owl:NamedIndividual ,
                                                      kwg-ont:CroplandObservableProperty ;
                                             rdfs:label "camelina area" .


###  http://stko-kwg.geog.ucsb.edu/lod/resource/croplandObservableProperty.caneberriesArea
kwgr:croplandObservableProperty.caneberriesArea rdf:type owl:NamedIndividual ,
                                                         kwg-ont:CroplandObservableProperty ;
                                                rdfs:label "caneberries area" .


###  http://stko-kwg.geog.ucsb.edu/lod/resource/croplandObservableProperty.canolaArea
kwgr:croplandObservableProperty.canolaArea rdf:type owl:NamedIndividual ,
                                                    kwg-ont:CroplandObservableProperty ;
                                           rdfs:label "canola area" .


###  http://stko-kwg.geog.ucsb.edu/lod/resource/croplandObservableProperty.cantaloupesArea
kwgr:croplandObservableProperty.cantaloupesArea rdf:type owl:NamedIndividual ,
                                                         kwg-ont:CroplandObservableProperty ;
                                                rdfs:label "cantaloupes area" .


###  http://stko-kwg.geog.ucsb.edu/lod/resource/croplandObservableProperty.carrotsArea
kwgr:croplandObservableProperty.carrotsArea rdf:type owl:NamedIndividual ,
                                                     kwg-ont:CroplandObservableProperty ;
                                            rdfs:label "carrots area" .


###  http://stko-kwg.geog.ucsb.edu/lod/resource/croplandObservableProperty.cauliflowerArea
kwgr:croplandObservableProperty.cauliflowerArea rdf:type owl:NamedIndividual ,
                                                         kwg-ont:CroplandObservableProperty ;
                                                rdfs:label "cauliflower area" .


###  http://stko-kwg.geog.ucsb.edu/lod/resource/croplandObservableProperty.celeryArea
kwgr:croplandObservableProperty.celeryArea rdf:type owl:NamedIndividual ,
                                                    kwg-ont:CroplandObservableProperty ;
                                           rdfs:label "celery area" .


###  http://stko-kwg.geog.ucsb.edu/lod/resource/croplandObservableProperty.cherriesArea
kwgr:croplandObservableProperty.cherriesArea rdf:type owl:NamedIndividual ,
                                                      kwg-ont:CroplandObservableProperty ;
                                             rdfs:label "cherries area" .


###  http://stko-kwg.geog.ucsb.edu/lod/resource/croplandObservableProperty.chickPeasArea
kwgr:croplandObservableProperty.chickPeasArea rdf:type owl:NamedIndividual ,
                                                       kwg-ont:CroplandObservableProperty ;
                                              rdfs:label "chick peas area" .


###  http://stko-kwg.geog.ucsb.edu/lod/resource/croplandObservableProperty.christmasTreesArea
kwgr:croplandObservableProperty.christmasTreesArea rdf:type owl:NamedIndividual ,
                                                            kwg-ont:CroplandObservableProperty ;
                                                   rdfs:label "christmas trees area" .


###  http://stko-kwg.geog.ucsb.edu/lod/resource/croplandObservableProperty.citrusArea
kwgr:croplandObservableProperty.citrusArea rdf:type owl:NamedIndividual ,
                                                    kwg-ont:CroplandObservableProperty ;
                                           rdfs:label "citrus area" .


###  http://stko-kwg.geog.ucsb.edu/lod/resource/croplandObservableProperty.cloudsNoDataArea
kwgr:croplandObservableProperty.cloudsNoDataArea rdf:type owl:NamedIndividual ,
                                                          kwg-ont:CroplandObservableProperty ;
                                                 rdfs:label "clouds no data area" .


###  http://stko-kwg.geog.ucsb.edu/lod/resource/croplandObservableProperty.cloverWildflowersArea
kwgr:croplandObservableProperty.cloverWildflowersArea rdf:type owl:NamedIndividual ,
                                                               kwg-ont:CroplandObservableProperty ;
                                                      rdfs:label "clover wildflowers area" .


###  http://stko-kwg.geog.ucsb.edu/lod/resource/croplandObservableProperty.cornArea
kwgr:croplandObservableProperty.cornArea rdf:type owl:NamedIndividual ,
                                                  kwg-ont:CroplandObservableProperty ;
                                         rdfs:label "corn area" .


###  http://stko-kwg.geog.ucsb.edu/lod/resource/croplandObservableProperty.cottonArea
kwgr:croplandObservableProperty.cottonArea rdf:type owl:NamedIndividual ,
                                                    kwg-ont:CroplandObservableProperty ;
                                           rdfs:label "cotton area" .


###  http://stko-kwg.geog.ucsb.edu/lod/resource/croplandObservableProperty.cranberriesArea
kwgr:croplandObservableProperty.cranberriesArea rdf:type owl:NamedIndividual ,
                                                         kwg-ont:CroplandObservableProperty ;
                                                rdfs:label "cranberries area" .


###  http://stko-kwg.geog.ucsb.edu/lod/resource/croplandObservableProperty.cucumbersArea
kwgr:croplandObservableProperty.cucumbersArea rdf:type owl:NamedIndividual ,
                                                       kwg-ont:CroplandObservableProperty ;
                                              rdfs:label "cucumbers area" .


###  http://stko-kwg.geog.ucsb.edu/lod/resource/croplandObservableProperty.dblCropBarleyCornArea
kwgr:croplandObservableProperty.dblCropBarleyCornArea rdf:type owl:NamedIndividual ,
                                                               kwg-ont:CroplandObservableProperty ;
                                                      rdfs:label "dbl crop barley corn area" .


###  http://stko-kwg.geog.ucsb.edu/lod/resource/croplandObservableProperty.dblCropBarleySorghumArea
kwgr:croplandObservableProperty.dblCropBarleySorghumArea rdf:type owl:NamedIndividual ,
                                                                  kwg-ont:CroplandObservableProperty ;
                                                         rdfs:label "dbl crop barley sorghum area" .


###  http://stko-kwg.geog.ucsb.edu/lod/resource/croplandObservableProperty.dblCropBarleySoybeansArea
kwgr:croplandObservableProperty.dblCropBarleySoybeansArea rdf:type owl:NamedIndividual ,
                                                                   kwg-ont:CroplandObservableProperty ;
                                                          rdfs:label "dbl crop barley soybeans area" .


###  http://stko-kwg.geog.ucsb.edu/lod/resource/croplandObservableProperty.dblCropCornSoybeansArea
kwgr:croplandObservableProperty.dblCropCornSoybeansArea rdf:type owl:NamedIndividual ,
                                                                 kwg-ont:CroplandObservableProperty ;
                                                        rdfs:label "dbl crop corn soybeans area" .


###  http://stko-kwg.geog.ucsb.edu/lod/resource/croplandObservableProperty.dblCropDurumWhtSorghumArea
kwgr:croplandObservableProperty.dblCropDurumWhtSorghumArea rdf:type owl:NamedIndividual ,
                                                                    kwg-ont:CroplandObservableProperty ;
                                                           rdfs:label "dbl crop durum wht sorghum area" .


###  http://stko-kwg.geog.ucsb.edu/lod/resource/croplandObservableProperty.dblCropLettuceBarleyArea
kwgr:croplandObservableProperty.dblCropLettuceBarleyArea rdf:type owl:NamedIndividual ,
                                                                  kwg-ont:CroplandObservableProperty ;
                                                         rdfs:label "dbl crop lettuce barley area" .


###  http://stko-kwg.geog.ucsb.edu/lod/resource/croplandObservableProperty.dblCropLettuceCantaloupeArea
kwgr:croplandObservableProperty.dblCropLettuceCantaloupeArea rdf:type owl:NamedIndividual ,
                                                                      kwg-ont:CroplandObservableProperty ;
                                                             rdfs:label "dbl crop lettuce cantaloupe area" .


###  http://stko-kwg.geog.ucsb.edu/lod/resource/croplandObservableProperty.dblCropLettuceCottonArea
kwgr:croplandObservableProperty.dblCropLettuceCottonArea rdf:type owl:NamedIndividual ,
                                                                  kwg-ont:CroplandObservableProperty ;
                                                         rdfs:label "dbl crop lettuce cotton area" .


###  http://stko-kwg.geog.ucsb.edu/lod/resource/croplandObservableProperty.dblCropLettuceDurumWhtArea
kwgr:croplandObservableProperty.dblCropLettuceDurumWhtArea rdf:type owl:NamedIndividual ,
                                                                    kwg-ont:CroplandObservableProperty ;
                                                           rdfs:label "dbl crop lettuce durum wht area" .


###  http://stko-kwg.geog.ucsb.edu/lod/resource/croplandObservableProperty.dblCropOatsCornArea
kwgr:croplandObservableProperty.dblCropOatsCornArea rdf:type owl:NamedIndividual ,
                                                             kwg-ont:CroplandObservableProperty ;
                                                    rdfs:label "dbl crop oats corn area" .


###  http://stko-kwg.geog.ucsb.edu/lod/resource/croplandObservableProperty.dblCropSoybeansCottonArea
kwgr:croplandObservableProperty.dblCropSoybeansCottonArea rdf:type owl:NamedIndividual ,
                                                                   kwg-ont:CroplandObservableProperty ;
                                                          rdfs:label "dbl crop soybeans cotton area" .


###  http://stko-kwg.geog.ucsb.edu/lod/resource/croplandObservableProperty.dblCropSoybeansOatsArea
kwgr:croplandObservableProperty.dblCropSoybeansOatsArea rdf:type owl:NamedIndividual ,
                                                                 kwg-ont:CroplandObservableProperty ;
                                                        rdfs:label "dbl crop soybeans oats area" .


###  http://stko-kwg.geog.ucsb.edu/lod/resource/croplandObservableProperty.dblCropTriticaleCornArea
kwgr:croplandObservableProperty.dblCropTriticaleCornArea rdf:type owl:NamedIndividual ,
                                                                  kwg-ont:CroplandObservableProperty ;
                                                         rdfs:label "dbl crop triticale corn area" .


###  http://stko-kwg.geog.ucsb.edu/lod/resource/croplandObservableProperty.dblCropWinwhtCornArea
kwgr:croplandObservableProperty.dblCropWinwhtCornArea rdf:type owl:NamedIndividual ,
                                                               kwg-ont:CroplandObservableProperty ;
                                                      rdfs:label "dbl crop winwht corn area" .


###  http://stko-kwg.geog.ucsb.edu/lod/resource/croplandObservableProperty.dblCropWinwhtCottonArea
kwgr:croplandObservableProperty.dblCropWinwhtCottonArea rdf:type owl:NamedIndividual ,
                                                                 kwg-ont:CroplandObservableProperty ;
                                                        rdfs:label "dbl crop winwht cotton area" .


###  http://stko-kwg.geog.ucsb.edu/lod/resource/croplandObservableProperty.dblCropWinwhtSorghumArea
kwgr:croplandObservableProperty.dblCropWinwhtSorghumArea rdf:type owl:NamedIndividual ,
                                                                  kwg-ont:CroplandObservableProperty ;
                                                         rdfs:label "dbl crop winwht sorghum area" .


###  http://stko-kwg.geog.ucsb.edu/lod/resource/croplandObservableProperty.dblCropWinwhtSoybeansArea
kwgr:croplandObservableProperty.dblCropWinwhtSoybeansArea rdf:type owl:NamedIndividual ,
                                                                   kwg-ont:CroplandObservableProperty ;
                                                          rdfs:label "dbl crop winwht soybeans area" .


###  http://stko-kwg.geog.ucsb.edu/lod/resource/croplandObservableProperty.deciduousForestArea
kwgr:croplandObservableProperty.deciduousForestArea rdf:type owl:NamedIndividual ,
                                                             kwg-ont:CroplandObservableProperty ;
                                                    rdfs:label "deciduous forest area" .


###  http://stko-kwg.geog.ucsb.edu/lod/resource/croplandObservableProperty.developedArea
kwgr:croplandObservableProperty.developedArea rdf:type owl:NamedIndividual ,
                                                       kwg-ont:CroplandObservableProperty ;
                                              rdfs:label "developed area" .


###  http://stko-kwg.geog.ucsb.edu/lod/resource/croplandObservableProperty.developedHighIntensityArea
kwgr:croplandObservableProperty.developedHighIntensityArea rdf:type owl:NamedIndividual ,
                                                                    kwg-ont:CroplandObservableProperty ;
                                                           rdfs:label "developed high intensity area" .


###  http://stko-kwg.geog.ucsb.edu/lod/resource/croplandObservableProperty.developedLowIntensityArea
kwgr:croplandObservableProperty.developedLowIntensityArea rdf:type owl:NamedIndividual ,
                                                                   kwg-ont:CroplandObservableProperty ;
                                                          rdfs:label "developed low intensity area" .


###  http://stko-kwg.geog.ucsb.edu/lod/resource/croplandObservableProperty.developedMedIntensityArea
kwgr:croplandObservableProperty.developedMedIntensityArea rdf:type owl:NamedIndividual ,
                                                                   kwg-ont:CroplandObservableProperty ;
                                                          rdfs:label "developed med intensity area" .


###  http://stko-kwg.geog.ucsb.edu/lod/resource/croplandObservableProperty.developedOpenSpaceArea
kwgr:croplandObservableProperty.developedOpenSpaceArea rdf:type owl:NamedIndividual ,
                                                                kwg-ont:CroplandObservableProperty ;
                                                       rdfs:label "developed open space area" .


###  http://stko-kwg.geog.ucsb.edu/lod/resource/croplandObservableProperty.dryBeansArea
kwgr:croplandObservableProperty.dryBeansArea rdf:type owl:NamedIndividual ,
                                                      kwg-ont:CroplandObservableProperty ;
                                             rdfs:label "dry beans area" .


###  http://stko-kwg.geog.ucsb.edu/lod/resource/croplandObservableProperty.durumWheatArea
kwgr:croplandObservableProperty.durumWheatArea rdf:type owl:NamedIndividual ,
                                                        kwg-ont:CroplandObservableProperty ;
                                               rdfs:label "durum wheat area" .


###  http://stko-kwg.geog.ucsb.edu/lod/resource/croplandObservableProperty.eggplantsArea
kwgr:croplandObservableProperty.eggplantsArea rdf:type owl:NamedIndividual ,
                                                       kwg-ont:CroplandObservableProperty ;
                                              rdfs:label "eggplants area" .


###  http://stko-kwg.geog.ucsb.edu/lod/resource/croplandObservableProperty.evergreenForestArea
kwgr:croplandObservableProperty.evergreenForestArea rdf:type owl:NamedIndividual ,
                                                             kwg-ont:CroplandObservableProperty ;
                                                    rdfs:label "evergreen forest area" .


###  http://stko-kwg.geog.ucsb.edu/lod/resource/croplandObservableProperty.fallowIdleCroplandArea
kwgr:croplandObservableProperty.fallowIdleCroplandArea rdf:type owl:NamedIndividual ,
                                                                kwg-ont:CroplandObservableProperty ;
                                                       rdfs:label "fallow idle cropland area" .


###  http://stko-kwg.geog.ucsb.edu/lod/resource/croplandObservableProperty.flaxseedArea
kwgr:croplandObservableProperty.flaxseedArea rdf:type owl:NamedIndividual ,
                                                      kwg-ont:CroplandObservableProperty ;
                                             rdfs:label "flaxseed area" .


###  http://stko-kwg.geog.ucsb.edu/lod/resource/croplandObservableProperty.forestArea
kwgr:croplandObservableProperty.forestArea rdf:type owl:NamedIndividual ,
                                                    kwg-ont:CroplandObservableProperty ;
                                           rdfs:label "forest area" .


###  http://stko-kwg.geog.ucsb.edu/lod/resource/croplandObservableProperty.garlicArea
kwgr:croplandObservableProperty.garlicArea rdf:type owl:NamedIndividual ,
                                                    kwg-ont:CroplandObservableProperty ;
                                           rdfs:label "garlic area" .


###  http://stko-kwg.geog.ucsb.edu/lod/resource/croplandObservableProperty.gourdsArea
kwgr:croplandObservableProperty.gourdsArea rdf:type owl:NamedIndividual ,
                                                    kwg-ont:CroplandObservableProperty ;
                                           rdfs:label "gourds area" .


###  http://stko-kwg.geog.ucsb.edu/lod/resource/croplandObservableProperty.grapesArea
kwgr:croplandObservableProperty.grapesArea rdf:type owl:NamedIndividual ,
                                                    kwg-ont:CroplandObservableProperty ;
                                           rdfs:label "grapes area" .


###  http://stko-kwg.geog.ucsb.edu/lod/resource/croplandObservableProperty.grasslandPastureArea
kwgr:croplandObservableProperty.grasslandPastureArea rdf:type owl:NamedIndividual ,
                                                              kwg-ont:CroplandObservableProperty ;
                                                     rdfs:label "grassland pasture area" .


###  http://stko-kwg.geog.ucsb.edu/lod/resource/croplandObservableProperty.greensArea
kwgr:croplandObservableProperty.greensArea rdf:type owl:NamedIndividual ,
                                                    kwg-ont:CroplandObservableProperty ;
                                           rdfs:label "greens area" .


###  http://stko-kwg.geog.ucsb.edu/lod/resource/croplandObservableProperty.herbaceousWetlandsArea
kwgr:croplandObservableProperty.herbaceousWetlandsArea rdf:type owl:NamedIndividual ,
                                                                kwg-ont:CroplandObservableProperty ;
                                                       rdfs:label "herbaceous wetlands area" .


###  http://stko-kwg.geog.ucsb.edu/lod/resource/croplandObservableProperty.herbsArea
kwgr:croplandObservableProperty.herbsArea rdf:type owl:NamedIndividual ,
                                                   kwg-ont:CroplandObservableProperty ;
                                          rdfs:label "herbs area" .


###  http://stko-kwg.geog.ucsb.edu/lod/resource/croplandObservableProperty.honeydewMelonsArea
kwgr:croplandObservableProperty.honeydewMelonsArea rdf:type owl:NamedIndividual ,
                                                            kwg-ont:CroplandObservableProperty ;
                                                   rdfs:label "honeydew melons area" .


###  http://stko-kwg.geog.ucsb.edu/lod/resource/croplandObservableProperty.hopsArea
kwgr:croplandObservableProperty.hopsArea rdf:type owl:NamedIndividual ,
                                                  kwg-ont:CroplandObservableProperty ;
                                         rdfs:label "hops area" .


###  http://stko-kwg.geog.ucsb.edu/lod/resource/croplandObservableProperty.lentilsArea
kwgr:croplandObservableProperty.lentilsArea rdf:type owl:NamedIndividual ,
                                                     kwg-ont:CroplandObservableProperty ;
                                            rdfs:label "lentils area" .


###  http://stko-kwg.geog.ucsb.edu/lod/resource/croplandObservableProperty.lettuceArea
kwgr:croplandObservableProperty.lettuceArea rdf:type owl:NamedIndividual ,
                                                     kwg-ont:CroplandObservableProperty ;
                                            rdfs:label "lettuce area" .


###  http://stko-kwg.geog.ucsb.edu/lod/resource/croplandObservableProperty.milletArea
kwgr:croplandObservableProperty.milletArea rdf:type owl:NamedIndividual ,
                                                    kwg-ont:CroplandObservableProperty ;
                                           rdfs:label "millet area" .


###  http://stko-kwg.geog.ucsb.edu/lod/resource/croplandObservableProperty.mintArea
kwgr:croplandObservableProperty.mintArea rdf:type owl:NamedIndividual ,
                                                  kwg-ont:CroplandObservableProperty ;
                                         rdfs:label "mint area" .


###  http://stko-kwg.geog.ucsb.edu/lod/resource/croplandObservableProperty.miscVegsAndFruitsArea
kwgr:croplandObservableProperty.miscVegsAndFruitsArea rdf:type owl:NamedIndividual ,
                                                               kwg-ont:CroplandObservableProperty ;
                                                      rdfs:label "misc vegs and fruits area" .


###  http://stko-kwg.geog.ucsb.edu/lod/resource/croplandObservableProperty.mixedForestArea
kwgr:croplandObservableProperty.mixedForestArea rdf:type owl:NamedIndividual ,
                                                         kwg-ont:CroplandObservableProperty ;
                                                rdfs:label "mixed forest area" .


###  http://stko-kwg.geog.ucsb.edu/lod/resource/croplandObservableProperty.mustardArea
kwgr:croplandObservableProperty.mustardArea rdf:type owl:NamedIndividual ,
                                                     kwg-ont:CroplandObservableProperty ;
                                            rdfs:label "mustard area" .


###  http://stko-kwg.geog.ucsb.edu/lod/resource/croplandObservableProperty.nectarinesArea
kwgr:croplandObservableProperty.nectarinesArea rdf:type owl:NamedIndividual ,
                                                        kwg-ont:CroplandObservableProperty ;
                                               rdfs:label "nectarines area" .


###  http://stko-kwg.geog.ucsb.edu/lod/resource/croplandObservableProperty.nonagUndefinedArea
kwgr:croplandObservableProperty.nonagUndefinedArea rdf:type owl:NamedIndividual ,
                                                            kwg-ont:CroplandObservableProperty ;
                                                   rdfs:label "non-ag undefined area" .


###  http://stko-kwg.geog.ucsb.edu/lod/resource/croplandObservableProperty.oatsArea
kwgr:croplandObservableProperty.oatsArea rdf:type owl:NamedIndividual ,
                                                  kwg-ont:CroplandObservableProperty ;
                                         rdfs:label "oats area" .


###  http://stko-kwg.geog.ucsb.edu/lod/resource/croplandObservableProperty.olivesArea
kwgr:croplandObservableProperty.olivesArea rdf:type owl:NamedIndividual ,
                                                    kwg-ont:CroplandObservableProperty ;
                                           rdfs:label "olives area" .


###  http://stko-kwg.geog.ucsb.edu/lod/resource/croplandObservableProperty.onionsArea
kwgr:croplandObservableProperty.onionsArea rdf:type owl:NamedIndividual ,
                                                    kwg-ont:CroplandObservableProperty ;
                                           rdfs:label "onions area" .


###  http://stko-kwg.geog.ucsb.edu/lod/resource/croplandObservableProperty.openWaterArea
kwgr:croplandObservableProperty.openWaterArea rdf:type owl:NamedIndividual ,
                                                       kwg-ont:CroplandObservableProperty ;
                                              rdfs:label "open water area" .


###  http://stko-kwg.geog.ucsb.edu/lod/resource/croplandObservableProperty.orangesArea
kwgr:croplandObservableProperty.orangesArea rdf:type owl:NamedIndividual ,
                                                     kwg-ont:CroplandObservableProperty ;
                                            rdfs:label "oranges area" .


###  http://stko-kwg.geog.ucsb.edu/lod/resource/croplandObservableProperty.otherCropsArea
kwgr:croplandObservableProperty.otherCropsArea rdf:type owl:NamedIndividual ,
                                                        kwg-ont:CroplandObservableProperty ;
                                               rdfs:label "other crops area" .


###  http://stko-kwg.geog.ucsb.edu/lod/resource/croplandObservableProperty.otherHayNonAlfalfaArea
kwgr:croplandObservableProperty.otherHayNonAlfalfaArea rdf:type owl:NamedIndividual ,
                                                                kwg-ont:CroplandObservableProperty ;
                                                       rdfs:label "other hay non alfalfa area" .


###  http://stko-kwg.geog.ucsb.edu/lod/resource/croplandObservableProperty.otherSmallGrainsArea
kwgr:croplandObservableProperty.otherSmallGrainsArea rdf:type owl:NamedIndividual ,
                                                              kwg-ont:CroplandObservableProperty ;
                                                     rdfs:label "other small grains area" .


###  http://stko-kwg.geog.ucsb.edu/lod/resource/croplandObservableProperty.otherTreeCropsArea
kwgr:croplandObservableProperty.otherTreeCropsArea rdf:type owl:NamedIndividual ,
                                                            kwg-ont:CroplandObservableProperty ;
                                                   rdfs:label "other tree crops area" .


###  http://stko-kwg.geog.ucsb.edu/lod/resource/croplandObservableProperty.peachesArea
kwgr:croplandObservableProperty.peachesArea rdf:type owl:NamedIndividual ,
                                                     kwg-ont:CroplandObservableProperty ;
                                            rdfs:label "peaches area" .


###  http://stko-kwg.geog.ucsb.edu/lod/resource/croplandObservableProperty.peanutsArea
kwgr:croplandObservableProperty.peanutsArea rdf:type owl:NamedIndividual ,
                                                     kwg-ont:CroplandObservableProperty ;
                                            rdfs:label "peanuts area" .


###  http://stko-kwg.geog.ucsb.edu/lod/resource/croplandObservableProperty.pearsArea
kwgr:croplandObservableProperty.pearsArea rdf:type owl:NamedIndividual ,
                                                   kwg-ont:CroplandObservableProperty ;
                                          rdfs:label "pears area" .


###  http://stko-kwg.geog.ucsb.edu/lod/resource/croplandObservableProperty.peasArea
kwgr:croplandObservableProperty.peasArea rdf:type owl:NamedIndividual ,
                                                  kwg-ont:CroplandObservableProperty ;
                                         rdfs:label "peas area" .


###  http://stko-kwg.geog.ucsb.edu/lod/resource/croplandObservableProperty.pecansArea
kwgr:croplandObservableProperty.pecansArea rdf:type owl:NamedIndividual ,
                                                    kwg-ont:CroplandObservableProperty ;
                                           rdfs:label "pecans area" .


###  http://stko-kwg.geog.ucsb.edu/lod/resource/croplandObservableProperty.peppersArea
kwgr:croplandObservableProperty.peppersArea rdf:type owl:NamedIndividual ,
                                                     kwg-ont:CroplandObservableProperty ;
                                            rdfs:label "peppers area" .


###  http://stko-kwg.geog.ucsb.edu/lod/resource/croplandObservableProperty.perennialIceSnowArea
kwgr:croplandObservableProperty.perennialIceSnowArea rdf:type owl:NamedIndividual ,
                                                              kwg-ont:CroplandObservableProperty ;
                                                     rdfs:label "perennial ice snow area" .


###  http://stko-kwg.geog.ucsb.edu/lod/resource/croplandObservableProperty.pistachiosArea
kwgr:croplandObservableProperty.pistachiosArea rdf:type owl:NamedIndividual ,
                                                        kwg-ont:CroplandObservableProperty ;
                                               rdfs:label "pistachios area" .


###  http://stko-kwg.geog.ucsb.edu/lod/resource/croplandObservableProperty.plumsArea
kwgr:croplandObservableProperty.plumsArea rdf:type owl:NamedIndividual ,
                                                   kwg-ont:CroplandObservableProperty ;
                                          rdfs:label "plums area" .


###  http://stko-kwg.geog.ucsb.edu/lod/resource/croplandObservableProperty.pomegranatesArea
kwgr:croplandObservableProperty.pomegranatesArea rdf:type owl:NamedIndividual ,
                                                          kwg-ont:CroplandObservableProperty ;
                                                 rdfs:label "pomegranates area" .


###  http://stko-kwg.geog.ucsb.edu/lod/resource/croplandObservableProperty.popOrOrnCornArea
kwgr:croplandObservableProperty.popOrOrnCornArea rdf:type owl:NamedIndividual ,
                                                          kwg-ont:CroplandObservableProperty ;
                                                 rdfs:label "pop or orn corn area" .


###  http://stko-kwg.geog.ucsb.edu/lod/resource/croplandObservableProperty.potatoesArea
kwgr:croplandObservableProperty.potatoesArea rdf:type owl:NamedIndividual ,
                                                      kwg-ont:CroplandObservableProperty ;
                                             rdfs:label "potatoes area" .


###  http://stko-kwg.geog.ucsb.edu/lod/resource/croplandObservableProperty.prunesArea
kwgr:croplandObservableProperty.prunesArea rdf:type owl:NamedIndividual ,
                                                    kwg-ont:CroplandObservableProperty ;
                                           rdfs:label "prunes area" .


###  http://stko-kwg.geog.ucsb.edu/lod/resource/croplandObservableProperty.pumpkinsArea
kwgr:croplandObservableProperty.pumpkinsArea rdf:type owl:NamedIndividual ,
                                                      kwg-ont:CroplandObservableProperty ;
                                             rdfs:label "pumpkins area" .


###  http://stko-kwg.geog.ucsb.edu/lod/resource/croplandObservableProperty.radishesArea
kwgr:croplandObservableProperty.radishesArea rdf:type owl:NamedIndividual ,
                                                      kwg-ont:CroplandObservableProperty ;
                                             rdfs:label "radishes area" .


###  http://stko-kwg.geog.ucsb.edu/lod/resource/croplandObservableProperty.rapeSeedArea
kwgr:croplandObservableProperty.rapeSeedArea rdf:type owl:NamedIndividual ,
                                                      kwg-ont:CroplandObservableProperty ;
                                             rdfs:label "rape seed area" .


###  http://stko-kwg.geog.ucsb.edu/lod/resource/croplandObservableProperty.riceArea
kwgr:croplandObservableProperty.riceArea rdf:type owl:NamedIndividual ,
                                                  kwg-ont:CroplandObservableProperty ;
                                         rdfs:label "rice area" .


###  http://stko-kwg.geog.ucsb.edu/lod/resource/croplandObservableProperty.ryeArea
kwgr:croplandObservableProperty.ryeArea rdf:type owl:NamedIndividual ,
                                                 kwg-ont:CroplandObservableProperty ;
                                        rdfs:label "rye area" .


###  http://stko-kwg.geog.ucsb.edu/lod/resource/croplandObservableProperty.safflowerArea
kwgr:croplandObservableProperty.safflowerArea rdf:type owl:NamedIndividual ,
                                                       kwg-ont:CroplandObservableProperty ;
                                              rdfs:label "safflower area" .


###  http://stko-kwg.geog.ucsb.edu/lod/resource/croplandObservableProperty.shrublandArea
kwgr:croplandObservableProperty.shrublandArea rdf:type owl:NamedIndividual ,
                                                       kwg-ont:CroplandObservableProperty ;
                                              rdfs:label "shrubland area" .


###  http://stko-kwg.geog.ucsb.edu/lod/resource/croplandObservableProperty.sodGrassSeedArea
kwgr:croplandObservableProperty.sodGrassSeedArea rdf:type owl:NamedIndividual ,
                                                          kwg-ont:CroplandObservableProperty ;
                                                 rdfs:label "sod grass seed area" .


###  http://stko-kwg.geog.ucsb.edu/lod/resource/croplandObservableProperty.sorghumArea
kwgr:croplandObservableProperty.sorghumArea rdf:type owl:NamedIndividual ,
                                                     kwg-ont:CroplandObservableProperty ;
                                            rdfs:label "sorghum area" .


###  http://stko-kwg.geog.ucsb.edu/lod/resource/croplandObservableProperty.soybeansArea
kwgr:croplandObservableProperty.soybeansArea rdf:type owl:NamedIndividual ,
                                                      kwg-ont:CroplandObservableProperty ;
                                             rdfs:label "soybeans area" .


###  http://stko-kwg.geog.ucsb.edu/lod/resource/croplandObservableProperty.speltzArea
kwgr:croplandObservableProperty.speltzArea rdf:type owl:NamedIndividual ,
                                                    kwg-ont:CroplandObservableProperty ;
                                           rdfs:label "speltz area" .


###  http://stko-kwg.geog.ucsb.edu/lod/resource/croplandObservableProperty.springWheatArea
kwgr:croplandObservableProperty.springWheatArea rdf:type owl:NamedIndividual ,
                                                         kwg-ont:CroplandObservableProperty ;
                                                rdfs:label "spring wheat area" .


###  http://stko-kwg.geog.ucsb.edu/lod/resource/croplandObservableProperty.squashArea
kwgr:croplandObservableProperty.squashArea rdf:type owl:NamedIndividual ,
                                                    kwg-ont:CroplandObservableProperty ;
                                           rdfs:label "squash area" .


###  http://stko-kwg.geog.ucsb.edu/lod/resource/croplandObservableProperty.strawberriesArea
kwgr:croplandObservableProperty.strawberriesArea rdf:type owl:NamedIndividual ,
                                                          kwg-ont:CroplandObservableProperty ;
                                                 rdfs:label "strawberries area" .


###  http://stko-kwg.geog.ucsb.edu/lod/resource/croplandObservableProperty.sugarbeetsArea
kwgr:croplandObservableProperty.sugarbeetsArea rdf:type owl:NamedIndividual ,
                                                        kwg-ont:CroplandObservableProperty ;
                                               rdfs:label "sugarbeets area" .


###  http://stko-kwg.geog.ucsb.edu/lod/resource/croplandObservableProperty.sugarcaneArea
kwgr:croplandObservableProperty.sugarcaneArea rdf:type owl:NamedIndividual ,
                                                       kwg-ont:CroplandObservableProperty ;
                                              rdfs:label "sugarcane area" .


###  http://stko-kwg.geog.ucsb.edu/lod/resource/croplandObservableProperty.sunflowerArea
kwgr:croplandObservableProperty.sunflowerArea rdf:type owl:NamedIndividual ,
                                                       kwg-ont:CroplandObservableProperty ;
                                              rdfs:label "sunflower area" .


###  http://stko-kwg.geog.ucsb.edu/lod/resource/croplandObservableProperty.sweetCornArea
kwgr:croplandObservableProperty.sweetCornArea rdf:type owl:NamedIndividual ,
                                                       kwg-ont:CroplandObservableProperty ;
                                              rdfs:label "sweet corn area" .


###  http://stko-kwg.geog.ucsb.edu/lod/resource/croplandObservableProperty.sweetPotatoesArea
kwgr:croplandObservableProperty.sweetPotatoesArea rdf:type owl:NamedIndividual ,
                                                           kwg-ont:CroplandObservableProperty ;
                                                  rdfs:label "sweet potatoes area" .


###  http://stko-kwg.geog.ucsb.edu/lod/resource/croplandObservableProperty.switchgrassArea
kwgr:croplandObservableProperty.switchgrassArea rdf:type owl:NamedIndividual ,
                                                         kwg-ont:CroplandObservableProperty ;
                                                rdfs:label "switchgrass area" .


###  http://stko-kwg.geog.ucsb.edu/lod/resource/croplandObservableProperty.tobaccoArea
kwgr:croplandObservableProperty.tobaccoArea rdf:type owl:NamedIndividual ,
                                                     kwg-ont:CroplandObservableProperty ;
                                            rdfs:label "tobacco area" .


###  http://stko-kwg.geog.ucsb.edu/lod/resource/croplandObservableProperty.tomatoesArea
kwgr:croplandObservableProperty.tomatoesArea rdf:type owl:NamedIndividual ,
                                                      kwg-ont:CroplandObservableProperty ;
                                             rdfs:label "tomatoes area" .


###  http://stko-kwg.geog.ucsb.edu/lod/resource/croplandObservableProperty.triticaleArea
kwgr:croplandObservableProperty.triticaleArea rdf:type owl:NamedIndividual ,
                                                       kwg-ont:CroplandObservableProperty ;
                                              rdfs:label "triticale area" .


###  http://stko-kwg.geog.ucsb.edu/lod/resource/croplandObservableProperty.turnipsArea
kwgr:croplandObservableProperty.turnipsArea rdf:type owl:NamedIndividual ,
                                                     kwg-ont:CroplandObservableProperty ;
                                            rdfs:label "turnips area" .


###  http://stko-kwg.geog.ucsb.edu/lod/resource/croplandObservableProperty.vetchArea
kwgr:croplandObservableProperty.vetchArea rdf:type owl:NamedIndividual ,
                                                   kwg-ont:CroplandObservableProperty ;
                                          rdfs:label "vetch area" .


###  http://stko-kwg.geog.ucsb.edu/lod/resource/croplandObservableProperty.walnutsArea
kwgr:croplandObservableProperty.walnutsArea rdf:type owl:NamedIndividual ,
                                                     kwg-ont:CroplandObservableProperty ;
                                            rdfs:label "walnuts area" .


###  http://stko-kwg.geog.ucsb.edu/lod/resource/croplandObservableProperty.waterArea
kwgr:croplandObservableProperty.waterArea rdf:type owl:NamedIndividual ,
                                                   kwg-ont:CroplandObservableProperty ;
                                          rdfs:label "water area" .


###  http://stko-kwg.geog.ucsb.edu/lod/resource/croplandObservableProperty.watermelonsArea
kwgr:croplandObservableProperty.watermelonsArea rdf:type owl:NamedIndividual ,
                                                         kwg-ont:CroplandObservableProperty ;
                                                rdfs:label "watermelons area" .


###  http://stko-kwg.geog.ucsb.edu/lod/resource/croplandObservableProperty.wetlandsArea
kwgr:croplandObservableProperty.wetlandsArea rdf:type owl:NamedIndividual ,
                                                      kwg-ont:CroplandObservableProperty ;
                                             rdfs:label "wetlands area" .


###  http://stko-kwg.geog.ucsb.edu/lod/resource/croplandObservableProperty.winterWheatArea
kwgr:croplandObservableProperty.winterWheatArea rdf:type owl:NamedIndividual ,
                                                         kwg-ont:CroplandObservableProperty ;
                                                rdfs:label "winter wheat area" .


###  http://stko-kwg.geog.ucsb.edu/lod/resource/croplandObservableProperty.woodyWetlandsArea
kwgr:croplandObservableProperty.woodyWetlandsArea rdf:type owl:NamedIndividual ,
                                                           kwg-ont:CroplandObservableProperty ;
                                                  rdfs:label "woody wetlands area" .


###  http://stko-kwg.geog.ucsb.edu/lod/resource/droughtObservableProperty.DroughtIntensity.D0
kwgr:droughtObservableProperty.DroughtIntensity.D0 rdf:type owl:NamedIndividual ,
                                                            kwg-ont:DroughtIntensity ;
                                                   rdfs:label "droughtIntensity.abnormallyDry" .


###  http://stko-kwg.geog.ucsb.edu/lod/resource/droughtObservableProperty.DroughtIntensity.D1
kwgr:droughtObservableProperty.DroughtIntensity.D1 rdf:type owl:NamedIndividual ,
                                                            kwg-ont:DroughtIntensity ;
                                                   rdfs:label "droughtIntensity.moderateDrought" .


###  http://stko-kwg.geog.ucsb.edu/lod/resource/droughtObservableProperty.DroughtIntensity.D2
kwgr:droughtObservableProperty.DroughtIntensity.D2 rdf:type owl:NamedIndividual ,
                                                            kwg-ont:DroughtIntensity ;
                                                   rdfs:label "droughtIntensity.severeDrought" .


###  http://stko-kwg.geog.ucsb.edu/lod/resource/droughtObservableProperty.DroughtIntensity.D3
kwgr:droughtObservableProperty.DroughtIntensity.D3 rdf:type owl:NamedIndividual ,
                                                            kwg-ont:DroughtIntensity ;
                                                   rdfs:label "droughtIntensity.extremeDrought" .


###  http://stko-kwg.geog.ucsb.edu/lod/resource/droughtObservableProperty.DroughtIntensity.D4
kwgr:droughtObservableProperty.DroughtIntensity.D4 rdf:type owl:NamedIndividual ,
                                                            kwg-ont:DroughtIntensity ;
                                                   rdfs:label "droughtIntensity.exceptionalDrought" .


###  http://stko-kwg.geog.ucsb.edu/lod/resource/earthquakeObservableProperty.depth
kwgr:earthquakeObservableProperty.depth rdf:type owl:NamedIndividual ,
                                                 kwg-ont:EarthquakeObservableProperty .


###  http://stko-kwg.geog.ucsb.edu/lod/resource/earthquakeObservableProperty.depthError
kwgr:earthquakeObservableProperty.depthError rdf:type owl:NamedIndividual ,
                                                      kwg-ont:EarthquakeObservableProperty .


###  http://stko-kwg.geog.ucsb.edu/lod/resource/earthquakeObservableProperty.dmin
kwgr:earthquakeObservableProperty.dmin rdf:type owl:NamedIndividual ,
                                                kwg-ont:EarthquakeObservableProperty .


###  http://stko-kwg.geog.ucsb.edu/lod/resource/earthquakeObservableProperty.gap
kwgr:earthquakeObservableProperty.gap rdf:type owl:NamedIndividual ,
                                               kwg-ont:EarthquakeObservableProperty .


###  http://stko-kwg.geog.ucsb.edu/lod/resource/earthquakeObservableProperty.horizontalError
kwgr:earthquakeObservableProperty.horizontalError rdf:type owl:NamedIndividual ,
                                                           kwg-ont:EarthquakeObservableProperty .


###  http://stko-kwg.geog.ucsb.edu/lod/resource/earthquakeObservableProperty.locationSource
kwgr:earthquakeObservableProperty.locationSource rdf:type owl:NamedIndividual ,
                                                          kwg-ont:EarthquakeObservableProperty .


###  http://stko-kwg.geog.ucsb.edu/lod/resource/earthquakeObservableProperty.mag
kwgr:earthquakeObservableProperty.mag rdf:type owl:NamedIndividual ,
                                               kwg-ont:EarthquakeObservableProperty .


###  http://stko-kwg.geog.ucsb.edu/lod/resource/earthquakeObservableProperty.magError
kwgr:earthquakeObservableProperty.magError rdf:type owl:NamedIndividual ,
                                                    kwg-ont:EarthquakeObservableProperty .


###  http://stko-kwg.geog.ucsb.edu/lod/resource/earthquakeObservableProperty.magNst
kwgr:earthquakeObservableProperty.magNst rdf:type owl:NamedIndividual ,
                                                  kwg-ont:EarthquakeObservableProperty .


###  http://stko-kwg.geog.ucsb.edu/lod/resource/earthquakeObservableProperty.magSource
kwgr:earthquakeObservableProperty.magSource rdf:type owl:NamedIndividual ,
                                                     kwg-ont:EarthquakeObservableProperty .


###  http://stko-kwg.geog.ucsb.edu/lod/resource/earthquakeObservableProperty.magType
kwgr:earthquakeObservableProperty.magType rdf:type owl:NamedIndividual ,
                                                   kwg-ont:EarthquakeObservableProperty .


###  http://stko-kwg.geog.ucsb.edu/lod/resource/earthquakeObservableProperty.net
kwgr:earthquakeObservableProperty.net rdf:type owl:NamedIndividual ,
                                               kwg-ont:EarthquakeObservableProperty .


###  http://stko-kwg.geog.ucsb.edu/lod/resource/earthquakeObservableProperty.nst
kwgr:earthquakeObservableProperty.nst rdf:type owl:NamedIndividual ,
                                               kwg-ont:EarthquakeObservableProperty .


###  http://stko-kwg.geog.ucsb.edu/lod/resource/earthquakeObservableProperty.rms
kwgr:earthquakeObservableProperty.rms rdf:type owl:NamedIndividual ,
                                               kwg-ont:EarthquakeObservableProperty .


###  http://stko-kwg.geog.ucsb.edu/lod/resource/earthquakeObservableProperty.status
kwgr:earthquakeObservableProperty.status rdf:type owl:NamedIndividual ,
                                                  kwg-ont:EarthquakeObservableProperty .


###  http://stko-kwg.geog.ucsb.edu/lod/resource/earthquakeObservableProperty.type
kwgr:earthquakeObservableProperty.type rdf:type owl:NamedIndividual ,
                                                kwg-ont:EarthquakeObservableProperty .


###  http://stko-kwg.geog.ucsb.edu/lod/resource/generalAcuteCare
kwgr:generalAcuteCare rdf:type owl:NamedIndividual ,
                               kwg-ont:HospitalType ;
                      rdfs:label "general acute care" .


###  http://stko-kwg.geog.ucsb.edu/lod/resource/impactObservableProperty.damageCrop
kwgr:impactObservableProperty.damageCrop rdf:type owl:NamedIndividual ,
                                                  kwg-ont:ImpactObservableProperty ;
                                         rdfs:label "damage crop" .


###  http://stko-kwg.geog.ucsb.edu/lod/resource/impactObservableProperty.damageProperty
kwgr:impactObservableProperty.damageProperty rdf:type owl:NamedIndividual ,
                                                      kwg-ont:ImpactObservableProperty ;
                                             rdfs:label "damage property" .


###  http://stko-kwg.geog.ucsb.edu/lod/resource/impactObservableProperty.deathDirect
kwgr:impactObservableProperty.deathDirect rdf:type owl:NamedIndividual ,
                                                   kwg-ont:ImpactObservableProperty ;
                                          rdfs:label "death direct" .


###  http://stko-kwg.geog.ucsb.edu/lod/resource/impactObservableProperty.deathIndirect
kwgr:impactObservableProperty.deathIndirect rdf:type owl:NamedIndividual ,
                                                     kwg-ont:ImpactObservableProperty ;
                                            rdfs:label "death indirect" .


###  http://stko-kwg.geog.ucsb.edu/lod/resource/impactObservableProperty.injuryDirect
kwgr:impactObservableProperty.injuryDirect rdf:type owl:NamedIndividual ,
                                                    kwg-ont:ImpactObservableProperty ;
                                           rdfs:label "injury direct" .


###  http://stko-kwg.geog.ucsb.edu/lod/resource/impactObservableProperty.injuryIndirect
kwgr:impactObservableProperty.injuryIndirect rdf:type owl:NamedIndividual ,
                                                      kwg-ont:ImpactObservableProperty ;
                                             rdfs:label "injury indirect" .


###  http://stko-kwg.geog.ucsb.edu/lod/resource/longTermCare
kwgr:longTermCare rdf:type owl:NamedIndividual ,
                           kwg-ont:HospitalType ;
                  rdfs:label "long term care" .


###  http://stko-kwg.geog.ucsb.edu/lod/resource/magnitudeObservableProperty.estimateSustainedWidth
kwgr:magnitudeObservableProperty.estimateSustainedWidth rdf:type owl:NamedIndividual ,
                                                                 kwg-ont:MagnitudeObservableProperty ;
                                                        rdfs:label "estimated sustained width" .


###  http://stko-kwg.geog.ucsb.edu/lod/resource/magnitudeObservableProperty.fujitaScale
kwgr:magnitudeObservableProperty.fujitaScale rdf:type owl:NamedIndividual ,
                                                      kwg-ont:MagnitudeObservableProperty ;
                                             rdfs:label "fujita scale" .


###  http://stko-kwg.geog.ucsb.edu/lod/resource/magnitudeObservableProperty.length
kwgr:magnitudeObservableProperty.length rdf:type owl:NamedIndividual ,
                                                 kwg-ont:MagnitudeObservableProperty ;
                                        rdfs:label "length" .


###  http://stko-kwg.geog.ucsb.edu/lod/resource/magnitudeObservableProperty.measuredSustainedWind
kwgr:magnitudeObservableProperty.measuredSustainedWind rdf:type owl:NamedIndividual ,
                                                                kwg-ont:MagnitudeObservableProperty ;
                                                       rdfs:label "measured sustained wind" .


###  http://stko-kwg.geog.ucsb.edu/lod/resource/magnitudeObservableProperty.measuredWind
kwgr:magnitudeObservableProperty.measuredWind rdf:type owl:NamedIndividual ,
                                                       kwg-ont:MagnitudeObservableProperty ;
                                              rdfs:label "measured wind" .


###  http://stko-kwg.geog.ucsb.edu/lod/resource/magnitudeObservableProperty.width
kwgr:magnitudeObservableProperty.width rdf:type owl:NamedIndividual ,
                                                kwg-ont:MagnitudeObservableProperty ;
                                       rdfs:label "hurricane width" .


###  http://stko-kwg.geog.ucsb.edu/lod/resource/magnitudeObservableProperty.windEstimatedGust
kwgr:magnitudeObservableProperty.windEstimatedGust rdf:type owl:NamedIndividual ,
                                                            kwg-ont:MagnitudeObservableProperty ;
                                                   rdfs:label "wind estimated gust" .


###  http://stko-kwg.geog.ucsb.edu/lod/resource/military
kwgr:military rdf:type owl:NamedIndividual ,
                       kwg-ont:HospitalType ;
              rdfs:label "military" .


###  http://stko-kwg.geog.ucsb.edu/lod/resource/mtbsFireObservableProperty.MeandNBRValue
kwgr:mtbsFireObservableProperty.MeandNBRValue rdf:type owl:NamedIndividual ,
                                                       kwg-ont:MTBSFireObservableProperty ;
                                              rdfs:comment "The mean dNBR value sampled from an unburned area outside the fire perimeter" ;
                                              rdfs:label "differenced Normalized Burn Ratio (mean)" .


###  http://stko-kwg.geog.ucsb.edu/lod/resource/mtbsFireObservableProperty.NumberOfAcresBurned
kwgr:mtbsFireObservableProperty.NumberOfAcresBurned rdf:type owl:NamedIndividual ,
                                                             kwg-ont:MTBSFireObservableProperty ;
                                                    rdfs:comment "Number of acres mapped" ;
                                                    rdfs:label "number of acres mapped" .


###  http://stko-kwg.geog.ucsb.edu/lod/resource/mtbsFireObservableProperty.StandardDeviationOfMeandNBRValue
kwgr:mtbsFireObservableProperty.StandardDeviationOfMeandNBRValue rdf:type owl:NamedIndividual ,
                                                                          kwg-ont:MTBSFireObservableProperty ;
                                                                 rdfs:comment "The standard deviation of the mean dNBR value sampled from an unburned area outside the fire perimeter" ;
                                                                 rdfs:label "differenced Normalized Burn Ratio (standard deviation)" .


###  http://stko-kwg.geog.ucsb.edu/lod/resource/nifcFireHumanCause
kwgr:nifcFireHumanCause rdf:type owl:NamedIndividual ,
                                 kwg-ont:FireCause ;
                        rdfs:label "human cause" .


###  http://stko-kwg.geog.ucsb.edu/lod/resource/nifcFireNaturalCause
kwgr:nifcFireNaturalCause rdf:type owl:NamedIndividual ,
                                   kwg-ont:FireCause ;
                          rdfs:label "natural cause" .


###  http://stko-kwg.geog.ucsb.edu/lod/resource/nifcFireObservableProperty.calculatedAcres
kwgr:nifcFireObservableProperty.calculatedAcres rdf:type owl:NamedIndividual ,
                                                         kwg-ont:NIFCFireObservableProperty ;
                                                rdfs:label "calculated acres" .


###  http://stko-kwg.geog.ucsb.edu/lod/resource/nifcFireObservableProperty.fireDiscoveryDateTime
kwgr:nifcFireObservableProperty.fireDiscoveryDateTime rdf:type owl:NamedIndividual ,
                                                               kwg-ont:NIFCFireObservableProperty ;
                                                      rdfs:label "fire discovery date time" .


###  http://stko-kwg.geog.ucsb.edu/lod/resource/nifcFireObservableProperty.fireOutDateTime
kwgr:nifcFireObservableProperty.fireOutDateTime rdf:type owl:NamedIndividual ,
                                                         kwg-ont:NIFCFireObservableProperty ;
                                                rdfs:label "fire out date time" .


###  http://stko-kwg.geog.ucsb.edu/lod/resource/nifcFireUndeterminedCause
kwgr:nifcFireUndeterminedCause rdf:type owl:NamedIndividual ,
                                        kwg-ont:FireCause ;
                               rdfs:label "undetermined cause" .


###  http://stko-kwg.geog.ucsb.edu/lod/resource/nifcFireUnknownCause
kwgr:nifcFireUnknownCause rdf:type owl:NamedIndividual ,
                                   kwg-ont:FireCause ;
                          rdfs:label "unknown cause" .


###  http://stko-kwg.geog.ucsb.edu/lod/resource/no
kwgr:no rdf:type owl:NamedIndividual ,
                 kwg-ont:HelipadAvailability ;
        rdfs:label "no" .


###  http://stko-kwg.geog.ucsb.edu/lod/resource/open
kwgr:open rdf:type owl:NamedIndividual ,
                   kwg-ont:HospitalStatus ;
          rdfs:label "open" .


###  http://stko-kwg.geog.ucsb.edu/lod/resource/overlapArea.squareMeter
kwgr:overlapArea.squareMeter rdf:type owl:NamedIndividual ,
                                      kwg-ont:SoilMapUnitObservableProperty ;
                             rdfs:comment "overlap area in square meters" ;
                             rdfs:label "overlapArea" .


###  http://stko-kwg.geog.ucsb.edu/lod/resource/pharmacyType.Dialysis_Center
kwgr:pharmacyType.Dialysis_Center rdf:type owl:NamedIndividual ,
                                           kwg-ont:PharmacyType ;
                                  rdfs:label "dialysis center" .


###  http://stko-kwg.geog.ucsb.edu/lod/resource/pharmacyType.Pharmacy
kwgr:pharmacyType.Pharmacy rdf:type owl:NamedIndividual ,
                                    kwg-ont:PharmacyType ;
                           rdfs:label "pharmacy" .


###  http://stko-kwg.geog.ucsb.edu/lod/resource/psychiatric
kwgr:psychiatric rdf:type owl:NamedIndividual ,
                          kwg-ont:HospitalType ;
                 rdfs:label "psychiatric" .


###  http://stko-kwg.geog.ucsb.edu/lod/resource/publicHealthObservableProperty.belowPovertyLevelPercent
kwgr:publicHealthObservableProperty.belowPovertyLevelPercent rdf:type owl:NamedIndividual ,
                                                                      kwg-ont:PublicHealthObservableProperty ;
                                                             rdfs:label "below poverty level percent" .


###  http://stko-kwg.geog.ucsb.edu/lod/resource/publicHealthObservableProperty.diabetesAgeAdjusted20PlusPercent
kwgr:publicHealthObservableProperty.diabetesAgeAdjusted20PlusPercent rdf:type owl:NamedIndividual ,
                                                                              kwg-ont:PublicHealthObservableProperty ;
                                                                     rdfs:label "diabetes age adjusted 20 plus percent" .


###  http://stko-kwg.geog.ucsb.edu/lod/resource/publicHealthObservableProperty.fluVaccination
kwgr:publicHealthObservableProperty.fluVaccination rdf:type owl:NamedIndividual ,
                                                            kwg-ont:PublicHealthObservableProperty ;
                                                   rdfs:comment "Percentage of fee-for-service (FFS) Medicare enrollees that had an annual flu vaccination. Age is a non-modifiable risk factor, and as age increases, poor health outcomes are more likely. We report an age-adjusted rate in order to fairly compare counties with differing age structures." ;
                                                   rdfs:label "flu vaccination" .


###  http://stko-kwg.geog.ucsb.edu/lod/resource/publicHealthObservableProperty.fluVaccination-americanIndian-alaskanNative
kwgr:publicHealthObservableProperty.fluVaccination-americanIndian-alaskanNative rdf:type owl:NamedIndividual ,
                                                                                         kwg-ont:PublicHealthObservableProperty ;
                                                                                rdfs:comment "Percentage of fee-for-service (FFS) Medicare enrollees who are americanIndian-alaskanNative that had an annual flu vaccination. Age is a non-modifiable risk factor, and as age increases, poor health outcomes are more likely. We report an age-adjusted rate in order to fairly compare counties with differing age structures." ;
                                                                                rdfs:label "flu vaccination - americanIndian-alaskanNative" .


###  http://stko-kwg.geog.ucsb.edu/lod/resource/publicHealthObservableProperty.fluVaccination-asian-pacificIslander
kwgr:publicHealthObservableProperty.fluVaccination-asian-pacificIslander rdf:type owl:NamedIndividual ,
                                                                                  kwg-ont:PublicHealthObservableProperty ;
                                                                         rdfs:comment "Percentage of fee-for-service (FFS) Medicare enrollees who are asian-pacificIslander that had an annual flu vaccination. Age is a non-modifiable risk factor, and as age increases, poor health outcomes are more likely. We report an age-adjusted rate in order to fairly compare counties with differing age structures." ;
                                                                         rdfs:label "flu vaccination - asian-pacificIslander" .


###  http://stko-kwg.geog.ucsb.edu/lod/resource/publicHealthObservableProperty.fluVaccination-black
kwgr:publicHealthObservableProperty.fluVaccination-black rdf:type owl:NamedIndividual ,
                                                                  kwg-ont:PublicHealthObservableProperty ;
                                                         rdfs:comment "Percentage of fee-for-service (FFS) Medicare enrollees who are black that had an annual flu vaccination. Age is a non-modifiable risk factor, and as age increases, poor health outcomes are more likely. We report an age-adjusted rate in order to fairly compare counties with differing age structures." ;
                                                         rdfs:label "flu vaccination - black" .


###  http://stko-kwg.geog.ucsb.edu/lod/resource/publicHealthObservableProperty.fluVaccination-hispanic
kwgr:publicHealthObservableProperty.fluVaccination-hispanic rdf:type owl:NamedIndividual ,
                                                                     kwg-ont:PublicHealthObservableProperty ;
                                                            rdfs:comment "Percentage of fee-for-service (FFS) Medicare enrollees who are hispanic that had an annual flu vaccination. Age is a non-modifiable risk factor, and as age increases, poor health outcomes are more likely. We report an age-adjusted rate in order to fairly compare counties with differing age structures." ;
                                                            rdfs:label "flu vaccination - hispanic" .


###  http://stko-kwg.geog.ucsb.edu/lod/resource/publicHealthObservableProperty.fluVaccination-white
kwgr:publicHealthObservableProperty.fluVaccination-white rdf:type owl:NamedIndividual ,
                                                                  kwg-ont:PublicHealthObservableProperty ;
                                                         rdfs:comment "Percentage of fee-for-service (FFS) Medicare enrollees who are white that had an annual flu vaccination. Age is a non-modifiable risk factor, and as age increases, poor health outcomes are more likely. We report an age-adjusted rate in order to fairly compare counties with differing age structures." ;
                                                         rdfs:label "flu vaccination - white" .


###  http://stko-kwg.geog.ucsb.edu/lod/resource/publicHealthObservableProperty.foodEnvironmentIndex
kwgr:publicHealthObservableProperty.foodEnvironmentIndex rdf:type owl:NamedIndividual ,
                                                                  kwg-ont:PublicHealthObservableProperty ;
                                                         rdfs:comment "Index of factors that contribute to a healthy food environment, from 0 (worst) to 10 (best)." ;
                                                         rdfs:label "food and environment index" ,
                                                                    "food environment index" .


###  http://stko-kwg.geog.ucsb.edu/lod/resource/publicHealthObservableProperty.injuryAndDeaths
kwgr:publicHealthObservableProperty.injuryAndDeaths rdf:type owl:NamedIndividual ,
                                                             kwg-ont:PublicHealthObservableProperty ;
                                                    rdfs:comment "Injury Deaths is the number of deaths from planned (e.g. homicide or suicide) and unplanned (e.g. motor vehicle deaths) injuries per 100,000 population. Deaths are counted in the county of residence of the deceased." ;
                                                    rdfs:label "injury and deaths" .


###  http://stko-kwg.geog.ucsb.edu/lod/resource/publicHealthObservableProperty.injuryAndDeaths-americanIndian-alaskanNative
kwgr:publicHealthObservableProperty.injuryAndDeaths-americanIndian-alaskanNative rdf:type owl:NamedIndividual ,
                                                                                          kwg-ont:PublicHealthObservableProperty ;
                                                                                 rdfs:comment "Number of americanIndian-alaskanNative deaths from planned (e.g. homicide or suicide) and unplanned (e.g. motor vehicle deaths) injuries per 100,000 population. Deaths are counted in the county of residence of the deceased." ;
                                                                                 rdfs:label "injury and deaths - americanIndian-alaskanNative" .


###  http://stko-kwg.geog.ucsb.edu/lod/resource/publicHealthObservableProperty.injuryAndDeaths-asian-pacificIslander
kwgr:publicHealthObservableProperty.injuryAndDeaths-asian-pacificIslander rdf:type owl:NamedIndividual ,
                                                                                   kwg-ont:PublicHealthObservableProperty ;
                                                                          rdfs:comment "Number of asian-pacificIslander deaths from planned (e.g. homicide or suicide) and unplanned (e.g. motor vehicle deaths) injuries per 100,000 population. Deaths are counted in the county of residence of the deceased." ;
                                                                          rdfs:label "injury and deaths - asian-pacificIslander" .


###  http://stko-kwg.geog.ucsb.edu/lod/resource/publicHealthObservableProperty.injuryAndDeaths-black
kwgr:publicHealthObservableProperty.injuryAndDeaths-black rdf:type owl:NamedIndividual ,
                                                                   kwg-ont:PublicHealthObservableProperty ;
                                                          rdfs:comment "Number of black deaths from planned (e.g. homicide or suicide) and unplanned (e.g. motor vehicle deaths) injuries per 100,000 population. Deaths are counted in the county of residence of the deceased." ;
                                                          rdfs:label "injury and deaths - black" .


###  http://stko-kwg.geog.ucsb.edu/lod/resource/publicHealthObservableProperty.injuryAndDeaths-hispanic
kwgr:publicHealthObservableProperty.injuryAndDeaths-hispanic rdf:type owl:NamedIndividual ,
                                                                      kwg-ont:PublicHealthObservableProperty ;
                                                             rdfs:label "Number of hispanic deaths from planned (e.g. homicide or suicide) and unplanned (e.g. motor vehicle deaths) injuries per 100,000 population. Deaths are counted in the county of residence of the deceased." ,
                                                                        "injury and deaths - hispanic" .


###  http://stko-kwg.geog.ucsb.edu/lod/resource/publicHealthObservableProperty.injuryAndDeaths-white
kwgr:publicHealthObservableProperty.injuryAndDeaths-white rdf:type owl:NamedIndividual ,
                                                                   kwg-ont:PublicHealthObservableProperty ;
                                                          rdfs:label "Number of white deaths from planned (e.g. homicide or suicide) and unplanned (e.g. motor vehicle deaths) injuries per 100,000 population. Deaths are counted in the county of residence of the deceased." ,
                                                                     "injury and deaths - white" .


###  http://stko-kwg.geog.ucsb.edu/lod/resource/publicHealthObservableProperty.lowBirthWeight
kwgr:publicHealthObservableProperty.lowBirthWeight rdf:type owl:NamedIndividual ,
                                                            kwg-ont:PublicHealthObservableProperty ;
                                                   rdfs:comment "Percentage of live births with low birthweight (< 2,500 grams)." ;
                                                   rdfs:label "llow birth weight" ,
                                                              "low birth weight" .


###  http://stko-kwg.geog.ucsb.edu/lod/resource/publicHealthObservableProperty.lowBirthWeight-americanIndian-alaskanNative
kwgr:publicHealthObservableProperty.lowBirthWeight-americanIndian-alaskanNative rdf:type owl:NamedIndividual ,
                                                                                         kwg-ont:PublicHealthObservableProperty ;
                                                                                rdfs:comment "Percentage of live americanIndian-alaskanNative births with low birthweight (< 2,500 grams)." ;
                                                                                rdfs:label "low birth weight - americanIndian-alaskanNative" .


###  http://stko-kwg.geog.ucsb.edu/lod/resource/publicHealthObservableProperty.lowBirthWeight-asian-pacificIslander
kwgr:publicHealthObservableProperty.lowBirthWeight-asian-pacificIslander rdf:type owl:NamedIndividual ,
                                                                                  kwg-ont:PublicHealthObservableProperty ;
                                                                         rdfs:comment "Percentage of live asian-pacificIslander births with low birthweight (< 2,500 grams)." ;
                                                                         rdfs:label "low birth weight - asian-pacificIslander" .


###  http://stko-kwg.geog.ucsb.edu/lod/resource/publicHealthObservableProperty.lowBirthWeight-black
kwgr:publicHealthObservableProperty.lowBirthWeight-black rdf:type owl:NamedIndividual ,
                                                                  kwg-ont:PublicHealthObservableProperty ;
                                                         rdfs:comment "Percentage of live black births with low birthweight (< 2,500 grams)." ;
                                                         rdfs:label "low birth weight - black" .


###  http://stko-kwg.geog.ucsb.edu/lod/resource/publicHealthObservableProperty.lowBirthWeight-hispanic
kwgr:publicHealthObservableProperty.lowBirthWeight-hispanic rdf:type owl:NamedIndividual ,
                                                                     kwg-ont:PublicHealthObservableProperty ;
                                                            rdfs:comment "Percentage of live hispanic births with low birthweight (< 2,500 grams)." ;
                                                            rdfs:label "low birth weight - hispanic" .


###  http://stko-kwg.geog.ucsb.edu/lod/resource/publicHealthObservableProperty.lowBirthWeight-white
kwgr:publicHealthObservableProperty.lowBirthWeight-white rdf:type owl:NamedIndividual ,
                                                                  kwg-ont:PublicHealthObservableProperty ;
                                                         rdfs:comment "Percentage of live white births with low birthweight (< 2,500 grams)." ;
                                                         rdfs:label "low birth weight - white" ,
                                                                    "low birth weigth - white" .


###  http://stko-kwg.geog.ucsb.edu/lod/resource/publicHealthObservableProperty.mammographyScreening
kwgr:publicHealthObservableProperty.mammographyScreening rdf:type owl:NamedIndividual ,
                                                                  kwg-ont:PublicHealthObservableProperty ;
                                                         rdfs:comment "Percentage of female Medicare enrollees ages 65-74 that received an annual mammography screening." ;
                                                         rdfs:label "mammography screening" .


###  http://stko-kwg.geog.ucsb.edu/lod/resource/publicHealthObservableProperty.mammographyScreening-americanIndian-alaskanNative
kwgr:publicHealthObservableProperty.mammographyScreening-americanIndian-alaskanNative rdf:type owl:NamedIndividual ,
                                                                                               kwg-ont:PublicHealthObservableProperty ;
                                                                                      rdfs:comment "Percentage of female americanIndian-alaskanNative Medicare enrollees ages 65-74 that received an annual mammography screening." ;
                                                                                      rdfs:label "mammography screening - americanIndian-alaskanNative" .


###  http://stko-kwg.geog.ucsb.edu/lod/resource/publicHealthObservableProperty.mammographyScreening-asian-pacificIslander
kwgr:publicHealthObservableProperty.mammographyScreening-asian-pacificIslander rdf:type owl:NamedIndividual ,
                                                                                        kwg-ont:PublicHealthObservableProperty ;
                                                                               rdfs:comment "Percentage of female asian-pacificIslander Medicare enrollees ages 65-74 that received an annual mammography screening." ;
                                                                               rdfs:label "mammography screening - asian-pacificIslander" .


###  http://stko-kwg.geog.ucsb.edu/lod/resource/publicHealthObservableProperty.mammographyScreening-black
kwgr:publicHealthObservableProperty.mammographyScreening-black rdf:type owl:NamedIndividual ,
                                                                        kwg-ont:PublicHealthObservableProperty ;
                                                               rdfs:comment "Percentage of female black Medicare enrollees ages 65-74 that received an annual mammography screening." ;
                                                               rdfs:label "mammography screening - black" .


###  http://stko-kwg.geog.ucsb.edu/lod/resource/publicHealthObservableProperty.mammographyScreening-hispanic
kwgr:publicHealthObservableProperty.mammographyScreening-hispanic rdf:type owl:NamedIndividual ,
                                                                           kwg-ont:PublicHealthObservableProperty ;
                                                                  rdfs:comment "Percentage of female hispanic Medicare enrollees ages 65-74 that received an annual mammography screening." ;
                                                                  rdfs:label "mammography screening - hispanic" .


###  http://stko-kwg.geog.ucsb.edu/lod/resource/publicHealthObservableProperty.mammographyScreening-white
kwgr:publicHealthObservableProperty.mammographyScreening-white rdf:type owl:NamedIndividual ,
                                                                        kwg-ont:PublicHealthObservableProperty ;
                                                               rdfs:comment "Percentage of female white Medicare enrollees ages 65-74 that received an annual mammography screening." ;
                                                               rdfs:label "mammography screening - white" .


###  http://stko-kwg.geog.ucsb.edu/lod/resource/publicHealthObservableProperty.mentalHealthProviders
kwgr:publicHealthObservableProperty.mentalHealthProviders rdf:type owl:NamedIndividual ,
                                                                   kwg-ont:PublicHealthObservableProperty ;
                                                          rdfs:comment "Number of mental health providers." ;
                                                          rdfs:label "mental health providers" .


###  http://stko-kwg.geog.ucsb.edu/lod/resource/publicHealthObservableProperty.obesityAgeAdjusted20PlusPercent
kwgr:publicHealthObservableProperty.obesityAgeAdjusted20PlusPercent rdf:type owl:NamedIndividual ,
                                                                             kwg-ont:PublicHealthObservableProperty ;
                                                                    rdfs:label "obesity age adjusted 20 plus percent" .


###  http://stko-kwg.geog.ucsb.edu/lod/resource/publicHealthObservableProperty.poorMentalHealthDays
kwgr:publicHealthObservableProperty.poorMentalHealthDays rdf:type owl:NamedIndividual ,
                                                                  kwg-ont:PublicHealthObservableProperty ;
                                                         rdfs:comment "Average number of mentally unhealthy days reported in past 30 days (age-adjusted)." ;
                                                         rdfs:label "poor mental health days" .


###  http://stko-kwg.geog.ucsb.edu/lod/resource/publicHealthObservableProperty.ratioOfPopulationToMentalHealthProviders
kwgr:publicHealthObservableProperty.ratioOfPopulationToMentalHealthProviders rdf:type owl:NamedIndividual ,
                                                                                      kwg-ont:PublicHealthObservableProperty ;
                                                                             rdfs:comment "Ratio of population to mental health providers." ;
                                                                             rdfs:label "ratio of population to mental health providers" .


###  http://stko-kwg.geog.ucsb.edu/lod/resource/publicHealthObservableProperty.uninsuredAdults
kwgr:publicHealthObservableProperty.uninsuredAdults rdf:type owl:NamedIndividual ,
                                                             kwg-ont:PublicHealthObservableProperty ;
                                                    rdfs:comment "Percentage of adult population under age 65 without health insurance." ;
                                                    rdfs:label "uninsured adults" .


###  http://stko-kwg.geog.ucsb.edu/lod/resource/publicHealthObservableProperty.uninsuredChildren
kwgr:publicHealthObservableProperty.uninsuredChildren rdf:type owl:NamedIndividual ,
                                                               kwg-ont:PublicHealthObservableProperty ;
                                                      rdfs:comment "Percentage of population who are children without health insurance." ;
                                                      rdfs:label "uninsured children" .


###  http://stko-kwg.geog.ucsb.edu/lod/resource/rehabilitation
kwgr:rehabilitation rdf:type owl:NamedIndividual ,
                             kwg-ont:HospitalType ;
                    rdfs:label "rehabilitation" .


###  http://stko-kwg.geog.ucsb.edu/lod/resource/roadType.C
kwgr:roadType.C rdf:type owl:NamedIndividual ,
                         kwg-ont:RoadType ;
                rdfs:label "county" .


###  http://stko-kwg.geog.ucsb.edu/lod/resource/roadType.I
kwgr:roadType.I rdf:type owl:NamedIndividual ,
                         kwg-ont:RoadType ;
                rdfs:label "interstate" .


###  http://stko-kwg.geog.ucsb.edu/lod/resource/roadType.M
kwgr:roadType.M rdf:type owl:NamedIndividual ,
                         kwg-ont:RoadType ;
                rdfs:label "common name" .


###  http://stko-kwg.geog.ucsb.edu/lod/resource/roadType.O
kwgr:roadType.O rdf:type owl:NamedIndividual ,
                         kwg-ont:RoadType ;
                rdfs:label "other" .


###  http://stko-kwg.geog.ucsb.edu/lod/resource/roadType.S
kwgr:roadType.S rdf:type owl:NamedIndividual ,
                         kwg-ont:RoadType ;
                rdfs:label "state recognized" .


###  http://stko-kwg.geog.ucsb.edu/lod/resource/roadType.U
kwgr:roadType.U rdf:type owl:NamedIndividual ,
                         kwg-ont:RoadType ;
                rdfs:label "U.S." .


###  http://stko-kwg.geog.ucsb.edu/lod/resource/smokePlumeObservableProperty.smokeDensity
kwgr:smokePlumeObservableProperty.smokeDensity rdf:type owl:NamedIndividual ,
                                                        kwg-ont:SmokePlumeObservableProperty ;
                                               rdfs:label "smoke density" .


###  http://stko-kwg.geog.ucsb.edu/lod/resource/soilMapUnitObservableProperty.aws0150wta
kwgr:soilMapUnitObservableProperty.aws0150wta rdf:type owl:NamedIndividual ,
                                                       kwg-ont:SoilMapUnitObservableProperty ;
                                              rdfs:comment "available water storage 0-150 cm - weighted average" ;
                                              rdfs:label "aws0150wta" .


###  http://stko-kwg.geog.ucsb.edu/lod/resource/soilMapUnitObservableProperty.castorieindex
kwgr:soilMapUnitObservableProperty.castorieindex rdf:type owl:NamedIndividual ,
                                                          kwg-ont:SoilMapUnitObservableProperty ;
                                                 rdfs:comment "california storie index" ;
                                                 rdfs:label "castorieindex" .


###  http://stko-kwg.geog.ucsb.edu/lod/resource/soilMapUnitObservableProperty.farmlndcl
kwgr:soilMapUnitObservableProperty.farmlndcl rdf:type owl:NamedIndividual ,
                                                      kwg-ont:SoilMapUnitObservableProperty ;
                                             rdfs:comment "farmland class" ;
                                             rdfs:label "farmlndcl" .


###  http://stko-kwg.geog.ucsb.edu/lod/resource/soilMapUnitObservableProperty.ffd_r
kwgr:soilMapUnitObservableProperty.ffd_r rdf:type owl:NamedIndividual ,
                                                  kwg-ont:SoilMapUnitObservableProperty ;
                                         rdfs:comment "days between last and first frost - representative value" ;
                                         rdfs:label "ffd_r" .


###  http://stko-kwg.geog.ucsb.edu/lod/resource/soilMapUnitObservableProperty.flodfreqdcd
kwgr:soilMapUnitObservableProperty.flodfreqdcd rdf:type owl:NamedIndividual ,
                                                        kwg-ont:SoilMapUnitObservableProperty ;
                                               rdfs:comment "flooding frequency - dominant condition" ;
                                               rdfs:label "flodfreqdcd" .


###  http://stko-kwg.geog.ucsb.edu/lod/resource/soilMapUnitObservableProperty.iccdcd
kwgr:soilMapUnitObservableProperty.iccdcd rdf:type owl:NamedIndividual ,
                                                   kwg-ont:SoilMapUnitObservableProperty ;
                                          rdfs:comment "non-irrigated capability class - dominant condition" ;
                                          rdfs:label "iccdcd" .


###  http://stko-kwg.geog.ucsb.edu/lod/resource/soilMapUnitObservableProperty.nccpi3all
kwgr:soilMapUnitObservableProperty.nccpi3all rdf:type owl:NamedIndividual ,
                                                      kwg-ont:SoilMapUnitObservableProperty ;
                                             rdfs:comment "nccpi v3 - all" ;
                                             rdfs:label "nccpi3all" .


###  http://stko-kwg.geog.ucsb.edu/lod/resource/soilMapUnitObservableProperty.niccdcd
kwgr:soilMapUnitObservableProperty.niccdcd rdf:type owl:NamedIndividual ,
                                                    kwg-ont:SoilMapUnitObservableProperty ;
                                           rdfs:comment "non-irrigated capability class - dominant condition" ;
                                           rdfs:label "niccdcd" .


###  http://stko-kwg.geog.ucsb.edu/lod/resource/soilMapUnitObservableProperty.pondfreqprs
kwgr:soilMapUnitObservableProperty.pondfreqprs rdf:type owl:NamedIndividual ,
                                                        kwg-ont:SoilMapUnitObservableProperty ;
                                               rdfs:comment "ponding frequency - presence" ;
                                               rdfs:label "pondfreqprs" .


###  http://stko-kwg.geog.ucsb.edu/lod/resource/special
kwgr:special rdf:type owl:NamedIndividual ,
                      kwg-ont:HospitalType ;
             rdfs:label "special" .


###  http://stko-kwg.geog.ucsb.edu/lod/resource/stormTrackObservableProperty.category
kwgr:stormTrackObservableProperty.category rdf:type owl:NamedIndividual ,
                                                    kwg-ont:StormTrackObservableProperty ;
                                           rdfs:label "storm track category" .


###  http://stko-kwg.geog.ucsb.edu/lod/resource/stormTrackObservableProperty.maxWindSpeed
kwgr:stormTrackObservableProperty.maxWindSpeed rdf:type owl:NamedIndividual ,
                                                        kwg-ont:StormTrackObservableProperty ;
                                               rdfs:label "storm track max wind speed" .


###  http://stko-kwg.geog.ucsb.edu/lod/resource/stormTrackObservableProperty.minPressure
kwgr:stormTrackObservableProperty.minPressure rdf:type owl:NamedIndividual ,
                                                       kwg-ont:StormTrackObservableProperty ;
                                              rdfs:label "storm track min pressure" .


###  http://stko-kwg.geog.ucsb.edu/lod/resource/stormTrackletObservableProperty.category
kwgr:stormTrackletObservableProperty.category rdf:type owl:NamedIndividual ,
                                                       kwg-ont:StormTrackletObservableProperty ;
                                              rdfs:label "storm tracklet category" .


###  http://stko-kwg.geog.ucsb.edu/lod/resource/stormTrackletObservableProperty.maxWindSpeed
kwgr:stormTrackletObservableProperty.maxWindSpeed rdf:type owl:NamedIndividual ,
                                                           kwg-ont:StormTrackletObservableProperty ;
                                                  rdfs:label "storm tracklet max wind speed" .


###  http://stko-kwg.geog.ucsb.edu/lod/resource/stormTrackletObservableProperty.minPressure
kwgr:stormTrackletObservableProperty.minPressure rdf:type owl:NamedIndividual ,
                                                          kwg-ont:StormTrackletObservableProperty ;
                                                 rdfs:label "storm tracklet min pressure" .


###  http://stko-kwg.geog.ucsb.edu/lod/resource/vulnerabilityObservableProperty.socialVulnerabilityIndex
kwgr:vulnerabilityObservableProperty.socialVulnerabilityIndex rdf:type owl:NamedIndividual ,
                                                                       kwg-ont:VulnerabilityObservableProperty ;
                                                              rdfs:label "social vulnerability index" .


###  http://stko-kwg.geog.ucsb.edu/lod/resource/women
kwgr:women rdf:type owl:NamedIndividual ,
                    kwg-ont:HospitalType ;
           rdfs:label "women" .


###  http://stko-kwg.geog.ucsb.edu/lod/resource/yes
kwgr:yes rdf:type owl:NamedIndividual ,
                  kwg-ont:HelipadAvailability ;
         rdfs:label "yes" .


#################################################################
#    Annotations
#################################################################

xsd:dateTimeStamp rdfs:label "date time stamp"@en .


#################################################################
#    General axioms
#################################################################

[ rdf:type owl:Restriction ;
  owl:onProperty kwg-ont:episodeHasPart ;
  owl:someValuesFrom kwg-ont:NOAAHazardEvent ;
  rdfs:subClassOf kwg-ont:HazardEpisode
] .


[ rdf:type owl:Restriction ;
  owl:onProperty kwg-ont:hasGeometryMember ;
  owl:someValuesFrom <http://www.opengis.net/ont/geosparql#Feature> ;
  rdfs:subClassOf kwg-ont:GeometryCollection
] .


[ rdf:type owl:Restriction ;
  owl:onProperty kwg-ont:hasPart ;
  owl:someValuesFrom kwg-ont:NOAAHazardEvent ;
  rdfs:subClassOf kwg-ont:NOAAHazard
] .


[ rdf:type owl:Restriction ;
  owl:onProperty kwg-ont:hasStormTrack ;
  owl:someValuesFrom kwg-ont:StormTrack ;
  rdfs:subClassOf kwg-ont:NOAAHazard
] .


[ rdf:type owl:Restriction ;
  owl:onProperty kwg-ont:nominatedBy ;
  owl:someValuesFrom kwg-ont:USPresident ;
  rdfs:subClassOf kwg-ont:JudegeInfo
] .


[ rdf:type owl:Restriction ;
  owl:onProperty kwg-ont:nominatedTime ;
  owl:someValuesFrom time:TemporalEntity ;
  rdfs:subClassOf kwg-ont:JudegeInfo
] .


[ rdf:type owl:Restriction ;
  owl:onProperty kwg-ont:startsFrom ;
  owl:someValuesFrom kwg-ont:Fix ;
  rdfs:subClassOf kwg-ont:EventSegment
] .


[ rdf:type owl:Restriction ;
  owl:onProperty kwg-ont:traumaCareLevel ;
  owl:someValuesFrom kwg-ont:TraumaCareLevel ;
  rdfs:subClassOf kwg-ont:TraumaCenter
] .


[ rdf:type owl:Restriction ;
  owl:onProperty kwg-ont:administrativeLevel ;
  owl:allValuesFrom kwg-ont:AdministrativeLevel ;
  rdfs:subClassOf kwg-ont:PublicHealthDepartment
] .


[ rdf:type owl:Restriction ;
  owl:onProperty kwg-ont:endsAt ;
  owl:allValuesFrom kwg-ont:RoadSegmentNode ;
  rdfs:subClassOf kwg-ont:RoadSegment
] .


[ rdf:type owl:Restriction ;
  owl:onProperty kwg-ont:hasChiefJudge ;
  owl:allValuesFrom kwg-ont:ChiefJudge ;
  rdfs:subClassOf kwg-ont:JudegeInfo
] .


[ rdf:type owl:Restriction ;
  owl:onProperty kwg-ont:hasDeclaration ;
  owl:allValuesFrom kwg-ont:Declaration ;
  rdfs:subClassOf kwg-ont:FEMADisaster
] .


[ rdf:type owl:Restriction ;
  owl:onProperty kwg-ont:hasFireCause ;
  owl:allValuesFrom kwg-ont:FireCause ;
  rdfs:subClassOf kwg-ont:NIFCFire
] .


[ rdf:type owl:Restriction ;
  owl:onProperty kwg-ont:hasFireMappingAssessmentLabel ;
  owl:allValuesFrom kwg-ont:FireMappingAssessmentLabel ;
  rdfs:subClassOf kwg-ont:MTBSFire
] .


[ rdf:type owl:Restriction ;
  owl:onProperty kwg-ont:hasGeometry ;
  owl:allValuesFrom kwg-ont:GeometryCollection ;
  rdfs:subClassOf kwg-ont:SoilMapUnit
] .


[ rdf:type owl:Restriction ;
  owl:onProperty kwg-ont:hasJudgeInfo ;
  owl:allValuesFrom kwg-ont:JudegeInfo ;
  rdfs:subClassOf kwg-ont:FederalJudicalDistrict
] .


[ rdf:type owl:Restriction ;
  owl:onProperty kwg-ont:hasMappingProgram ;
  owl:allValuesFrom kwg-ont:MappingProgram ;
  rdfs:subClassOf kwg-ont:MTBSFireObservationCollection
] .


[ rdf:type owl:Restriction ;
  owl:onProperty kwg-ont:hasProgram ;
  owl:allValuesFrom kwg-ont:Program ;
  rdfs:subClassOf kwg-ont:FEMADisaster
] .


[ rdf:type owl:Restriction ;
  owl:onProperty kwg-ont:hasRoadType ;
  owl:allValuesFrom kwg-ont:RoadType ;
  rdfs:subClassOf kwg-ont:RoadSegment
] .


[ rdf:type owl:Restriction ;
  owl:onProperty kwg-ont:hasSegment ;
  owl:allValuesFrom kwg-ont:EventSegment ;
  rdfs:subClassOf kwg-ont:NOAAHazardEvent
] .


[ rdf:type owl:Restriction ;
  owl:onProperty kwg-ont:hasStormTracklet ;
  owl:allValuesFrom kwg-ont:StormTracklet ;
  rdfs:subClassOf kwg-ont:StormTrack
] .


[ rdf:type owl:Restriction ;
  owl:onProperty kwg-ont:hasTraumaDescription ;
  owl:allValuesFrom kwg-ont:TraumaDescription ;
  rdfs:subClassOf kwg-ont:TraumaCareLevel
] .


[ rdf:type owl:Restriction ;
  owl:onProperty kwg-ont:helipadAvailability ;
  owl:allValuesFrom kwg-ont:HelipadAvailability ;
  rdfs:subClassOf kwg-ont:Hospital
] .


[ rdf:type owl:Restriction ;
  owl:onProperty kwg-ont:hospitalStatus ;
  owl:allValuesFrom kwg-ont:HospitalStatus ;
  rdfs:subClassOf kwg-ont:Hospital
] .


[ rdf:type owl:Restriction ;
  owl:onProperty kwg-ont:hospitalType ;
  owl:allValuesFrom kwg-ont:HospitalType ;
  rdfs:subClassOf kwg-ont:Hospital
] .


[ rdf:type owl:Restriction ;
  owl:onProperty kwg-ont:inCircuit ;
  owl:allValuesFrom kwg-ont:RegionalCircuit ;
  rdfs:subClassOf kwg-ont:FederalJudicalDistrict
] .


[ rdf:type owl:Restriction ;
  owl:onProperty kwg-ont:mean ;
  owl:allValuesFrom <http://qudt.org/2.1/schema/qudt#Quantity> ;
  rdfs:subClassOf kwg-ont:ClimateDivisionObservationResult
] .


[ rdf:type owl:Restriction ;
  owl:onProperty kwg-ont:nominatedBy ;
  owl:allValuesFrom kwg-ont:USPresident ;
  rdfs:subClassOf kwg-ont:FederalJudicalDistrict
] .


[ rdf:type owl:Restriction ;
  owl:onProperty kwg-ont:nominatedTime ;
  owl:allValuesFrom time:TemporalEntity ;
  rdfs:subClassOf kwg-ont:FederalJudicalDistrict
] .


[ rdf:type owl:Restriction ;
  owl:onProperty kwg-ont:pharmacyType ;
  owl:allValuesFrom kwg-ont:PharmacyType ;
  rdfs:subClassOf kwg-ont:Pharmacy
] .


[ rdf:type owl:Restriction ;
  owl:onProperty kwg-ont:startsFrom ;
  owl:allValuesFrom kwg-ont:RoadSegmentNode ;
  rdfs:subClassOf kwg-ont:RoadSegment
] .


[ rdf:type owl:Restriction ;
  owl:onProperty kwg-ont:traumaDescriptionSourceDate ;
  owl:allValuesFrom time:Instant ;
  rdfs:subClassOf kwg-ont:TraumaDescription
] .


[ rdf:type owl:Restriction ;
  owl:onProperty kwg-ont:typeOfLSAD ;
  owl:allValuesFrom kwg-ont:LSADArea ;
  rdfs:subClassOf kwg-ont:USCensusMSA
] .


[ rdf:type owl:Restriction ;
  owl:onProperty kwg-ont:correspondingMapID ;
  owl:someValuesFrom xsd:string ;
  rdfs:subClassOf kwg-ont:MTBSFire
] .


[ rdf:type owl:Restriction ;
  owl:onProperty kwg-ont:fipsCountyCode ;
  owl:someValuesFrom xsd:string ;
  rdfs:subClassOf kwg-ont:Declaration
] .


[ rdf:type owl:Restriction ;
  owl:onProperty kwg-ont:fipsStateCode ;
  owl:someValuesFrom xsd:string ;
  rdfs:subClassOf kwg-ont:Declaration
] .


[ rdf:type owl:Restriction ;
  owl:onProperty kwg-ont:hasAzimuth ;
  owl:someValuesFrom xsd:string ;
  rdfs:subClassOf kwg-ont:Fix
] .


[ rdf:type owl:Restriction ;
  owl:onProperty kwg-ont:hasCode ;
  owl:someValuesFrom xsd:string ;
  rdfs:subClassOf kwg-ont:LSADArea
] .


[ rdf:type owl:Restriction ;
  owl:onProperty kwg-ont:hasDeclarationID ;
  owl:someValuesFrom xsd:string ;
  rdfs:subClassOf kwg-ont:Declaration
] .


[ rdf:type owl:Restriction ;
  owl:onProperty kwg-ont:hasFireName ;
  owl:someValuesFrom xsd:string ;
  rdfs:subClassOf kwg-ont:MTBSFire
] .


[ rdf:type owl:Restriction ;
  owl:onProperty kwg-ont:hasNarrative ;
  owl:someValuesFrom xsd:string ;
  rdfs:subClassOf kwg-ont:HazardEpisode
] .


[ rdf:type owl:Restriction ;
  owl:onProperty kwg-ont:hasRange ;
  owl:someValuesFrom xsd:string ;
  rdfs:subClassOf kwg-ont:Fix
] .


[ rdf:type owl:Restriction ;
  owl:onProperty kwg-ont:hasName ;
  owl:someValuesFrom xsd:string ;
  rdfs:subClassOf kwg-ont:FederalJudicalDistrict
] .


[ rdf:type owl:Restriction ;
  owl:onProperty kwg-ont:address ;
  owl:allValuesFrom xsd:string ;
  rdfs:subClassOf kwg-ont:Pharmacy
] .


[ rdf:type owl:Restriction ;
  owl:onProperty kwg-ont:address ;
  owl:allValuesFrom xsd:string ;
  rdfs:subClassOf kwg-ont:PublicHealthDepartment
] .


[ rdf:type owl:Restriction ;
  owl:onProperty kwg-ont:anomaly ;
  owl:allValuesFrom xsd:decimal ;
  rdfs:subClassOf kwg-ont:ClimateDivisionObservationResult
] .


[ rdf:type owl:Restriction ;
  owl:onProperty kwg-ont:cbsaCode ;
  owl:allValuesFrom xsd:string ;
  rdfs:subClassOf kwg-ont:AirQualitySite
] .


[ rdf:type owl:Restriction ;
  owl:onProperty kwg-ont:cbsaName ;
  owl:allValuesFrom xsd:string ;
  rdfs:subClassOf kwg-ont:AirQualitySite
] .


[ rdf:type owl:Restriction ;
  owl:onProperty kwg-ont:compositePercentageInformation ;
  owl:allValuesFrom xsd:string ;
  rdfs:subClassOf kwg-ont:DroughtZoneOverlapObservationCollection
] .


[ rdf:type owl:Restriction ;
  owl:onProperty kwg-ont:hasIncidentName ;
  owl:allValuesFrom xsd:string ;
  rdfs:subClassOf kwg-ont:NIFCFire
] .


[ rdf:type owl:Restriction ;
  owl:onProperty kwg-ont:hasLength ;
  owl:allValuesFrom xsd:decimal ;
  rdfs:subClassOf kwg-ont:RoadSegment
] .


[ rdf:type owl:Restriction ;
  owl:onProperty kwg-ont:hasMapUnitAreaSymbol ;
  owl:allValuesFrom xsd:string ;
  rdfs:subClassOf kwg-ont:SoilMapUnitObservationCollection
] .


[ rdf:type owl:Restriction ;
  owl:onProperty kwg-ont:hasProgramID ;
  owl:allValuesFrom xsd:string ;
  rdfs:subClassOf kwg-ont:Program
] .


[ rdf:type owl:Restriction ;
  owl:onProperty kwg-ont:hasRoadName ;
  owl:allValuesFrom xsd:string ;
  rdfs:subClassOf kwg-ont:RoadSegment
] .


[ rdf:type owl:Restriction ;
  owl:onProperty kwg-ont:hasRoadSign ;
  owl:allValuesFrom xsd:string ;
  rdfs:subClassOf kwg-ont:RoadSegment
] .


[ rdf:type owl:Restriction ;
  owl:onProperty kwg-ont:hasSoilMapUnitKey ;
  owl:allValuesFrom xsd:string ;
  rdfs:subClassOf kwg-ont:SoilMapUnitObservationCollection
] .


[ rdf:type owl:Restriction ;
  owl:onProperty kwg-ont:hasSoilMapUnitSymbol ;
  owl:allValuesFrom xsd:string ;
  rdfs:subClassOf kwg-ont:SoilMapUnitObservationCollection
] .


[ rdf:type owl:Restriction ;
  owl:onProperty kwg-ont:hasZipCode ;
  owl:allValuesFrom xsd:string ;
  rdfs:subClassOf kwg-ont:ZipCodeArea
] .


[ rdf:type owl:Restriction ;
  owl:onProperty kwg-ont:hospitalAddress ;
  owl:allValuesFrom xsd:string ;
  rdfs:subClassOf kwg-ont:Hospital
] .


[ rdf:type owl:Restriction ;
  owl:onProperty kwg-ont:hospitalName ;
  owl:allValuesFrom xsd:string ;
  rdfs:subClassOf kwg-ont:Hospital
] .


[ rdf:type owl:Restriction ;
  owl:onProperty kwg-ont:nielsenMarketZoneDMA ;
  owl:allValuesFrom xsd:int ;
  rdfs:subClassOf kwg-ont:NielsenMarketZone
] .


[ rdf:type owl:Restriction ;
  owl:onProperty kwg-ont:nielsenMarketZoneHHTV ;
  owl:allValuesFrom xsd:int ;
  rdfs:subClassOf kwg-ont:NielsenMarketZone
] .


[ rdf:type owl:Restriction ;
  owl:onProperty kwg-ont:nielsenMarketZoneID ;
  owl:allValuesFrom xsd:double ;
  rdfs:subClassOf kwg-ont:NielsenMarketZone
] .


[ rdf:type owl:Restriction ;
  owl:onProperty kwg-ont:nielsenMarketZonePUSA ;
  owl:allValuesFrom xsd:string ;
  rdfs:subClassOf kwg-ont:NielsenMarketZone
] .


[ rdf:type owl:Restriction ;
  owl:onProperty kwg-ont:nielsenMarketZoneRank ;
  owl:allValuesFrom xsd:int ;
  rdfs:subClassOf kwg-ont:NielsenMarketZone
] .


[ rdf:type owl:Restriction ;
  owl:onProperty kwg-ont:noHospitalBeds ;
  owl:allValuesFrom xsd:decimal ;
  rdfs:subClassOf kwg-ont:Hospital
] .


[ rdf:type owl:Restriction ;
  owl:onProperty kwg-ont:pharmacyName ;
  owl:allValuesFrom xsd:string ;
  rdfs:subClassOf kwg-ont:Pharmacy
] .


[ rdf:type owl:Restriction ;
  owl:onProperty kwg-ont:pocValue ;
  owl:allValuesFrom xsd:string ;
  rdfs:subClassOf kwg-ont:AirQualityInstrument
] .


[ rdf:type owl:Restriction ;
  owl:onProperty kwg-ont:publicHealthDepartmentName ;
  owl:allValuesFrom xsd:string ;
  rdfs:subClassOf kwg-ont:PublicHealthDepartment
] .


[ rdf:type owl:Restriction ;
  owl:onProperty kwg-ont:rank ;
  owl:allValuesFrom xsd:integer ;
  rdfs:subClassOf kwg-ont:ClimateDivisionObservationResult
] .


[ rdf:type owl:Restriction ;
  owl:onProperty kwg-ont:siteID ;
  owl:allValuesFrom xsd:string ;
  rdfs:subClassOf kwg-ont:AirQualitySite
] .


[ rdf:type owl:Restriction ;
  owl:onProperty kwg-ont:siteName ;
  owl:allValuesFrom xsd:string ;
  rdfs:subClassOf kwg-ont:AirQualitySite
] .


[ rdf:type owl:Restriction ;
  owl:onProperty kwg-ont:telephoneNo ;
  owl:allValuesFrom xsd:string ;
  rdfs:subClassOf kwg-ont:Hospital
] .


[ rdf:type owl:Restriction ;
  owl:onProperty kwg-ont:telephoneNo ;
  owl:allValuesFrom xsd:string ;
  rdfs:subClassOf kwg-ont:Pharmacy
] .


[ rdf:type owl:Restriction ;
  owl:onProperty kwg-ont:telephoneNo ;
  owl:allValuesFrom xsd:string ;
  rdfs:subClassOf kwg-ont:PublicHealthDepartment
] .


[ rdf:type owl:Restriction ;
  owl:onProperty kwg-ont:traumaDescriptionForState ;
  owl:allValuesFrom xsd:string ;
  rdfs:subClassOf kwg-ont:TraumaDescription
] .


[ rdf:type owl:Restriction ;
  owl:onProperty kwg-ont:traumaDescriptionSource ;
  owl:allValuesFrom xsd:string ;
  rdfs:subClassOf kwg-ont:TraumaDescription
] .


[ rdf:type owl:Restriction ;
  owl:onProperty kwg-ont:website ;
  owl:allValuesFrom xsd:string ;
  rdfs:subClassOf kwg-ont:Hospital
] .


[ rdf:type owl:Restriction ;
  owl:onProperty kwg-ont:zipCode ;
  owl:allValuesFrom xsd:integer ;
  rdfs:subClassOf kwg-ont:Hospital
] .


[ rdf:type owl:Restriction ;
  owl:onProperty kwg-ont:zipCode ;
  owl:allValuesFrom xsd:integer ;
  rdfs:subClassOf kwg-ont:Pharmacy
] .


[ rdf:type owl:Restriction ;
  owl:onProperty kwg-ont:zipCode ;
  owl:allValuesFrom xsd:integer ;
  rdfs:subClassOf kwg-ont:PublicHealthDepartment
] .


[ rdf:type owl:Restriction ;
  owl:onProperty kwg-ont:zoneNumber ;
  owl:allValuesFrom xsd:string ;
  rdfs:subClassOf kwg-ont:NWZone
] .


[ rdf:type owl:Restriction ;
  owl:onProperty sosa:hasABBR ;
  owl:allValuesFrom xsd:string ;
  rdfs:subClassOf kwg-ont:FederalJudicalDistrict
] .


###  Generated by the OWL API (version 4.5.9.2019-02-01T07:24:44Z) https://github.com/owlcs/owlapi
